update the generated files
git-svn-id: https://projects.brucker.ch/hol-testgen/svn/HOL-TestGen/trunk/hol-testgen@10706 3260e6d1-4efc-4170-b0a7-36055960796d

doc/Employee_DesignModel_UMLPart_generated.thy
@@ -1,4 +1,4 @@
-theory Employee_DesignModel_UMLPart_generated imports "../src/OCL_main"   "../src/OCL_compiler_static"   "../src/OCL_compiler_generator_dynamic" begin
+theory Employee_DesignModel_UMLPart_generated imports "../src/UML_Main"   "../src/compiler/OCL_compiler_static"   "../src/compiler/OCL_compiler_generator_dynamic" begin
 
 (* 1 ************************************ 0 + 1 *)
 text{* 
@@ -109,27 +109,28 @@ text{*
 to OCL types. Again, we exploit that our representation of OCL is a ``shallow embedding'' with a
 one-to-one correspondance of OCL-types to types of the meta-language HOL.  *}
 
-(* 18 ************************************ 24 + 6 *)
+(* 18 ************************************ 24 + 7 *)
 type_synonym Boolean = "\<AA> Boolean"
 type_synonym Set_int = "(\<AA>, int option option) Set"
+type_synonym Set_Integer = "(\<AA>, int option option) Set"
 type_synonym Person = "(\<AA>, typeoid\<^sub>P\<^sub>e\<^sub>r\<^sub>s\<^sub>o\<^sub>n option option) val"
 type_synonym Planet = "(\<AA>, typeoid\<^sub>P\<^sub>l\<^sub>a\<^sub>n\<^sub>e\<^sub>t option option) val"
 type_synonym Galaxy = "(\<AA>, typeoid\<^sub>G\<^sub>a\<^sub>l\<^sub>a\<^sub>x\<^sub>y option option) val"
 type_synonym OclAny = "(\<AA>, typeoid\<^sub>O\<^sub>c\<^sub>l\<^sub>A\<^sub>n\<^sub>y option option) val"
 
-(* 19 ************************************ 30 + 4 *)
+(* 19 ************************************ 31 + 4 *)
 type_synonym Set_Person = "(\<AA>, typeoid\<^sub>P\<^sub>e\<^sub>r\<^sub>s\<^sub>o\<^sub>n option option) Set"
 type_synonym Set_Planet = "(\<AA>, typeoid\<^sub>P\<^sub>l\<^sub>a\<^sub>n\<^sub>e\<^sub>t option option) Set"
 type_synonym Set_Galaxy = "(\<AA>, typeoid\<^sub>G\<^sub>a\<^sub>l\<^sub>a\<^sub>x\<^sub>y option option) Set"
 type_synonym Set_OclAny = "(\<AA>, typeoid\<^sub>O\<^sub>c\<^sub>l\<^sub>A\<^sub>n\<^sub>y option option) Set"
 
-(* 20 ************************************ 34 + 1 *)
+(* 20 ************************************ 35 + 1 *)
 text{* 
    To reuse key-elements of the library like referential equality, we have
 to show that the object universe belongs to the type class ``oclany,'' \ie,
  each class type has to provide a function @{term oid_of} yielding the object id (oid) of the object.  *}
 
-(* 21 ************************************ 35 + 4 *)
+(* 21 ************************************ 36 + 4 *)
 instantiation typeoid\<^sub>P\<^sub>e\<^sub>r\<^sub>s\<^sub>o\<^sub>n :: object
 begin
   definition oid_of_typeoid\<^sub>P\<^sub>e\<^sub>r\<^sub>s\<^sub>o\<^sub>n_def : "oid_of = (\<lambda> mkoid\<^sub>P\<^sub>e\<^sub>r\<^sub>s\<^sub>o\<^sub>n t _ _ \<Rightarrow> (case t of (mk\<^sub>P\<^sub>e\<^sub>r\<^sub>s\<^sub>o\<^sub>n (t) (_) (_) (_) (_)) \<Rightarrow> t))"
@@ -157,7 +158,7 @@ begin
   instance ..
 end
 
-(* 22 ************************************ 39 + 1 *)
+(* 22 ************************************ 40 + 1 *)
 instantiation \<AA> :: object
 begin
   definition oid_of_\<AA>_def : "oid_of = (\<lambda> in\<^sub>P\<^sub>e\<^sub>r\<^sub>s\<^sub>o\<^sub>n Person \<Rightarrow> oid_of Person
@@ -167,52 +168,52 @@ begin
   instance ..
 end
 
-(* 23 ************************************ 40 + 1 *)
+(* 23 ************************************ 41 + 1 *)
 section{* Instantiation of the Generic Strict Equality *}
 
-(* 24 ************************************ 41 + 1 *)
+(* 24 ************************************ 42 + 1 *)
 text{* 
    We instantiate the referential equality
 on @{text "Person"} and @{text "OclAny"}  *}
 
-(* 25 ************************************ 42 + 4 *)
+(* 25 ************************************ 43 + 4 *)
 defs(overloaded) StrictRefEq\<^sub>O\<^sub>b\<^sub>j\<^sub>e\<^sub>c\<^sub>t_\<^sub>P\<^sub>e\<^sub>r\<^sub>s\<^sub>o\<^sub>n : "(x::Person) \<doteq> y \<equiv> StrictRefEq\<^sub>O\<^sub>b\<^sub>j\<^sub>e\<^sub>c\<^sub>t x y"
 defs(overloaded) StrictRefEq\<^sub>O\<^sub>b\<^sub>j\<^sub>e\<^sub>c\<^sub>t_\<^sub>P\<^sub>l\<^sub>a\<^sub>n\<^sub>e\<^sub>t : "(x::Planet) \<doteq> y \<equiv> StrictRefEq\<^sub>O\<^sub>b\<^sub>j\<^sub>e\<^sub>c\<^sub>t x y"
 defs(overloaded) StrictRefEq\<^sub>O\<^sub>b\<^sub>j\<^sub>e\<^sub>c\<^sub>t_\<^sub>G\<^sub>a\<^sub>l\<^sub>a\<^sub>x\<^sub>y : "(x::Galaxy) \<doteq> y \<equiv> StrictRefEq\<^sub>O\<^sub>b\<^sub>j\<^sub>e\<^sub>c\<^sub>t x y"
 defs(overloaded) StrictRefEq\<^sub>O\<^sub>b\<^sub>j\<^sub>e\<^sub>c\<^sub>t_\<^sub>O\<^sub>c\<^sub>l\<^sub>A\<^sub>n\<^sub>y : "(x::OclAny) \<doteq> y \<equiv> StrictRefEq\<^sub>O\<^sub>b\<^sub>j\<^sub>e\<^sub>c\<^sub>t x y"
 
-(* 26 ************************************ 46 + 1 *)
-lemmas [simp,code_unfold] = StrictRefEq\<^sub>O\<^sub>b\<^sub>j\<^sub>e\<^sub>c\<^sub>t_\<^sub>P\<^sub>e\<^sub>r\<^sub>s\<^sub>o\<^sub>n
+(* 26 ************************************ 47 + 1 *)
+lemmas[simp,code_unfold] = StrictRefEq\<^sub>O\<^sub>b\<^sub>j\<^sub>e\<^sub>c\<^sub>t_\<^sub>P\<^sub>e\<^sub>r\<^sub>s\<^sub>o\<^sub>n
                             StrictRefEq\<^sub>O\<^sub>b\<^sub>j\<^sub>e\<^sub>c\<^sub>t_\<^sub>P\<^sub>l\<^sub>a\<^sub>n\<^sub>e\<^sub>t
                             StrictRefEq\<^sub>O\<^sub>b\<^sub>j\<^sub>e\<^sub>c\<^sub>t_\<^sub>G\<^sub>a\<^sub>l\<^sub>a\<^sub>x\<^sub>y
                             StrictRefEq\<^sub>O\<^sub>b\<^sub>j\<^sub>e\<^sub>c\<^sub>t_\<^sub>O\<^sub>c\<^sub>l\<^sub>A\<^sub>n\<^sub>y
 
-(* 27 ************************************ 47 + 1 *)
+(* 27 ************************************ 48 + 1 *)
 text{* 
    For each Class \emph{C}, we will have a casting operation \inlineocl{.oclAsType($C$)},
    a test on the actual type \inlineocl{.oclIsTypeOf($C$)} as well as its relaxed form
    \inlineocl{.oclIsKindOf($C$)} (corresponding exactly to Java's \verb+instanceof+-operator.
  *}
 
-(* 28 ************************************ 48 + 1 *)
+(* 28 ************************************ 49 + 1 *)
 text{* 
    Thus, since we have two class-types in our concrete class hierarchy, we have
 two operations to declare and to provide two overloading definitions for the two static types.
  *}
 
-(* 29 ************************************ 49 + 1 *)
+(* 29 ************************************ 50 + 1 *)
 section{* OclAsType *}
 
-(* 30 ************************************ 50 + 1 *)
+(* 30 ************************************ 51 + 1 *)
 subsection{* Definition *}
 
-(* 31 ************************************ 51 + 4 *)
+(* 31 ************************************ 52 + 4 *)
 consts OclAsType\<^sub>P\<^sub>e\<^sub>r\<^sub>s\<^sub>o\<^sub>n :: "'\<alpha> \<Rightarrow> Person" ("(_) .oclAsType'(Person')")
 consts OclAsType\<^sub>P\<^sub>l\<^sub>a\<^sub>n\<^sub>e\<^sub>t :: "'\<alpha> \<Rightarrow> Planet" ("(_) .oclAsType'(Planet')")
 consts OclAsType\<^sub>G\<^sub>a\<^sub>l\<^sub>a\<^sub>x\<^sub>y :: "'\<alpha> \<Rightarrow> Galaxy" ("(_) .oclAsType'(Galaxy')")
 consts OclAsType\<^sub>O\<^sub>c\<^sub>l\<^sub>A\<^sub>n\<^sub>y :: "'\<alpha> \<Rightarrow> OclAny" ("(_) .oclAsType'(OclAny')")
 
-(* 32 ************************************ 55 + 16 *)
+(* 32 ************************************ 56 + 16 *)
 defs(overloaded) OclAsType\<^sub>P\<^sub>e\<^sub>r\<^sub>s\<^sub>o\<^sub>n_Person : "(x::Person) .oclAsType(Person) \<equiv> x"
 defs(overloaded) OclAsType\<^sub>P\<^sub>e\<^sub>r\<^sub>s\<^sub>o\<^sub>n_Planet : "(x::Planet) .oclAsType(Person) \<equiv> (\<lambda>\<tau>. (case (x (\<tau>)) of \<bottom> \<Rightarrow> (invalid (\<tau>))
     | \<lfloor>\<bottom>\<rfloor> \<Rightarrow> (null (\<tau>))
@@ -260,7 +261,7 @@ defs(overloaded) OclAsType\<^sub>O\<^sub>c\<^sub>l\<^sub>A\<^sub>n\<^sub>y_Galax
     | \<lfloor>\<bottom>\<rfloor> \<Rightarrow> (null (\<tau>))
     | \<lfloor>\<lfloor>Galaxy\<rfloor>\<rfloor> \<Rightarrow> \<lfloor>\<lfloor>(mkoid\<^sub>O\<^sub>c\<^sub>l\<^sub>A\<^sub>n\<^sub>y ((mk\<^sub>O\<^sub>c\<^sub>l\<^sub>A\<^sub>n\<^sub>y_\<^sub>G\<^sub>a\<^sub>l\<^sub>a\<^sub>x\<^sub>y (Galaxy))))\<rfloor>\<rfloor>))"
 
-(* 33 ************************************ 71 + 4 *)
+(* 33 ************************************ 72 + 4 *)
 definition "OclAsType\<^sub>P\<^sub>e\<^sub>r\<^sub>s\<^sub>o\<^sub>n_\<AA> = (\<lambda> (in\<^sub>P\<^sub>e\<^sub>r\<^sub>s\<^sub>o\<^sub>n (Person)) \<Rightarrow> \<lfloor>Person\<rfloor>
     | (in\<^sub>P\<^sub>l\<^sub>a\<^sub>n\<^sub>e\<^sub>t ((mkoid\<^sub>P\<^sub>l\<^sub>a\<^sub>n\<^sub>e\<^sub>t ((mk\<^sub>P\<^sub>l\<^sub>a\<^sub>n\<^sub>e\<^sub>t_\<^sub>P\<^sub>e\<^sub>r\<^sub>s\<^sub>o\<^sub>n (Person))) (_) (_)))) \<Rightarrow> \<lfloor>Person\<rfloor>
     | (in\<^sub>G\<^sub>a\<^sub>l\<^sub>a\<^sub>x\<^sub>y ((mkoid\<^sub>G\<^sub>a\<^sub>l\<^sub>a\<^sub>x\<^sub>y ((mk\<^sub>G\<^sub>a\<^sub>l\<^sub>a\<^sub>x\<^sub>y_\<^sub>P\<^sub>e\<^sub>r\<^sub>s\<^sub>o\<^sub>n (Person))) (_) (_)))) \<Rightarrow> \<lfloor>Person\<rfloor>
@@ -281,16 +282,16 @@ definition "OclAsType\<^sub>O\<^sub>c\<^sub>l\<^sub>A\<^sub>n\<^sub>y_\<AA> = So
     | (in\<^sub>P\<^sub>l\<^sub>a\<^sub>n\<^sub>e\<^sub>t (Planet)) \<Rightarrow> (mkoid\<^sub>O\<^sub>c\<^sub>l\<^sub>A\<^sub>n\<^sub>y ((mk\<^sub>O\<^sub>c\<^sub>l\<^sub>A\<^sub>n\<^sub>y_\<^sub>P\<^sub>l\<^sub>a\<^sub>n\<^sub>e\<^sub>t (Planet))))
     | (in\<^sub>G\<^sub>a\<^sub>l\<^sub>a\<^sub>x\<^sub>y (Galaxy)) \<Rightarrow> (mkoid\<^sub>O\<^sub>c\<^sub>l\<^sub>A\<^sub>n\<^sub>y ((mk\<^sub>O\<^sub>c\<^sub>l\<^sub>A\<^sub>n\<^sub>y_\<^sub>G\<^sub>a\<^sub>l\<^sub>a\<^sub>x\<^sub>y (Galaxy)))))"
 
-(* 34 ************************************ 75 + 1 *)
-lemmas [simp,code_unfold] = OclAsType\<^sub>P\<^sub>e\<^sub>r\<^sub>s\<^sub>o\<^sub>n_Person
+(* 34 ************************************ 76 + 1 *)
+lemmas[simp,code_unfold] = OclAsType\<^sub>P\<^sub>e\<^sub>r\<^sub>s\<^sub>o\<^sub>n_Person
                             OclAsType\<^sub>P\<^sub>l\<^sub>a\<^sub>n\<^sub>e\<^sub>t_Planet
                             OclAsType\<^sub>G\<^sub>a\<^sub>l\<^sub>a\<^sub>x\<^sub>y_Galaxy
                             OclAsType\<^sub>O\<^sub>c\<^sub>l\<^sub>A\<^sub>n\<^sub>y_OclAny
 
-(* 35 ************************************ 76 + 1 *)
+(* 35 ************************************ 77 + 1 *)
 subsection{* Context Passing *}
 
-(* 36 ************************************ 77 + 64 *)
+(* 36 ************************************ 78 + 64 *)
 lemma cp_OclAsType\<^sub>O\<^sub>c\<^sub>l\<^sub>A\<^sub>n\<^sub>y_OclAny_OclAny : "(cp (p)) \<Longrightarrow> (cp ((\<lambda>x. (((p ((x::OclAny)))::OclAny) .oclAsType(OclAny)))))"
 by(rule cpI1, simp)
 lemma cp_OclAsType\<^sub>O\<^sub>c\<^sub>l\<^sub>A\<^sub>n\<^sub>y_Galaxy_OclAny : "(cp (p)) \<Longrightarrow> (cp ((\<lambda>x. (((p ((x::Galaxy)))::OclAny) .oclAsType(OclAny)))))"
@@ -420,8 +421,8 @@ by(rule cpI1, simp)
 lemma cp_OclAsType\<^sub>P\<^sub>e\<^sub>r\<^sub>s\<^sub>o\<^sub>n_Person_Person : "(cp (p)) \<Longrightarrow> (cp ((\<lambda>x. (((p ((x::Person)))::Person) .oclAsType(Person)))))"
 by(rule cpI1, simp)
 
-(* 37 ************************************ 141 + 1 *)
-lemmas [simp,code_unfold] = cp_OclAsType\<^sub>O\<^sub>c\<^sub>l\<^sub>A\<^sub>n\<^sub>y_OclAny_OclAny
+(* 37 ************************************ 142 + 1 *)
+lemmas[simp,code_unfold] = cp_OclAsType\<^sub>O\<^sub>c\<^sub>l\<^sub>A\<^sub>n\<^sub>y_OclAny_OclAny
                             cp_OclAsType\<^sub>O\<^sub>c\<^sub>l\<^sub>A\<^sub>n\<^sub>y_Galaxy_OclAny
                             cp_OclAsType\<^sub>O\<^sub>c\<^sub>l\<^sub>A\<^sub>n\<^sub>y_Planet_OclAny
                             cp_OclAsType\<^sub>O\<^sub>c\<^sub>l\<^sub>A\<^sub>n\<^sub>y_Person_OclAny
@@ -486,10 +487,10 @@ lemmas [simp,code_unfold] = cp_OclAsType\<^sub>O\<^sub>c\<^sub>l\<^sub>A\<^sub>n
                             cp_OclAsType\<^sub>P\<^sub>e\<^sub>r\<^sub>s\<^sub>o\<^sub>n_Planet_Person
                             cp_OclAsType\<^sub>P\<^sub>e\<^sub>r\<^sub>s\<^sub>o\<^sub>n_Person_Person
 
-(* 38 ************************************ 142 + 1 *)
+(* 38 ************************************ 143 + 1 *)
 subsection{* Execution with Invalid or Null as Argument *}
 
-(* 39 ************************************ 143 + 32 *)
+(* 39 ************************************ 144 + 32 *)
 lemma OclAsType\<^sub>O\<^sub>c\<^sub>l\<^sub>A\<^sub>n\<^sub>y_OclAny_invalid : "((invalid::OclAny) .oclAsType(OclAny)) = invalid"
 by(simp)
 lemma OclAsType\<^sub>O\<^sub>c\<^sub>l\<^sub>A\<^sub>n\<^sub>y_Galaxy_invalid : "((invalid::Galaxy) .oclAsType(OclAny)) = invalid"
@@ -555,8 +556,8 @@ by(rule ext, simp add: OclAsType\<^sub>P\<^sub>e\<^sub>r\<^sub>s\<^sub>o\<^sub>n
 lemma OclAsType\<^sub>P\<^sub>e\<^sub>r\<^sub>s\<^sub>o\<^sub>n_Person_null : "((null::Person) .oclAsType(Person)) = null"
 by(simp)
 
-(* 40 ************************************ 175 + 1 *)
-lemmas [simp,code_unfold] = OclAsType\<^sub>O\<^sub>c\<^sub>l\<^sub>A\<^sub>n\<^sub>y_OclAny_invalid
+(* 40 ************************************ 176 + 1 *)
+lemmas[simp,code_unfold] = OclAsType\<^sub>O\<^sub>c\<^sub>l\<^sub>A\<^sub>n\<^sub>y_OclAny_invalid
                             OclAsType\<^sub>O\<^sub>c\<^sub>l\<^sub>A\<^sub>n\<^sub>y_Galaxy_invalid
                             OclAsType\<^sub>O\<^sub>c\<^sub>l\<^sub>A\<^sub>n\<^sub>y_Planet_invalid
                             OclAsType\<^sub>O\<^sub>c\<^sub>l\<^sub>A\<^sub>n\<^sub>y_Person_invalid
@@ -589,10 +590,10 @@ lemmas [simp,code_unfold] = OclAsType\<^sub>O\<^sub>c\<^sub>l\<^sub>A\<^sub>n\<^
                             OclAsType\<^sub>P\<^sub>e\<^sub>r\<^sub>s\<^sub>o\<^sub>n_Planet_null
                             OclAsType\<^sub>P\<^sub>e\<^sub>r\<^sub>s\<^sub>o\<^sub>n_Person_null
 
-(* 41 ************************************ 176 + 1 *)
+(* 41 ************************************ 177 + 1 *)
 subsection{* Validity and Definedness Properties *}
 
-(* 42 ************************************ 177 + 6 *)
+(* 42 ************************************ 178 + 6 *)
 lemma OclAsType\<^sub>P\<^sub>l\<^sub>a\<^sub>n\<^sub>e\<^sub>t_Person_defined : 
 assumes isdef: "\<tau> \<Turnstile> (\<delta> (X))"
 shows "\<tau> \<Turnstile> (\<delta> ((X::Person) .oclAsType(Planet)))"
@@ -624,10 +625,10 @@ shows "\<tau> \<Turnstile> (\<delta> ((X::Galaxy) .oclAsType(OclAny)))"
   using isdef
 by(auto simp: OclAsType\<^sub>O\<^sub>c\<^sub>l\<^sub>A\<^sub>n\<^sub>y_Galaxy foundation16 null_option_def bot_option_def) 
 
-(* 43 ************************************ 183 + 1 *)
+(* 43 ************************************ 184 + 1 *)
 subsection{* Up Down Casting *}
 
-(* 44 ************************************ 184 + 6 *)
+(* 44 ************************************ 185 + 6 *)
 lemma up\<^sub>P\<^sub>l\<^sub>a\<^sub>n\<^sub>e\<^sub>t_down\<^sub>P\<^sub>e\<^sub>r\<^sub>s\<^sub>o\<^sub>n_cast0 : 
 assumes isdef: "\<tau> \<Turnstile> (\<delta> (X))"
 shows "\<tau> \<Turnstile> (((X::Person) .oclAsType(Planet)) .oclAsType(Person)) \<triangleq> X"
@@ -659,7 +660,7 @@ shows "\<tau> \<Turnstile> (((X::Galaxy) .oclAsType(OclAny)) .oclAsType(Galaxy))
   using isdef
 by(auto simp: OclAsType\<^sub>O\<^sub>c\<^sub>l\<^sub>A\<^sub>n\<^sub>y_Galaxy OclAsType\<^sub>G\<^sub>a\<^sub>l\<^sub>a\<^sub>x\<^sub>y_OclAny foundation22 foundation16 null_option_def bot_option_def split: type\<^sub>G\<^sub>a\<^sub>l\<^sub>a\<^sub>x\<^sub>y.split typeoid\<^sub>G\<^sub>a\<^sub>l\<^sub>a\<^sub>x\<^sub>y.split) 
 
-(* 45 ************************************ 190 + 6 *)
+(* 45 ************************************ 191 + 6 *)
 lemma up\<^sub>P\<^sub>l\<^sub>a\<^sub>n\<^sub>e\<^sub>t_down\<^sub>P\<^sub>e\<^sub>r\<^sub>s\<^sub>o\<^sub>n_cast : 
 shows "(((X::Person) .oclAsType(Planet)) .oclAsType(Person)) = X"
   apply(rule ext, rename_tac \<tau>)
@@ -709,19 +710,51 @@ shows "(((X::Galaxy) .oclAsType(OclAny)) .oclAsType(Galaxy)) = X"
   apply((erule StrongEq_L_subst2_rev, simp, simp)+)
 done 
 
-(* 46 ************************************ 196 + 1 *)
+(* 46 ************************************ 197 + 6 *)
+lemma down\<^sub>P\<^sub>e\<^sub>r\<^sub>s\<^sub>o\<^sub>n_up\<^sub>P\<^sub>l\<^sub>a\<^sub>n\<^sub>e\<^sub>t_cast : 
+assumes def_X: "X = ((Y::Person) .oclAsType(Planet))"
+shows "(\<tau> \<Turnstile> ((not ((\<upsilon> (X)))) or ((X .oclAsType(Person)) .oclAsType(Planet)) \<doteq> X))"
+  apply(case_tac "(\<tau> \<Turnstile> ((not ((\<upsilon> (X))))))", rule foundation25, simp)
+by(rule foundation25', simp add: def_X up\<^sub>P\<^sub>l\<^sub>a\<^sub>n\<^sub>e\<^sub>t_down\<^sub>P\<^sub>e\<^sub>r\<^sub>s\<^sub>o\<^sub>n_cast StrictRefEq\<^sub>O\<^sub>b\<^sub>j\<^sub>e\<^sub>c\<^sub>t_sym) 
+lemma down\<^sub>P\<^sub>e\<^sub>r\<^sub>s\<^sub>o\<^sub>n_up\<^sub>G\<^sub>a\<^sub>l\<^sub>a\<^sub>x\<^sub>y_cast : 
+assumes def_X: "X = ((Y::Person) .oclAsType(Galaxy))"
+shows "(\<tau> \<Turnstile> ((not ((\<upsilon> (X)))) or ((X .oclAsType(Person)) .oclAsType(Galaxy)) \<doteq> X))"
+  apply(case_tac "(\<tau> \<Turnstile> ((not ((\<upsilon> (X))))))", rule foundation25, simp)
+by(rule foundation25', simp add: def_X up\<^sub>G\<^sub>a\<^sub>l\<^sub>a\<^sub>x\<^sub>y_down\<^sub>P\<^sub>e\<^sub>r\<^sub>s\<^sub>o\<^sub>n_cast StrictRefEq\<^sub>O\<^sub>b\<^sub>j\<^sub>e\<^sub>c\<^sub>t_sym) 
+lemma down\<^sub>P\<^sub>e\<^sub>r\<^sub>s\<^sub>o\<^sub>n_up\<^sub>O\<^sub>c\<^sub>l\<^sub>A\<^sub>n\<^sub>y_cast : 
+assumes def_X: "X = ((Y::Person) .oclAsType(OclAny))"
+shows "(\<tau> \<Turnstile> ((not ((\<upsilon> (X)))) or ((X .oclAsType(Person)) .oclAsType(OclAny)) \<doteq> X))"
+  apply(case_tac "(\<tau> \<Turnstile> ((not ((\<upsilon> (X))))))", rule foundation25, simp)
+by(rule foundation25', simp add: def_X up\<^sub>O\<^sub>c\<^sub>l\<^sub>A\<^sub>n\<^sub>y_down\<^sub>P\<^sub>e\<^sub>r\<^sub>s\<^sub>o\<^sub>n_cast StrictRefEq\<^sub>O\<^sub>b\<^sub>j\<^sub>e\<^sub>c\<^sub>t_sym) 
+lemma down\<^sub>P\<^sub>l\<^sub>a\<^sub>n\<^sub>e\<^sub>t_up\<^sub>G\<^sub>a\<^sub>l\<^sub>a\<^sub>x\<^sub>y_cast : 
+assumes def_X: "X = ((Y::Planet) .oclAsType(Galaxy))"
+shows "(\<tau> \<Turnstile> ((not ((\<upsilon> (X)))) or ((X .oclAsType(Planet)) .oclAsType(Galaxy)) \<doteq> X))"
+  apply(case_tac "(\<tau> \<Turnstile> ((not ((\<upsilon> (X))))))", rule foundation25, simp)
+by(rule foundation25', simp add: def_X up\<^sub>G\<^sub>a\<^sub>l\<^sub>a\<^sub>x\<^sub>y_down\<^sub>P\<^sub>l\<^sub>a\<^sub>n\<^sub>e\<^sub>t_cast StrictRefEq\<^sub>O\<^sub>b\<^sub>j\<^sub>e\<^sub>c\<^sub>t_sym) 
+lemma down\<^sub>P\<^sub>l\<^sub>a\<^sub>n\<^sub>e\<^sub>t_up\<^sub>O\<^sub>c\<^sub>l\<^sub>A\<^sub>n\<^sub>y_cast : 
+assumes def_X: "X = ((Y::Planet) .oclAsType(OclAny))"
+shows "(\<tau> \<Turnstile> ((not ((\<upsilon> (X)))) or ((X .oclAsType(Planet)) .oclAsType(OclAny)) \<doteq> X))"
+  apply(case_tac "(\<tau> \<Turnstile> ((not ((\<upsilon> (X))))))", rule foundation25, simp)
+by(rule foundation25', simp add: def_X up\<^sub>O\<^sub>c\<^sub>l\<^sub>A\<^sub>n\<^sub>y_down\<^sub>P\<^sub>l\<^sub>a\<^sub>n\<^sub>e\<^sub>t_cast StrictRefEq\<^sub>O\<^sub>b\<^sub>j\<^sub>e\<^sub>c\<^sub>t_sym) 
+lemma down\<^sub>G\<^sub>a\<^sub>l\<^sub>a\<^sub>x\<^sub>y_up\<^sub>O\<^sub>c\<^sub>l\<^sub>A\<^sub>n\<^sub>y_cast : 
+assumes def_X: "X = ((Y::Galaxy) .oclAsType(OclAny))"
+shows "(\<tau> \<Turnstile> ((not ((\<upsilon> (X)))) or ((X .oclAsType(Galaxy)) .oclAsType(OclAny)) \<doteq> X))"
+  apply(case_tac "(\<tau> \<Turnstile> ((not ((\<upsilon> (X))))))", rule foundation25, simp)
+by(rule foundation25', simp add: def_X up\<^sub>O\<^sub>c\<^sub>l\<^sub>A\<^sub>n\<^sub>y_down\<^sub>G\<^sub>a\<^sub>l\<^sub>a\<^sub>x\<^sub>y_cast StrictRefEq\<^sub>O\<^sub>b\<^sub>j\<^sub>e\<^sub>c\<^sub>t_sym) 
+
+(* 47 ************************************ 203 + 1 *)
 section{* OclIsTypeOf *}
 
-(* 47 ************************************ 197 + 1 *)
+(* 48 ************************************ 204 + 1 *)
 subsection{* Definition *}
 
-(* 48 ************************************ 198 + 4 *)
+(* 49 ************************************ 205 + 4 *)
 consts OclIsTypeOf\<^sub>P\<^sub>e\<^sub>r\<^sub>s\<^sub>o\<^sub>n :: "'\<alpha> \<Rightarrow> Boolean" ("(_) .oclIsTypeOf'(Person')")
 consts OclIsTypeOf\<^sub>P\<^sub>l\<^sub>a\<^sub>n\<^sub>e\<^sub>t :: "'\<alpha> \<Rightarrow> Boolean" ("(_) .oclIsTypeOf'(Planet')")
 consts OclIsTypeOf\<^sub>G\<^sub>a\<^sub>l\<^sub>a\<^sub>x\<^sub>y :: "'\<alpha> \<Rightarrow> Boolean" ("(_) .oclIsTypeOf'(Galaxy')")
 consts OclIsTypeOf\<^sub>O\<^sub>c\<^sub>l\<^sub>A\<^sub>n\<^sub>y :: "'\<alpha> \<Rightarrow> Boolean" ("(_) .oclIsTypeOf'(OclAny')")
 
-(* 49 ************************************ 202 + 16 *)
+(* 50 ************************************ 209 + 16 *)
 defs(overloaded) OclIsTypeOf\<^sub>P\<^sub>e\<^sub>r\<^sub>s\<^sub>o\<^sub>n_Person : "(x::Person) .oclIsTypeOf(Person) \<equiv> (\<lambda>\<tau>. (case (x (\<tau>)) of \<bottom> \<Rightarrow> (invalid (\<tau>))
     | \<lfloor>\<bottom>\<rfloor> \<Rightarrow> (true (\<tau>))
     | \<lfloor>\<lfloor>(mkoid\<^sub>P\<^sub>e\<^sub>r\<^sub>s\<^sub>o\<^sub>n ((mk\<^sub>P\<^sub>e\<^sub>r\<^sub>s\<^sub>o\<^sub>n (_) (_) (_) (_) (_))) (_) (_))\<rfloor>\<rfloor> \<Rightarrow> (true (\<tau>))))"
@@ -780,7 +813,7 @@ defs(overloaded) OclIsTypeOf\<^sub>O\<^sub>c\<^sub>l\<^sub>A\<^sub>n\<^sub>y_Gal
     | \<lfloor>\<bottom>\<rfloor> \<Rightarrow> (true (\<tau>))
     | _ \<Rightarrow> (false (\<tau>))))"
 
-(* 50 ************************************ 218 + 4 *)
+(* 51 ************************************ 225 + 4 *)
 definition "OclIsTypeOf\<^sub>P\<^sub>e\<^sub>r\<^sub>s\<^sub>o\<^sub>n_\<AA> = (\<lambda> (in\<^sub>P\<^sub>e\<^sub>r\<^sub>s\<^sub>o\<^sub>n (Person)) \<Rightarrow> (((((\<lambda>x _. \<lfloor>\<lfloor>x\<rfloor>\<rfloor>)) (Person))::Person) .oclIsTypeOf(Person))
     | (in\<^sub>P\<^sub>l\<^sub>a\<^sub>n\<^sub>e\<^sub>t (Planet)) \<Rightarrow> (((((\<lambda>x _. \<lfloor>\<lfloor>x\<rfloor>\<rfloor>)) (Planet))::Planet) .oclIsTypeOf(Person))
     | (in\<^sub>G\<^sub>a\<^sub>l\<^sub>a\<^sub>x\<^sub>y (Galaxy)) \<Rightarrow> (((((\<lambda>x _. \<lfloor>\<lfloor>x\<rfloor>\<rfloor>)) (Galaxy))::Galaxy) .oclIsTypeOf(Person))
@@ -798,16 +831,16 @@ definition "OclIsTypeOf\<^sub>O\<^sub>c\<^sub>l\<^sub>A\<^sub>n\<^sub>y_\<AA> = 
     | (in\<^sub>P\<^sub>l\<^sub>a\<^sub>n\<^sub>e\<^sub>t (Planet)) \<Rightarrow> (((((\<lambda>x _. \<lfloor>\<lfloor>x\<rfloor>\<rfloor>)) (Planet))::Planet) .oclIsTypeOf(OclAny))
     | (in\<^sub>G\<^sub>a\<^sub>l\<^sub>a\<^sub>x\<^sub>y (Galaxy)) \<Rightarrow> (((((\<lambda>x _. \<lfloor>\<lfloor>x\<rfloor>\<rfloor>)) (Galaxy))::Galaxy) .oclIsTypeOf(OclAny)))"
 
-(* 51 ************************************ 222 + 1 *)
-lemmas [simp,code_unfold] = OclIsTypeOf\<^sub>P\<^sub>e\<^sub>r\<^sub>s\<^sub>o\<^sub>n_Person
+(* 52 ************************************ 229 + 1 *)
+lemmas[simp,code_unfold] = OclIsTypeOf\<^sub>P\<^sub>e\<^sub>r\<^sub>s\<^sub>o\<^sub>n_Person
                             OclIsTypeOf\<^sub>P\<^sub>l\<^sub>a\<^sub>n\<^sub>e\<^sub>t_Planet
                             OclIsTypeOf\<^sub>G\<^sub>a\<^sub>l\<^sub>a\<^sub>x\<^sub>y_Galaxy
                             OclIsTypeOf\<^sub>O\<^sub>c\<^sub>l\<^sub>A\<^sub>n\<^sub>y_OclAny
 
-(* 52 ************************************ 223 + 1 *)
+(* 53 ************************************ 230 + 1 *)
 subsection{* Context Passing *}
 
-(* 53 ************************************ 224 + 64 *)
+(* 54 ************************************ 231 + 64 *)
 lemma cp_OclIsTypeOf\<^sub>O\<^sub>c\<^sub>l\<^sub>A\<^sub>n\<^sub>y_OclAny_OclAny : "(cp (p)) \<Longrightarrow> (cp ((\<lambda>x. (((p ((x::OclAny)))::OclAny) .oclIsTypeOf(OclAny)))))"
 by(rule cpI1, simp)
 lemma cp_OclIsTypeOf\<^sub>O\<^sub>c\<^sub>l\<^sub>A\<^sub>n\<^sub>y_Galaxy_OclAny : "(cp (p)) \<Longrightarrow> (cp ((\<lambda>x. (((p ((x::Galaxy)))::OclAny) .oclIsTypeOf(OclAny)))))"
@@ -937,8 +970,8 @@ by(rule cpI1, simp)
 lemma cp_OclIsTypeOf\<^sub>P\<^sub>e\<^sub>r\<^sub>s\<^sub>o\<^sub>n_Person_Person : "(cp (p)) \<Longrightarrow> (cp ((\<lambda>x. (((p ((x::Person)))::Person) .oclIsTypeOf(Person)))))"
 by(rule cpI1, simp)
 
-(* 54 ************************************ 288 + 1 *)
-lemmas [simp,code_unfold] = cp_OclIsTypeOf\<^sub>O\<^sub>c\<^sub>l\<^sub>A\<^sub>n\<^sub>y_OclAny_OclAny
+(* 55 ************************************ 295 + 1 *)
+lemmas[simp,code_unfold] = cp_OclIsTypeOf\<^sub>O\<^sub>c\<^sub>l\<^sub>A\<^sub>n\<^sub>y_OclAny_OclAny
                             cp_OclIsTypeOf\<^sub>O\<^sub>c\<^sub>l\<^sub>A\<^sub>n\<^sub>y_Galaxy_OclAny
                             cp_OclIsTypeOf\<^sub>O\<^sub>c\<^sub>l\<^sub>A\<^sub>n\<^sub>y_Planet_OclAny
                             cp_OclIsTypeOf\<^sub>O\<^sub>c\<^sub>l\<^sub>A\<^sub>n\<^sub>y_Person_OclAny
@@ -1003,10 +1036,10 @@ lemmas [simp,code_unfold] = cp_OclIsTypeOf\<^sub>O\<^sub>c\<^sub>l\<^sub>A\<^sub
                             cp_OclIsTypeOf\<^sub>P\<^sub>e\<^sub>r\<^sub>s\<^sub>o\<^sub>n_Planet_Person
                             cp_OclIsTypeOf\<^sub>P\<^sub>e\<^sub>r\<^sub>s\<^sub>o\<^sub>n_Person_Person
 
-(* 55 ************************************ 289 + 1 *)
+(* 56 ************************************ 296 + 1 *)
 subsection{* Execution with Invalid or Null as Argument *}
 
-(* 56 ************************************ 290 + 32 *)
+(* 57 ************************************ 297 + 32 *)
 lemma OclIsTypeOf\<^sub>O\<^sub>c\<^sub>l\<^sub>A\<^sub>n\<^sub>y_OclAny_invalid : "((invalid::OclAny) .oclIsTypeOf(OclAny)) = invalid"
 by(rule ext, simp add: bot_option_def invalid_def)
 lemma OclIsTypeOf\<^sub>O\<^sub>c\<^sub>l\<^sub>A\<^sub>n\<^sub>y_Galaxy_invalid : "((invalid::Galaxy) .oclIsTypeOf(OclAny)) = invalid"
@@ -1072,8 +1105,8 @@ by(rule ext, simp add: OclIsTypeOf\<^sub>P\<^sub>e\<^sub>r\<^sub>s\<^sub>o\<^sub
 lemma OclIsTypeOf\<^sub>P\<^sub>e\<^sub>r\<^sub>s\<^sub>o\<^sub>n_Person_null : "((null::Person) .oclIsTypeOf(Person)) = true"
 by(rule ext, simp add: bot_option_def null_fun_def null_option_def)
 
-(* 57 ************************************ 322 + 1 *)
-lemmas [simp,code_unfold] = OclIsTypeOf\<^sub>O\<^sub>c\<^sub>l\<^sub>A\<^sub>n\<^sub>y_OclAny_invalid
+(* 58 ************************************ 329 + 1 *)
+lemmas[simp,code_unfold] = OclIsTypeOf\<^sub>O\<^sub>c\<^sub>l\<^sub>A\<^sub>n\<^sub>y_OclAny_invalid
                             OclIsTypeOf\<^sub>O\<^sub>c\<^sub>l\<^sub>A\<^sub>n\<^sub>y_Galaxy_invalid
                             OclIsTypeOf\<^sub>O\<^sub>c\<^sub>l\<^sub>A\<^sub>n\<^sub>y_Planet_invalid
                             OclIsTypeOf\<^sub>O\<^sub>c\<^sub>l\<^sub>A\<^sub>n\<^sub>y_Person_invalid
@@ -1106,10 +1139,10 @@ lemmas [simp,code_unfold] = OclIsTypeOf\<^sub>O\<^sub>c\<^sub>l\<^sub>A\<^sub>n\
                             OclIsTypeOf\<^sub>P\<^sub>e\<^sub>r\<^sub>s\<^sub>o\<^sub>n_Planet_null
                             OclIsTypeOf\<^sub>P\<^sub>e\<^sub>r\<^sub>s\<^sub>o\<^sub>n_Person_null
 
-(* 58 ************************************ 323 + 1 *)
+(* 59 ************************************ 330 + 1 *)
 subsection{* Validity and Definedness Properties *}
 
-(* 59 ************************************ 324 + 16 *)
+(* 60 ************************************ 331 + 16 *)
 lemma OclIsTypeOf\<^sub>P\<^sub>e\<^sub>r\<^sub>s\<^sub>o\<^sub>n_Person_defined : 
 assumes isdef: "\<tau> \<Turnstile> (\<upsilon> (X))"
 shows "\<tau> \<Turnstile> (\<delta> ((X::Person) .oclIsTypeOf(Person)))"
@@ -1191,7 +1224,7 @@ shows "\<tau> \<Turnstile> (\<delta> ((X::Galaxy) .oclIsTypeOf(OclAny)))"
   apply(insert isdef[simplified foundation18'], simp only: OclValid_def, subst cp_defined)
 by(auto simp: cp_defined[symmetric ] bot_option_def OclIsTypeOf\<^sub>O\<^sub>c\<^sub>l\<^sub>A\<^sub>n\<^sub>y_Galaxy split: option.split type\<^sub>G\<^sub>a\<^sub>l\<^sub>a\<^sub>x\<^sub>y.split typeoid\<^sub>G\<^sub>a\<^sub>l\<^sub>a\<^sub>x\<^sub>y.split) 
 
-(* 60 ************************************ 340 + 16 *)
+(* 61 ************************************ 347 + 16 *)
 lemma OclIsTypeOf\<^sub>P\<^sub>e\<^sub>r\<^sub>s\<^sub>o\<^sub>n_Person_defined' : 
 assumes isdef: "\<tau> \<Turnstile> (\<delta> (X))"
 shows "\<tau> \<Turnstile> (\<delta> ((X::Person) .oclIsTypeOf(Person)))"
@@ -1257,10 +1290,10 @@ assumes isdef: "\<tau> \<Turnstile> (\<delta> (X))"
 shows "\<tau> \<Turnstile> (\<delta> ((X::Galaxy) .oclIsTypeOf(OclAny)))"
 by(rule OclIsTypeOf\<^sub>O\<^sub>c\<^sub>l\<^sub>A\<^sub>n\<^sub>y_Galaxy_defined[OF isdef[THEN foundation20]]) 
 
-(* 61 ************************************ 356 + 1 *)
+(* 62 ************************************ 363 + 1 *)
 subsection{* Up Down Casting *}
 
-(* 62 ************************************ 357 + 6 *)
+(* 63 ************************************ 364 + 6 *)
 lemma actualType\<^sub>P\<^sub>e\<^sub>r\<^sub>s\<^sub>o\<^sub>n_larger_staticType\<^sub>P\<^sub>l\<^sub>a\<^sub>n\<^sub>e\<^sub>t : 
 assumes isdef: "\<tau> \<Turnstile> (\<delta> (X))"
 shows "\<tau> \<Turnstile> ((X::Person) .oclIsTypeOf(Planet)) \<triangleq> false"
@@ -1292,7 +1325,7 @@ shows "\<tau> \<Turnstile> ((X::Galaxy) .oclIsTypeOf(OclAny)) \<triangleq> false
   using isdef
 by(auto simp: OclIsTypeOf\<^sub>O\<^sub>c\<^sub>l\<^sub>A\<^sub>n\<^sub>y_Galaxy foundation22 foundation16 null_option_def bot_option_def) 
 
-(* 63 ************************************ 363 + 10 *)
+(* 64 ************************************ 370 + 10 *)
 lemma down_cast_type\<^sub>P\<^sub>l\<^sub>a\<^sub>n\<^sub>e\<^sub>t_from_Planet_to_Person : 
 assumes istyp: "\<tau> \<Turnstile> ((X::Planet) .oclIsTypeOf(Planet))"
 assumes isdef: "\<tau> \<Turnstile> (\<delta> (X))"
@@ -1364,19 +1397,19 @@ shows "\<tau> \<Turnstile> (X .oclAsType(Galaxy)) \<triangleq> invalid"
   apply(auto simp: OclAsType\<^sub>G\<^sub>a\<^sub>l\<^sub>a\<^sub>x\<^sub>y_OclAny foundation22 foundation16 null_option_def bot_option_def split: type\<^sub>O\<^sub>c\<^sub>l\<^sub>A\<^sub>n\<^sub>y.split typeoid\<^sub>O\<^sub>c\<^sub>l\<^sub>A\<^sub>n\<^sub>y.split)
 by(simp add: OclValid_def false_def true_def) 
 
-(* 64 ************************************ 373 + 1 *)
+(* 65 ************************************ 380 + 1 *)
 section{* OclIsKindOf *}
 
-(* 65 ************************************ 374 + 1 *)
+(* 66 ************************************ 381 + 1 *)
 subsection{* Definition *}
 
-(* 66 ************************************ 375 + 4 *)
+(* 67 ************************************ 382 + 4 *)
 consts OclIsKindOf\<^sub>P\<^sub>e\<^sub>r\<^sub>s\<^sub>o\<^sub>n :: "'\<alpha> \<Rightarrow> Boolean" ("(_) .oclIsKindOf'(Person')")
 consts OclIsKindOf\<^sub>P\<^sub>l\<^sub>a\<^sub>n\<^sub>e\<^sub>t :: "'\<alpha> \<Rightarrow> Boolean" ("(_) .oclIsKindOf'(Planet')")
 consts OclIsKindOf\<^sub>G\<^sub>a\<^sub>l\<^sub>a\<^sub>x\<^sub>y :: "'\<alpha> \<Rightarrow> Boolean" ("(_) .oclIsKindOf'(Galaxy')")
 consts OclIsKindOf\<^sub>O\<^sub>c\<^sub>l\<^sub>A\<^sub>n\<^sub>y :: "'\<alpha> \<Rightarrow> Boolean" ("(_) .oclIsKindOf'(OclAny')")
 
-(* 67 ************************************ 379 + 16 *)
+(* 68 ************************************ 386 + 16 *)
 defs(overloaded) OclIsKindOf\<^sub>P\<^sub>e\<^sub>r\<^sub>s\<^sub>o\<^sub>n_Person : "(x::Person) .oclIsKindOf(Person) \<equiv> (x .oclIsTypeOf(Person))"
 defs(overloaded) OclIsKindOf\<^sub>P\<^sub>e\<^sub>r\<^sub>s\<^sub>o\<^sub>n_Planet : "(x::Planet) .oclIsKindOf(Person) \<equiv> (x .oclIsTypeOf(Person))"
 defs(overloaded) OclIsKindOf\<^sub>P\<^sub>e\<^sub>r\<^sub>s\<^sub>o\<^sub>n_Galaxy : "(x::Galaxy) .oclIsKindOf(Person) \<equiv> (x .oclIsTypeOf(Person))"
@@ -1394,7 +1427,7 @@ defs(overloaded) OclIsKindOf\<^sub>O\<^sub>c\<^sub>l\<^sub>A\<^sub>n\<^sub>y_Per
 defs(overloaded) OclIsKindOf\<^sub>O\<^sub>c\<^sub>l\<^sub>A\<^sub>n\<^sub>y_Planet : "(x::Planet) .oclIsKindOf(OclAny) \<equiv> (x .oclIsTypeOf(OclAny)) or (x .oclIsKindOf(Galaxy))"
 defs(overloaded) OclIsKindOf\<^sub>O\<^sub>c\<^sub>l\<^sub>A\<^sub>n\<^sub>y_Galaxy : "(x::Galaxy) .oclIsKindOf(OclAny) \<equiv> (x .oclIsTypeOf(OclAny)) or (x .oclIsKindOf(Galaxy))"
 
-(* 68 ************************************ 395 + 4 *)
+(* 69 ************************************ 402 + 4 *)
 definition "OclIsKindOf\<^sub>P\<^sub>e\<^sub>r\<^sub>s\<^sub>o\<^sub>n_\<AA> = (\<lambda> (in\<^sub>P\<^sub>e\<^sub>r\<^sub>s\<^sub>o\<^sub>n (Person)) \<Rightarrow> (((((\<lambda>x _. \<lfloor>\<lfloor>x\<rfloor>\<rfloor>)) (Person))::Person) .oclIsKindOf(Person))
     | (in\<^sub>P\<^sub>l\<^sub>a\<^sub>n\<^sub>e\<^sub>t (Planet)) \<Rightarrow> (((((\<lambda>x _. \<lfloor>\<lfloor>x\<rfloor>\<rfloor>)) (Planet))::Planet) .oclIsKindOf(Person))
     | (in\<^sub>G\<^sub>a\<^sub>l\<^sub>a\<^sub>x\<^sub>y (Galaxy)) \<Rightarrow> (((((\<lambda>x _. \<lfloor>\<lfloor>x\<rfloor>\<rfloor>)) (Galaxy))::Galaxy) .oclIsKindOf(Person))
@@ -1412,16 +1445,16 @@ definition "OclIsKindOf\<^sub>O\<^sub>c\<^sub>l\<^sub>A\<^sub>n\<^sub>y_\<AA> = 
     | (in\<^sub>P\<^sub>l\<^sub>a\<^sub>n\<^sub>e\<^sub>t (Planet)) \<Rightarrow> (((((\<lambda>x _. \<lfloor>\<lfloor>x\<rfloor>\<rfloor>)) (Planet))::Planet) .oclIsKindOf(OclAny))
     | (in\<^sub>G\<^sub>a\<^sub>l\<^sub>a\<^sub>x\<^sub>y (Galaxy)) \<Rightarrow> (((((\<lambda>x _. \<lfloor>\<lfloor>x\<rfloor>\<rfloor>)) (Galaxy))::Galaxy) .oclIsKindOf(OclAny)))"
 
-(* 69 ************************************ 399 + 1 *)
-lemmas [simp,code_unfold] = OclIsKindOf\<^sub>P\<^sub>e\<^sub>r\<^sub>s\<^sub>o\<^sub>n_Person
+(* 70 ************************************ 406 + 1 *)
+lemmas[simp,code_unfold] = OclIsKindOf\<^sub>P\<^sub>e\<^sub>r\<^sub>s\<^sub>o\<^sub>n_Person
                             OclIsKindOf\<^sub>P\<^sub>l\<^sub>a\<^sub>n\<^sub>e\<^sub>t_Planet
                             OclIsKindOf\<^sub>G\<^sub>a\<^sub>l\<^sub>a\<^sub>x\<^sub>y_Galaxy
                             OclIsKindOf\<^sub>O\<^sub>c\<^sub>l\<^sub>A\<^sub>n\<^sub>y_OclAny
 
-(* 70 ************************************ 400 + 1 *)
+(* 71 ************************************ 407 + 1 *)
 subsection{* Context Passing *}
 
-(* 71 ************************************ 401 + 64 *)
+(* 72 ************************************ 408 + 64 *)
 lemma cp_OclIsKindOf\<^sub>P\<^sub>e\<^sub>r\<^sub>s\<^sub>o\<^sub>n_Person_Person : "(cp (p)) \<Longrightarrow> (cp ((\<lambda>x. (((p ((x::Person)))::Person) .oclIsKindOf(Person)))))"
 by(simp only: OclIsKindOf\<^sub>P\<^sub>e\<^sub>r\<^sub>s\<^sub>o\<^sub>n_Person, simp only: cp_OclIsTypeOf\<^sub>P\<^sub>e\<^sub>r\<^sub>s\<^sub>o\<^sub>n_Person_Person)
 lemma cp_OclIsKindOf\<^sub>P\<^sub>e\<^sub>r\<^sub>s\<^sub>o\<^sub>n_Planet_Person : "(cp (p)) \<Longrightarrow> (cp ((\<lambda>x. (((p ((x::Planet)))::Person) .oclIsKindOf(Person)))))"
@@ -1695,8 +1728,8 @@ lemma cp_OclIsKindOf\<^sub>O\<^sub>c\<^sub>l\<^sub>A\<^sub>n\<^sub>y_Galaxy_Gala
   apply(simp only: cp_OclIsTypeOf\<^sub>O\<^sub>c\<^sub>l\<^sub>A\<^sub>n\<^sub>y_Galaxy_Galaxy)
 by(simp only: cp_OclIsKindOf\<^sub>G\<^sub>a\<^sub>l\<^sub>a\<^sub>x\<^sub>y_Galaxy_Galaxy)
 
-(* 72 ************************************ 465 + 1 *)
-lemmas [simp,code_unfold] = cp_OclIsKindOf\<^sub>O\<^sub>c\<^sub>l\<^sub>A\<^sub>n\<^sub>y_OclAny_OclAny
+(* 73 ************************************ 472 + 1 *)
+lemmas[simp,code_unfold] = cp_OclIsKindOf\<^sub>O\<^sub>c\<^sub>l\<^sub>A\<^sub>n\<^sub>y_OclAny_OclAny
                             cp_OclIsKindOf\<^sub>O\<^sub>c\<^sub>l\<^sub>A\<^sub>n\<^sub>y_Galaxy_OclAny
                             cp_OclIsKindOf\<^sub>O\<^sub>c\<^sub>l\<^sub>A\<^sub>n\<^sub>y_Planet_OclAny
                             cp_OclIsKindOf\<^sub>O\<^sub>c\<^sub>l\<^sub>A\<^sub>n\<^sub>y_Person_OclAny
@@ -1761,10 +1794,10 @@ lemmas [simp,code_unfold] = cp_OclIsKindOf\<^sub>O\<^sub>c\<^sub>l\<^sub>A\<^sub
                             cp_OclIsKindOf\<^sub>P\<^sub>e\<^sub>r\<^sub>s\<^sub>o\<^sub>n_Planet_Person
                             cp_OclIsKindOf\<^sub>P\<^sub>e\<^sub>r\<^sub>s\<^sub>o\<^sub>n_Person_Person
 
-(* 73 ************************************ 466 + 1 *)
+(* 74 ************************************ 473 + 1 *)
 subsection{* Execution with Invalid or Null as Argument *}
 
-(* 74 ************************************ 467 + 32 *)
+(* 75 ************************************ 474 + 32 *)
 lemma OclIsKindOf\<^sub>P\<^sub>e\<^sub>r\<^sub>s\<^sub>o\<^sub>n_Person_invalid : "((invalid::Person) .oclIsKindOf(Person)) = invalid"
 by(simp only: OclIsKindOf\<^sub>P\<^sub>e\<^sub>r\<^sub>s\<^sub>o\<^sub>n_Person OclIsTypeOf\<^sub>P\<^sub>e\<^sub>r\<^sub>s\<^sub>o\<^sub>n_Person_invalid)
 lemma OclIsKindOf\<^sub>P\<^sub>e\<^sub>r\<^sub>s\<^sub>o\<^sub>n_Person_null : "((null::Person) .oclIsKindOf(Person)) = true"
@@ -1830,8 +1863,8 @@ by(simp only: OclIsKindOf\<^sub>O\<^sub>c\<^sub>l\<^sub>A\<^sub>n\<^sub>y_Galaxy
 lemma OclIsKindOf\<^sub>O\<^sub>c\<^sub>l\<^sub>A\<^sub>n\<^sub>y_Galaxy_null : "((null::Galaxy) .oclIsKindOf(OclAny)) = true"
 by(simp only: OclIsKindOf\<^sub>O\<^sub>c\<^sub>l\<^sub>A\<^sub>n\<^sub>y_Galaxy OclIsTypeOf\<^sub>O\<^sub>c\<^sub>l\<^sub>A\<^sub>n\<^sub>y_Galaxy_null OclIsKindOf\<^sub>G\<^sub>a\<^sub>l\<^sub>a\<^sub>x\<^sub>y_Galaxy_null, simp)
 
-(* 75 ************************************ 499 + 1 *)
-lemmas [simp,code_unfold] = OclIsKindOf\<^sub>O\<^sub>c\<^sub>l\<^sub>A\<^sub>n\<^sub>y_OclAny_invalid
+(* 76 ************************************ 506 + 1 *)
+lemmas[simp,code_unfold] = OclIsKindOf\<^sub>O\<^sub>c\<^sub>l\<^sub>A\<^sub>n\<^sub>y_OclAny_invalid
                             OclIsKindOf\<^sub>O\<^sub>c\<^sub>l\<^sub>A\<^sub>n\<^sub>y_Galaxy_invalid
                             OclIsKindOf\<^sub>O\<^sub>c\<^sub>l\<^sub>A\<^sub>n\<^sub>y_Planet_invalid
                             OclIsKindOf\<^sub>O\<^sub>c\<^sub>l\<^sub>A\<^sub>n\<^sub>y_Person_invalid
@@ -1864,10 +1897,10 @@ lemmas [simp,code_unfold] = OclIsKindOf\<^sub>O\<^sub>c\<^sub>l\<^sub>A\<^sub>n\
                             OclIsKindOf\<^sub>P\<^sub>e\<^sub>r\<^sub>s\<^sub>o\<^sub>n_Planet_null
                             OclIsKindOf\<^sub>P\<^sub>e\<^sub>r\<^sub>s\<^sub>o\<^sub>n_Person_null
 
-(* 76 ************************************ 500 + 1 *)
+(* 77 ************************************ 507 + 1 *)
 subsection{* Validity and Definedness Properties *}
 
-(* 77 ************************************ 501 + 16 *)
+(* 78 ************************************ 508 + 16 *)
 lemma OclIsKindOf\<^sub>P\<^sub>e\<^sub>r\<^sub>s\<^sub>o\<^sub>n_Person_defined : 
 assumes isdef: "\<tau> \<Turnstile> (\<upsilon> (X))"
 shows "\<tau> \<Turnstile> (\<delta> ((X::Person) .oclIsKindOf(Person)))"
@@ -1933,7 +1966,7 @@ assumes isdef: "\<tau> \<Turnstile> (\<upsilon> (X))"
 shows "\<tau> \<Turnstile> (\<delta> ((X::Galaxy) .oclIsKindOf(OclAny)))"
 by(simp only: OclIsKindOf\<^sub>O\<^sub>c\<^sub>l\<^sub>A\<^sub>n\<^sub>y_Galaxy, rule defined_or_I[OF OclIsTypeOf\<^sub>O\<^sub>c\<^sub>l\<^sub>A\<^sub>n\<^sub>y_Galaxy_defined[OF isdef], OF OclIsKindOf\<^sub>G\<^sub>a\<^sub>l\<^sub>a\<^sub>x\<^sub>y_Galaxy_defined[OF isdef]]) 
 
-(* 78 ************************************ 517 + 16 *)
+(* 79 ************************************ 524 + 16 *)
 lemma OclIsKindOf\<^sub>P\<^sub>e\<^sub>r\<^sub>s\<^sub>o\<^sub>n_Person_defined' : 
 assumes isdef: "\<tau> \<Turnstile> (\<delta> (X))"
 shows "\<tau> \<Turnstile> (\<delta> ((X::Person) .oclIsKindOf(Person)))"
@@ -1999,40 +2032,40 @@ assumes isdef: "\<tau> \<Turnstile> (\<delta> (X))"
 shows "\<tau> \<Turnstile> (\<delta> ((X::Galaxy) .oclIsKindOf(OclAny)))"
 by(rule OclIsKindOf\<^sub>O\<^sub>c\<^sub>l\<^sub>A\<^sub>n\<^sub>y_Galaxy_defined[OF isdef[THEN foundation20]]) 
 
-(* 79 ************************************ 533 + 1 *)
+(* 80 ************************************ 540 + 1 *)
 subsection{* Up Down Casting *}
 
-(* 80 ************************************ 534 + 4 *)
+(* 81 ************************************ 541 + 4 *)
 lemma actual_eq_static\<^sub>P\<^sub>e\<^sub>r\<^sub>s\<^sub>o\<^sub>n : 
 assumes isdef: "\<tau> \<Turnstile> (\<delta> (X))"
 shows "\<tau> \<Turnstile> ((X::Person) .oclIsKindOf(Person))"
   apply(simp only: OclValid_def, insert isdef)
   apply(simp only: OclIsKindOf\<^sub>P\<^sub>e\<^sub>r\<^sub>s\<^sub>o\<^sub>n_Person)
   apply(auto simp: foundation16 bot_option_def split: option.split type\<^sub>P\<^sub>e\<^sub>r\<^sub>s\<^sub>o\<^sub>n.split typeoid\<^sub>P\<^sub>e\<^sub>r\<^sub>s\<^sub>o\<^sub>n.split)
-by(((simp add: false_def true_def OclOr_def OclAnd_def OclNot_def)+)?) 
+by((simp_all add: false_def true_def OclOr_def OclAnd_def OclNot_def)?) 
 lemma actual_eq_static\<^sub>P\<^sub>l\<^sub>a\<^sub>n\<^sub>e\<^sub>t : 
 assumes isdef: "\<tau> \<Turnstile> (\<delta> (X))"
 shows "\<tau> \<Turnstile> ((X::Planet) .oclIsKindOf(Planet))"
   apply(simp only: OclValid_def, insert isdef)
   apply(simp only: OclIsKindOf\<^sub>P\<^sub>l\<^sub>a\<^sub>n\<^sub>e\<^sub>t_Planet, subst (1) cp_OclOr, simp only: OclIsKindOf\<^sub>P\<^sub>e\<^sub>r\<^sub>s\<^sub>o\<^sub>n_Planet)
   apply(auto simp: cp_OclOr[symmetric ] foundation16 bot_option_def OclIsTypeOf\<^sub>P\<^sub>e\<^sub>r\<^sub>s\<^sub>o\<^sub>n_Planet split: option.split type\<^sub>P\<^sub>l\<^sub>a\<^sub>n\<^sub>e\<^sub>t.split typeoid\<^sub>P\<^sub>l\<^sub>a\<^sub>n\<^sub>e\<^sub>t.split type\<^sub>P\<^sub>e\<^sub>r\<^sub>s\<^sub>o\<^sub>n.split typeoid\<^sub>P\<^sub>e\<^sub>r\<^sub>s\<^sub>o\<^sub>n.split)
-by(((simp add: false_def true_def OclOr_def OclAnd_def OclNot_def)+)?) 
+by((simp_all add: false_def true_def OclOr_def OclAnd_def OclNot_def)?) 
 lemma actual_eq_static\<^sub>G\<^sub>a\<^sub>l\<^sub>a\<^sub>x\<^sub>y : 
 assumes isdef: "\<tau> \<Turnstile> (\<delta> (X))"
 shows "\<tau> \<Turnstile> ((X::Galaxy) .oclIsKindOf(Galaxy))"
   apply(simp only: OclValid_def, insert isdef)
   apply(simp only: OclIsKindOf\<^sub>G\<^sub>a\<^sub>l\<^sub>a\<^sub>x\<^sub>y_Galaxy, subst (1) cp_OclOr, simp only: OclIsKindOf\<^sub>P\<^sub>l\<^sub>a\<^sub>n\<^sub>e\<^sub>t_Galaxy, subst (2 1) cp_OclOr, simp only: OclIsKindOf\<^sub>P\<^sub>e\<^sub>r\<^sub>s\<^sub>o\<^sub>n_Galaxy)
   apply(auto simp: cp_OclOr[symmetric ] foundation16 bot_option_def OclIsTypeOf\<^sub>P\<^sub>e\<^sub>r\<^sub>s\<^sub>o\<^sub>n_Galaxy OclIsTypeOf\<^sub>P\<^sub>l\<^sub>a\<^sub>n\<^sub>e\<^sub>t_Galaxy split: option.split type\<^sub>G\<^sub>a\<^sub>l\<^sub>a\<^sub>x\<^sub>y.split typeoid\<^sub>G\<^sub>a\<^sub>l\<^sub>a\<^sub>x\<^sub>y.split type\<^sub>P\<^sub>e\<^sub>r\<^sub>s\<^sub>o\<^sub>n.split typeoid\<^sub>P\<^sub>e\<^sub>r\<^sub>s\<^sub>o\<^sub>n.split type\<^sub>P\<^sub>l\<^sub>a\<^sub>n\<^sub>e\<^sub>t.split typeoid\<^sub>P\<^sub>l\<^sub>a\<^sub>n\<^sub>e\<^sub>t.split)
-by(((simp add: false_def true_def OclOr_def OclAnd_def OclNot_def)+)?) 
+by((simp_all add: false_def true_def OclOr_def OclAnd_def OclNot_def)?) 
 lemma actual_eq_static\<^sub>O\<^sub>c\<^sub>l\<^sub>A\<^sub>n\<^sub>y : 
 assumes isdef: "\<tau> \<Turnstile> (\<delta> (X))"
 shows "\<tau> \<Turnstile> ((X::OclAny) .oclIsKindOf(OclAny))"
   apply(simp only: OclValid_def, insert isdef)
   apply(simp only: OclIsKindOf\<^sub>O\<^sub>c\<^sub>l\<^sub>A\<^sub>n\<^sub>y_OclAny, subst (1) cp_OclOr, simp only: OclIsKindOf\<^sub>G\<^sub>a\<^sub>l\<^sub>a\<^sub>x\<^sub>y_OclAny, subst (2 1) cp_OclOr, simp only: OclIsKindOf\<^sub>P\<^sub>l\<^sub>a\<^sub>n\<^sub>e\<^sub>t_OclAny, subst (3 2 1) cp_OclOr, simp only: OclIsKindOf\<^sub>P\<^sub>e\<^sub>r\<^sub>s\<^sub>o\<^sub>n_OclAny)
   apply(auto simp: cp_OclOr[symmetric ] foundation16 bot_option_def OclIsTypeOf\<^sub>P\<^sub>e\<^sub>r\<^sub>s\<^sub>o\<^sub>n_OclAny OclIsTypeOf\<^sub>P\<^sub>l\<^sub>a\<^sub>n\<^sub>e\<^sub>t_OclAny OclIsTypeOf\<^sub>G\<^sub>a\<^sub>l\<^sub>a\<^sub>x\<^sub>y_OclAny split: option.split type\<^sub>O\<^sub>c\<^sub>l\<^sub>A\<^sub>n\<^sub>y.split typeoid\<^sub>O\<^sub>c\<^sub>l\<^sub>A\<^sub>n\<^sub>y.split type\<^sub>P\<^sub>e\<^sub>r\<^sub>s\<^sub>o\<^sub>n.split typeoid\<^sub>P\<^sub>e\<^sub>r\<^sub>s\<^sub>o\<^sub>n.split type\<^sub>P\<^sub>l\<^sub>a\<^sub>n\<^sub>e\<^sub>t.split typeoid\<^sub>P\<^sub>l\<^sub>a\<^sub>n\<^sub>e\<^sub>t.split type\<^sub>G\<^sub>a\<^sub>l\<^sub>a\<^sub>x\<^sub>y.split typeoid\<^sub>G\<^sub>a\<^sub>l\<^sub>a\<^sub>x\<^sub>y.split)
-by(((simp add: false_def true_def OclOr_def OclAnd_def OclNot_def)+)?) 
+by((simp_all add: false_def true_def OclOr_def OclAnd_def OclNot_def)?) 
 
-(* 81 ************************************ 538 + 6 *)
+(* 82 ************************************ 545 + 6 *)
 lemma actualKind\<^sub>P\<^sub>e\<^sub>r\<^sub>s\<^sub>o\<^sub>n_larger_staticKind\<^sub>P\<^sub>l\<^sub>a\<^sub>n\<^sub>e\<^sub>t : 
 assumes isdef: "\<tau> \<Turnstile> (\<delta> (X))"
 shows "\<tau> \<Turnstile> ((X::Person) .oclIsKindOf(Planet))"
@@ -2064,7 +2097,7 @@ shows "\<tau> \<Turnstile> ((X::Galaxy) .oclIsKindOf(OclAny))"
   apply(simp only: OclIsKindOf\<^sub>O\<^sub>c\<^sub>l\<^sub>A\<^sub>n\<^sub>y_Galaxy)
 by(rule foundation25', rule actual_eq_static\<^sub>G\<^sub>a\<^sub>l\<^sub>a\<^sub>x\<^sub>y[OF isdef]) 
 
-(* 82 ************************************ 544 + 6 *)
+(* 83 ************************************ 551 + 6 *)
 lemma not_OclIsKindOf\<^sub>P\<^sub>e\<^sub>r\<^sub>s\<^sub>o\<^sub>n_then_Planet_OclIsTypeOf_others_unfold : 
 assumes isdef: "(\<tau> \<Turnstile> (\<delta> (X)))"
 assumes iskin: "(\<tau> \<Turnstile> ((X::Planet) .oclIsKindOf(Person)))"
@@ -2117,7 +2150,7 @@ shows "((\<tau> \<Turnstile> ((X::OclAny) .oclIsTypeOf(Galaxy))) \<or> ((\<tau> 
   apply(drule not_OclIsKindOf\<^sub>P\<^sub>l\<^sub>a\<^sub>n\<^sub>e\<^sub>t_then_OclAny_OclIsTypeOf_others_unfold[OF isdef], blast)
 done 
 
-(* 83 ************************************ 550 + 6 *)
+(* 84 ************************************ 557 + 6 *)
 lemma not_OclIsKindOf\<^sub>P\<^sub>e\<^sub>r\<^sub>s\<^sub>o\<^sub>n_then_Planet_OclIsTypeOf_others : 
 assumes iskin: "\<not> \<tau> \<Turnstile> ((X::Planet) .oclIsKindOf(Person))"
 assumes isdef: "\<tau> \<Turnstile> (\<delta> (X))"
@@ -2191,7 +2224,7 @@ shows "\<tau> \<Turnstile> ((X::OclAny) .oclIsTypeOf(OclAny))"
   apply(simp add: iskin)
 done 
 
-(* 84 ************************************ 556 + 10 *)
+(* 85 ************************************ 563 + 10 *)
 lemma down_cast_kind\<^sub>P\<^sub>e\<^sub>r\<^sub>s\<^sub>o\<^sub>n_from_Planet_to_Person : 
 assumes iskin: "\<not> \<tau> \<Turnstile> ((X::Planet) .oclIsKindOf(Person))"
 assumes isdef: "\<tau> \<Turnstile> (\<delta> (X))"
@@ -2268,64 +2301,64 @@ shows "\<tau> \<Turnstile> (X .oclAsType(Planet)) \<triangleq> invalid"
   apply(rule down_cast_type\<^sub>O\<^sub>c\<^sub>l\<^sub>A\<^sub>n\<^sub>y_from_OclAny_to_Planet, simp only: , simp only: isdef)
 done 
 
-(* 85 ************************************ 566 + 1 *)
+(* 86 ************************************ 573 + 1 *)
 section{* OclAllInstances *}
 
-(* 86 ************************************ 567 + 1 *)
+(* 87 ************************************ 574 + 1 *)
 text{* 
    To denote OCL-types occuring in OCL expressions syntactically---as, for example,  as
 ``argument'' of \inlineisar{oclAllInstances()}---we use the inverses of the injection
 functions into the object universes; we show that this is sufficient ``characterization.''  *}
 
-(* 87 ************************************ 568 + 4 *)
+(* 88 ************************************ 575 + 4 *)
 definition "Person = OclAsType\<^sub>P\<^sub>e\<^sub>r\<^sub>s\<^sub>o\<^sub>n_\<AA>"
 definition "Planet = OclAsType\<^sub>P\<^sub>l\<^sub>a\<^sub>n\<^sub>e\<^sub>t_\<AA>"
 definition "Galaxy = OclAsType\<^sub>G\<^sub>a\<^sub>l\<^sub>a\<^sub>x\<^sub>y_\<AA>"
 definition "OclAny = OclAsType\<^sub>O\<^sub>c\<^sub>l\<^sub>A\<^sub>n\<^sub>y_\<AA>"
 
-(* 88 ************************************ 572 + 1 *)
-lemmas [simp,code_unfold] = Person_def
+(* 89 ************************************ 579 + 1 *)
+lemmas[simp,code_unfold] = Person_def
                             Planet_def
                             Galaxy_def
                             OclAny_def
 
-(* 89 ************************************ 573 + 1 *)
+(* 90 ************************************ 580 + 1 *)
 lemma OclAsType\<^sub>O\<^sub>c\<^sub>l\<^sub>A\<^sub>n\<^sub>y_\<AA>_some : "(OclAsType\<^sub>O\<^sub>c\<^sub>l\<^sub>A\<^sub>n\<^sub>y_\<AA> (x)) \<noteq> None"
 by(simp add: OclAsType\<^sub>O\<^sub>c\<^sub>l\<^sub>A\<^sub>n\<^sub>y_\<AA>_def)
 
-(* 90 ************************************ 574 + 3 *)
+(* 91 ************************************ 581 + 3 *)
 lemma OclAllInstances_generic\<^sub>O\<^sub>c\<^sub>l\<^sub>A\<^sub>n\<^sub>y_exec : 
-shows "(OclAllInstances_generic (pre_post) (OclAny)) = (\<lambda>\<tau>. (Abs_Set_0 (\<lfloor>\<lfloor>Some ` OclAny ` (ran ((heap ((pre_post (\<tau>))))))\<rfloor>\<rfloor>)))"
+shows "(OclAllInstances_generic (pre_post) (OclAny)) = (\<lambda>\<tau>. (Abs_Set\<^sub>b\<^sub>a\<^sub>s\<^sub>e (\<lfloor>\<lfloor>Some ` OclAny ` (ran ((heap ((pre_post (\<tau>))))))\<rfloor>\<rfloor>)))"
   proof - let ?S1 = "(\<lambda>\<tau>. OclAny ` (ran ((heap ((pre_post (\<tau>)))))))" show ?thesis
   proof - let ?S2 = "(\<lambda>\<tau>. ((?S1) (\<tau>)) - {None})" show ?thesis
-  proof - have B: "(\<And>\<tau>. ((?S2) (\<tau>)) \<subseteq> ((?S1) (\<tau>)))" by(auto simp: ) show ?thesis
+  proof - have B: "(\<And>\<tau>. ((?S2) (\<tau>)) \<subseteq> ((?S1) (\<tau>)))" by(auto) show ?thesis
   proof - have C: "(\<And>\<tau>. ((?S1) (\<tau>)) \<subseteq> ((?S2) (\<tau>)))" by(auto simp: OclAsType\<^sub>O\<^sub>c\<^sub>l\<^sub>A\<^sub>n\<^sub>y_\<AA>_some) show ?thesis
   apply(simp add: OclValid_def del: OclAllInstances_generic_def OclIsKindOf\<^sub>O\<^sub>c\<^sub>l\<^sub>A\<^sub>n\<^sub>y_OclAny)
 by(insert equalityI[OF B, OF C], simp) qed qed qed qed
 lemma OclAllInstances_at_post\<^sub>O\<^sub>c\<^sub>l\<^sub>A\<^sub>n\<^sub>y_exec : 
-shows "(OclAllInstances_at_post (OclAny)) = (\<lambda>\<tau>. (Abs_Set_0 (\<lfloor>\<lfloor>Some ` OclAny ` (ran ((heap ((snd (\<tau>))))))\<rfloor>\<rfloor>)))"
+shows "(OclAllInstances_at_post (OclAny)) = (\<lambda>\<tau>. (Abs_Set\<^sub>b\<^sub>a\<^sub>s\<^sub>e (\<lfloor>\<lfloor>Some ` OclAny ` (ran ((heap ((snd (\<tau>))))))\<rfloor>\<rfloor>)))"
   unfolding OclAllInstances_at_post_def
 by(rule OclAllInstances_generic\<^sub>O\<^sub>c\<^sub>l\<^sub>A\<^sub>n\<^sub>y_exec) 
 lemma OclAllInstances_at_pre\<^sub>O\<^sub>c\<^sub>l\<^sub>A\<^sub>n\<^sub>y_exec : 
-shows "(OclAllInstances_at_pre (OclAny)) = (\<lambda>\<tau>. (Abs_Set_0 (\<lfloor>\<lfloor>Some ` OclAny ` (ran ((heap ((fst (\<tau>))))))\<rfloor>\<rfloor>)))"
+shows "(OclAllInstances_at_pre (OclAny)) = (\<lambda>\<tau>. (Abs_Set\<^sub>b\<^sub>a\<^sub>s\<^sub>e (\<lfloor>\<lfloor>Some ` OclAny ` (ran ((heap ((fst (\<tau>))))))\<rfloor>\<rfloor>)))"
   unfolding OclAllInstances_at_pre_def
 by(rule OclAllInstances_generic\<^sub>O\<^sub>c\<^sub>l\<^sub>A\<^sub>n\<^sub>y_exec) 
 
-(* 91 ************************************ 577 + 1 *)
+(* 92 ************************************ 584 + 1 *)
 subsection{* OclIsTypeOf *}
 
-(* 92 ************************************ 578 + 2 *)
+(* 93 ************************************ 585 + 2 *)
 lemma ex_ssubst : "(\<forall>x \<in> B. (s (x)) = (t (x))) \<Longrightarrow> (\<exists>x \<in> B. (P ((s (x))))) = (\<exists>x \<in> B. (P ((t (x)))))"
 by(simp)
 lemma ex_def : "x \<in> \<lceil>\<lceil>\<lfloor>\<lfloor>Some ` (X - {None})\<rfloor>\<rfloor>\<rceil>\<rceil> \<Longrightarrow> (\<exists>y. x = \<lfloor>\<lfloor>y\<rfloor>\<rfloor>)"
-by(auto simp: )
+by(auto)
 
-(* 93 ************************************ 580 + 21 *)
+(* 94 ************************************ 587 + 21 *)
 lemma Person_OclAllInstances_generic_OclIsTypeOf\<^sub>P\<^sub>e\<^sub>r\<^sub>s\<^sub>o\<^sub>n : "\<tau> \<Turnstile> (OclForall ((OclAllInstances_generic (pre_post) (Person))) (OclIsTypeOf\<^sub>P\<^sub>e\<^sub>r\<^sub>s\<^sub>o\<^sub>n))"
   apply(simp add: OclValid_def del: OclAllInstances_generic_def)
   apply(simp only: OclForall_def refl if_True OclAllInstances_generic_defined[simplified OclValid_def])
   apply(simp only: OclAllInstances_generic_def)
-  apply(subst (1 2 3) Abs_Set_0_inverse, simp add: bot_option_def)
+  apply(subst (1 2 3) Abs_Set\<^sub>b\<^sub>a\<^sub>s\<^sub>e_inverse, simp add: bot_option_def)
   apply(subst (1 2 3) ex_ssubst[where s = "(\<lambda>x. (((\<lambda>_. x) .oclIsTypeOf(Person)) (\<tau>)))" and t = "(\<lambda>_. (true (\<tau>)))"])
   apply(intro ballI actual_eq_static\<^sub>P\<^sub>e\<^sub>r\<^sub>s\<^sub>o\<^sub>n[simplified OclValid_def, simplified OclIsKindOf\<^sub>P\<^sub>e\<^sub>r\<^sub>s\<^sub>o\<^sub>n_Person])
   apply(drule ex_def, erule exE, simp)
@@ -2344,7 +2377,7 @@ shows "(\<exists>\<tau>. \<tau> \<Turnstile> (OclForall ((OclAllInstances_generi
   apply(rule exI[where x = "\<tau>\<^sub>0"], simp add: \<tau>\<^sub>0_def OclValid_def del: OclAllInstances_generic_def)
   apply(simp only: OclForall_def refl if_True OclAllInstances_generic_defined[simplified OclValid_def])
   apply(simp only: OclAllInstances_generic_def)
-  apply(subst (1 2 3) Abs_Set_0_inverse, simp add: bot_option_def)
+  apply(subst (1 2 3) Abs_Set\<^sub>b\<^sub>a\<^sub>s\<^sub>e_inverse, simp add: bot_option_def)
 by(simp) 
 lemma Planet_OclAllInstances_at_post_OclIsTypeOf\<^sub>P\<^sub>l\<^sub>a\<^sub>n\<^sub>e\<^sub>t1 : 
 shows "(\<exists>\<tau>. \<tau> \<Turnstile> (OclForall ((OclAllInstances_at_post (Planet))) (OclIsTypeOf\<^sub>P\<^sub>l\<^sub>a\<^sub>n\<^sub>e\<^sub>t)))"
@@ -2362,7 +2395,7 @@ shows "(\<exists>\<tau>. \<tau> \<Turnstile> (not ((OclForall ((OclAllInstances_
   apply(rule exI[where x = "(?t0 , ?t0)"], simp add: OclValid_def del: OclAllInstances_generic_def)
   apply(simp only: OclForall_def refl if_True OclAllInstances_generic_defined[simplified OclValid_def])
   apply(simp only: OclAllInstances_generic_def OclAsType\<^sub>P\<^sub>l\<^sub>a\<^sub>n\<^sub>e\<^sub>t_\<AA>_def)
-  apply(subst (1 2 3) Abs_Set_0_inverse, simp add: bot_option_def)
+  apply(subst (1 2 3) Abs_Set\<^sub>b\<^sub>a\<^sub>s\<^sub>e_inverse, simp add: bot_option_def)
 by(simp add: state.make_def OclNot_def) qed qed
 lemma Planet_OclAllInstances_at_post_OclIsTypeOf\<^sub>P\<^sub>l\<^sub>a\<^sub>n\<^sub>e\<^sub>t2 : 
 shows "(\<exists>\<tau>. \<tau> \<Turnstile> (not ((OclForall ((OclAllInstances_at_post (Planet))) (OclIsTypeOf\<^sub>P\<^sub>l\<^sub>a\<^sub>n\<^sub>e\<^sub>t)))))"
@@ -2378,7 +2411,7 @@ shows "(\<exists>\<tau>. \<tau> \<Turnstile> (OclForall ((OclAllInstances_generi
   apply(rule exI[where x = "\<tau>\<^sub>0"], simp add: \<tau>\<^sub>0_def OclValid_def del: OclAllInstances_generic_def)
   apply(simp only: OclForall_def refl if_True OclAllInstances_generic_defined[simplified OclValid_def])
   apply(simp only: OclAllInstances_generic_def)
-  apply(subst (1 2 3) Abs_Set_0_inverse, simp add: bot_option_def)
+  apply(subst (1 2 3) Abs_Set\<^sub>b\<^sub>a\<^sub>s\<^sub>e_inverse, simp add: bot_option_def)
 by(simp) 
 lemma Galaxy_OclAllInstances_at_post_OclIsTypeOf\<^sub>G\<^sub>a\<^sub>l\<^sub>a\<^sub>x\<^sub>y1 : 
 shows "(\<exists>\<tau>. \<tau> \<Turnstile> (OclForall ((OclAllInstances_at_post (Galaxy))) (OclIsTypeOf\<^sub>G\<^sub>a\<^sub>l\<^sub>a\<^sub>x\<^sub>y)))"
@@ -2396,7 +2429,7 @@ shows "(\<exists>\<tau>. \<tau> \<Turnstile> (not ((OclForall ((OclAllInstances_
   apply(rule exI[where x = "(?t0 , ?t0)"], simp add: OclValid_def del: OclAllInstances_generic_def)
   apply(simp only: OclForall_def refl if_True OclAllInstances_generic_defined[simplified OclValid_def])
   apply(simp only: OclAllInstances_generic_def OclAsType\<^sub>G\<^sub>a\<^sub>l\<^sub>a\<^sub>x\<^sub>y_\<AA>_def)
-  apply(subst (1 2 3) Abs_Set_0_inverse, simp add: bot_option_def)
+  apply(subst (1 2 3) Abs_Set\<^sub>b\<^sub>a\<^sub>s\<^sub>e_inverse, simp add: bot_option_def)
 by(simp add: state.make_def OclNot_def) qed qed
 lemma Galaxy_OclAllInstances_at_post_OclIsTypeOf\<^sub>G\<^sub>a\<^sub>l\<^sub>a\<^sub>x\<^sub>y2 : 
 shows "(\<exists>\<tau>. \<tau> \<Turnstile> (not ((OclForall ((OclAllInstances_at_post (Galaxy))) (OclIsTypeOf\<^sub>G\<^sub>a\<^sub>l\<^sub>a\<^sub>x\<^sub>y)))))"
@@ -2412,7 +2445,7 @@ shows "(\<exists>\<tau>. \<tau> \<Turnstile> (OclForall ((OclAllInstances_generi
   apply(rule exI[where x = "\<tau>\<^sub>0"], simp add: \<tau>\<^sub>0_def OclValid_def del: OclAllInstances_generic_def)
   apply(simp only: OclForall_def refl if_True OclAllInstances_generic_defined[simplified OclValid_def])
   apply(simp only: OclAllInstances_generic_def)
-  apply(subst (1 2 3) Abs_Set_0_inverse, simp add: bot_option_def)
+  apply(subst (1 2 3) Abs_Set\<^sub>b\<^sub>a\<^sub>s\<^sub>e_inverse, simp add: bot_option_def)
 by(simp) 
 lemma OclAny_OclAllInstances_at_post_OclIsTypeOf\<^sub>O\<^sub>c\<^sub>l\<^sub>A\<^sub>n\<^sub>y1 : 
 shows "(\<exists>\<tau>. \<tau> \<Turnstile> (OclForall ((OclAllInstances_at_post (OclAny))) (OclIsTypeOf\<^sub>O\<^sub>c\<^sub>l\<^sub>A\<^sub>n\<^sub>y)))"
@@ -2430,7 +2463,7 @@ shows "(\<exists>\<tau>. \<tau> \<Turnstile> (not ((OclForall ((OclAllInstances_
   apply(rule exI[where x = "(?t0 , ?t0)"], simp add: OclValid_def del: OclAllInstances_generic_def)
   apply(simp only: OclForall_def refl if_True OclAllInstances_generic_defined[simplified OclValid_def])
   apply(simp only: OclAllInstances_generic_def OclAsType\<^sub>O\<^sub>c\<^sub>l\<^sub>A\<^sub>n\<^sub>y_\<AA>_def)
-  apply(subst (1 2 3) Abs_Set_0_inverse, simp add: bot_option_def)
+  apply(subst (1 2 3) Abs_Set\<^sub>b\<^sub>a\<^sub>s\<^sub>e_inverse, simp add: bot_option_def)
 by(simp add: state.make_def OclNot_def) qed qed
 lemma OclAny_OclAllInstances_at_post_OclIsTypeOf\<^sub>O\<^sub>c\<^sub>l\<^sub>A\<^sub>n\<^sub>y2 : 
 shows "(\<exists>\<tau>. \<tau> \<Turnstile> (not ((OclForall ((OclAllInstances_at_post (OclAny))) (OclIsTypeOf\<^sub>O\<^sub>c\<^sub>l\<^sub>A\<^sub>n\<^sub>y)))))"
@@ -2441,15 +2474,15 @@ shows "(\<exists>\<tau>. \<tau> \<Turnstile> (not ((OclForall ((OclAllInstances_
   unfolding OclAllInstances_at_pre_def
 by(rule OclAny_OclAllInstances_generic_OclIsTypeOf\<^sub>O\<^sub>c\<^sub>l\<^sub>A\<^sub>n\<^sub>y2, simp) 
 
-(* 94 ************************************ 601 + 1 *)
+(* 95 ************************************ 608 + 1 *)
 subsection{* OclIsKindOf *}
 
-(* 95 ************************************ 602 + 12 *)
+(* 96 ************************************ 609 + 12 *)
 lemma Person_OclAllInstances_generic_OclIsKindOf\<^sub>P\<^sub>e\<^sub>r\<^sub>s\<^sub>o\<^sub>n : "\<tau> \<Turnstile> (OclForall ((OclAllInstances_generic (pre_post) (Person))) (OclIsKindOf\<^sub>P\<^sub>e\<^sub>r\<^sub>s\<^sub>o\<^sub>n))"
   apply(simp add: OclValid_def del: OclAllInstances_generic_def OclIsKindOf\<^sub>P\<^sub>e\<^sub>r\<^sub>s\<^sub>o\<^sub>n_Person)
   apply(simp only: OclForall_def refl if_True OclAllInstances_generic_defined[simplified OclValid_def])
   apply(simp only: OclAllInstances_generic_def)
-  apply(subst (1 2 3) Abs_Set_0_inverse, simp add: bot_option_def)
+  apply(subst (1 2 3) Abs_Set\<^sub>b\<^sub>a\<^sub>s\<^sub>e_inverse, simp add: bot_option_def)
   apply(subst (1 2 3) ex_ssubst[where s = "(\<lambda>x. (((\<lambda>_. x) .oclIsKindOf(Person)) (\<tau>)))" and t = "(\<lambda>_. (true (\<tau>)))"])
   apply(intro ballI actual_eq_static\<^sub>P\<^sub>e\<^sub>r\<^sub>s\<^sub>o\<^sub>n[simplified OclValid_def])
   apply(drule ex_def, erule exE, simp)
@@ -2466,7 +2499,7 @@ lemma Planet_OclAllInstances_generic_OclIsKindOf\<^sub>P\<^sub>l\<^sub>a\<^sub>n
   apply(simp add: OclValid_def del: OclAllInstances_generic_def OclIsKindOf\<^sub>P\<^sub>l\<^sub>a\<^sub>n\<^sub>e\<^sub>t_Planet)
   apply(simp only: OclForall_def refl if_True OclAllInstances_generic_defined[simplified OclValid_def])
   apply(simp only: OclAllInstances_generic_def)
-  apply(subst (1 2 3) Abs_Set_0_inverse, simp add: bot_option_def)
+  apply(subst (1 2 3) Abs_Set\<^sub>b\<^sub>a\<^sub>s\<^sub>e_inverse, simp add: bot_option_def)
   apply(subst (1 2 3) ex_ssubst[where s = "(\<lambda>x. (((\<lambda>_. x) .oclIsKindOf(Planet)) (\<tau>)))" and t = "(\<lambda>_. (true (\<tau>)))"])
   apply(intro ballI actual_eq_static\<^sub>P\<^sub>l\<^sub>a\<^sub>n\<^sub>e\<^sub>t[simplified OclValid_def])
   apply(drule ex_def, erule exE, simp)
@@ -2483,7 +2516,7 @@ lemma Galaxy_OclAllInstances_generic_OclIsKindOf\<^sub>G\<^sub>a\<^sub>l\<^sub>a
   apply(simp add: OclValid_def del: OclAllInstances_generic_def OclIsKindOf\<^sub>G\<^sub>a\<^sub>l\<^sub>a\<^sub>x\<^sub>y_Galaxy)
   apply(simp only: OclForall_def refl if_True OclAllInstances_generic_defined[simplified OclValid_def])
   apply(simp only: OclAllInstances_generic_def)
-  apply(subst (1 2 3) Abs_Set_0_inverse, simp add: bot_option_def)
+  apply(subst (1 2 3) Abs_Set\<^sub>b\<^sub>a\<^sub>s\<^sub>e_inverse, simp add: bot_option_def)
   apply(subst (1 2 3) ex_ssubst[where s = "(\<lambda>x. (((\<lambda>_. x) .oclIsKindOf(Galaxy)) (\<tau>)))" and t = "(\<lambda>_. (true (\<tau>)))"])
   apply(intro ballI actual_eq_static\<^sub>G\<^sub>a\<^sub>l\<^sub>a\<^sub>x\<^sub>y[simplified OclValid_def])
   apply(drule ex_def, erule exE, simp)
@@ -2500,7 +2533,7 @@ lemma OclAny_OclAllInstances_generic_OclIsKindOf\<^sub>O\<^sub>c\<^sub>l\<^sub>A
   apply(simp add: OclValid_def del: OclAllInstances_generic_def OclIsKindOf\<^sub>O\<^sub>c\<^sub>l\<^sub>A\<^sub>n\<^sub>y_OclAny)
   apply(simp only: OclForall_def refl if_True OclAllInstances_generic_defined[simplified OclValid_def])
   apply(simp only: OclAllInstances_generic_def)
-  apply(subst (1 2 3) Abs_Set_0_inverse, simp add: bot_option_def)
+  apply(subst (1 2 3) Abs_Set\<^sub>b\<^sub>a\<^sub>s\<^sub>e_inverse, simp add: bot_option_def)
   apply(subst (1 2 3) ex_ssubst[where s = "(\<lambda>x. (((\<lambda>_. x) .oclIsKindOf(OclAny)) (\<tau>)))" and t = "(\<lambda>_. (true (\<tau>)))"])
   apply(intro ballI actual_eq_static\<^sub>O\<^sub>c\<^sub>l\<^sub>A\<^sub>n\<^sub>y[simplified OclValid_def])
   apply(drule ex_def, erule exE, simp)
@@ -2514,12 +2547,12 @@ shows "\<tau> \<Turnstile> (OclForall ((OclAllInstances_at_pre (OclAny))) (OclIs
   unfolding OclAllInstances_at_pre_def
 by(rule OclAny_OclAllInstances_generic_OclIsKindOf\<^sub>O\<^sub>c\<^sub>l\<^sub>A\<^sub>n\<^sub>y) 
 
-(* 96 ************************************ 614 + 18 *)
+(* 97 ************************************ 621 + 18 *)
 lemma Person_OclAllInstances_generic_OclIsKindOf\<^sub>P\<^sub>l\<^sub>a\<^sub>n\<^sub>e\<^sub>t : "\<tau> \<Turnstile> (OclForall ((OclAllInstances_generic (pre_post) (Person))) (OclIsKindOf\<^sub>P\<^sub>l\<^sub>a\<^sub>n\<^sub>e\<^sub>t))"
   apply(simp add: OclValid_def del: OclAllInstances_generic_def OclIsKindOf\<^sub>P\<^sub>l\<^sub>a\<^sub>n\<^sub>e\<^sub>t_Person)
   apply(simp only: OclForall_def refl if_True OclAllInstances_generic_defined[simplified OclValid_def])
   apply(simp only: OclAllInstances_generic_def)
-  apply(subst (1 2 3) Abs_Set_0_inverse, simp add: bot_option_def)
+  apply(subst (1 2 3) Abs_Set\<^sub>b\<^sub>a\<^sub>s\<^sub>e_inverse, simp add: bot_option_def)
   apply(subst (1 2 3) ex_ssubst[where s = "(\<lambda>x. (((\<lambda>_. x) .oclIsKindOf(Planet)) (\<tau>)))" and t = "(\<lambda>_. (true (\<tau>)))"])
   apply(intro ballI actualKind\<^sub>P\<^sub>e\<^sub>r\<^sub>s\<^sub>o\<^sub>n_larger_staticKind\<^sub>P\<^sub>l\<^sub>a\<^sub>n\<^sub>e\<^sub>t[simplified OclValid_def])
   apply(drule ex_def, erule exE, simp)
@@ -2536,7 +2569,7 @@ lemma Person_OclAllInstances_generic_OclIsKindOf\<^sub>G\<^sub>a\<^sub>l\<^sub>a
   apply(simp add: OclValid_def del: OclAllInstances_generic_def OclIsKindOf\<^sub>G\<^sub>a\<^sub>l\<^sub>a\<^sub>x\<^sub>y_Person)
   apply(simp only: OclForall_def refl if_True OclAllInstances_generic_defined[simplified OclValid_def])
   apply(simp only: OclAllInstances_generic_def)
-  apply(subst (1 2 3) Abs_Set_0_inverse, simp add: bot_option_def)
+  apply(subst (1 2 3) Abs_Set\<^sub>b\<^sub>a\<^sub>s\<^sub>e_inverse, simp add: bot_option_def)
   apply(subst (1 2 3) ex_ssubst[where s = "(\<lambda>x. (((\<lambda>_. x) .oclIsKindOf(Galaxy)) (\<tau>)))" and t = "(\<lambda>_. (true (\<tau>)))"])
   apply(intro ballI actualKind\<^sub>P\<^sub>e\<^sub>r\<^sub>s\<^sub>o\<^sub>n_larger_staticKind\<^sub>G\<^sub>a\<^sub>l\<^sub>a\<^sub>x\<^sub>y[simplified OclValid_def])
   apply(drule ex_def, erule exE, simp)
@@ -2553,7 +2586,7 @@ lemma Person_OclAllInstances_generic_OclIsKindOf\<^sub>O\<^sub>c\<^sub>l\<^sub>A
   apply(simp add: OclValid_def del: OclAllInstances_generic_def OclIsKindOf\<^sub>O\<^sub>c\<^sub>l\<^sub>A\<^sub>n\<^sub>y_Person)
   apply(simp only: OclForall_def refl if_True OclAllInstances_generic_defined[simplified OclValid_def])
   apply(simp only: OclAllInstances_generic_def)
-  apply(subst (1 2 3) Abs_Set_0_inverse, simp add: bot_option_def)
+  apply(subst (1 2 3) Abs_Set\<^sub>b\<^sub>a\<^sub>s\<^sub>e_inverse, simp add: bot_option_def)
   apply(subst (1 2 3) ex_ssubst[where s = "(\<lambda>x. (((\<lambda>_. x) .oclIsKindOf(OclAny)) (\<tau>)))" and t = "(\<lambda>_. (true (\<tau>)))"])
   apply(intro ballI actualKind\<^sub>P\<^sub>e\<^sub>r\<^sub>s\<^sub>o\<^sub>n_larger_staticKind\<^sub>O\<^sub>c\<^sub>l\<^sub>A\<^sub>n\<^sub>y[simplified OclValid_def])
   apply(drule ex_def, erule exE, simp)
@@ -2570,7 +2603,7 @@ lemma Planet_OclAllInstances_generic_OclIsKindOf\<^sub>G\<^sub>a\<^sub>l\<^sub>a
   apply(simp add: OclValid_def del: OclAllInstances_generic_def OclIsKindOf\<^sub>G\<^sub>a\<^sub>l\<^sub>a\<^sub>x\<^sub>y_Planet)
   apply(simp only: OclForall_def refl if_True OclAllInstances_generic_defined[simplified OclValid_def])
   apply(simp only: OclAllInstances_generic_def)
-  apply(subst (1 2 3) Abs_Set_0_inverse, simp add: bot_option_def)
+  apply(subst (1 2 3) Abs_Set\<^sub>b\<^sub>a\<^sub>s\<^sub>e_inverse, simp add: bot_option_def)
   apply(subst (1 2 3) ex_ssubst[where s = "(\<lambda>x. (((\<lambda>_. x) .oclIsKindOf(Galaxy)) (\<tau>)))" and t = "(\<lambda>_. (true (\<tau>)))"])
   apply(intro ballI actualKind\<^sub>P\<^sub>l\<^sub>a\<^sub>n\<^sub>e\<^sub>t_larger_staticKind\<^sub>G\<^sub>a\<^sub>l\<^sub>a\<^sub>x\<^sub>y[simplified OclValid_def])
   apply(drule ex_def, erule exE, simp)
@@ -2587,7 +2620,7 @@ lemma Planet_OclAllInstances_generic_OclIsKindOf\<^sub>O\<^sub>c\<^sub>l\<^sub>A
   apply(simp add: OclValid_def del: OclAllInstances_generic_def OclIsKindOf\<^sub>O\<^sub>c\<^sub>l\<^sub>A\<^sub>n\<^sub>y_Planet)
   apply(simp only: OclForall_def refl if_True OclAllInstances_generic_defined[simplified OclValid_def])
   apply(simp only: OclAllInstances_generic_def)
-  apply(subst (1 2 3) Abs_Set_0_inverse, simp add: bot_option_def)
+  apply(subst (1 2 3) Abs_Set\<^sub>b\<^sub>a\<^sub>s\<^sub>e_inverse, simp add: bot_option_def)
   apply(subst (1 2 3) ex_ssubst[where s = "(\<lambda>x. (((\<lambda>_. x) .oclIsKindOf(OclAny)) (\<tau>)))" and t = "(\<lambda>_. (true (\<tau>)))"])
   apply(intro ballI actualKind\<^sub>P\<^sub>l\<^sub>a\<^sub>n\<^sub>e\<^sub>t_larger_staticKind\<^sub>O\<^sub>c\<^sub>l\<^sub>A\<^sub>n\<^sub>y[simplified OclValid_def])
   apply(drule ex_def, erule exE, simp)
@@ -2604,7 +2637,7 @@ lemma Galaxy_OclAllInstances_generic_OclIsKindOf\<^sub>O\<^sub>c\<^sub>l\<^sub>A
   apply(simp add: OclValid_def del: OclAllInstances_generic_def OclIsKindOf\<^sub>O\<^sub>c\<^sub>l\<^sub>A\<^sub>n\<^sub>y_Galaxy)
   apply(simp only: OclForall_def refl if_True OclAllInstances_generic_defined[simplified OclValid_def])
   apply(simp only: OclAllInstances_generic_def)
-  apply(subst (1 2 3) Abs_Set_0_inverse, simp add: bot_option_def)
+  apply(subst (1 2 3) Abs_Set\<^sub>b\<^sub>a\<^sub>s\<^sub>e_inverse, simp add: bot_option_def)
   apply(subst (1 2 3) ex_ssubst[where s = "(\<lambda>x. (((\<lambda>_. x) .oclIsKindOf(OclAny)) (\<tau>)))" and t = "(\<lambda>_. (true (\<tau>)))"])
   apply(intro ballI actualKind\<^sub>G\<^sub>a\<^sub>l\<^sub>a\<^sub>x\<^sub>y_larger_staticKind\<^sub>O\<^sub>c\<^sub>l\<^sub>A\<^sub>n\<^sub>y[simplified OclValid_def])
   apply(drule ex_def, erule exE, simp)
@@ -2618,53 +2651,53 @@ shows "\<tau> \<Turnstile> (OclForall ((OclAllInstances_at_pre (Galaxy))) (OclIs
   unfolding OclAllInstances_at_pre_def
 by(rule Galaxy_OclAllInstances_generic_OclIsKindOf\<^sub>O\<^sub>c\<^sub>l\<^sub>A\<^sub>n\<^sub>y) 
 
-(* 97 ************************************ 632 + 1 *)
+(* 98 ************************************ 639 + 1 *)
 section{* The Accessors *}
 
-(* 98 ************************************ 633 + 1 *)
+(* 99 ************************************ 640 + 1 *)
 text{* 
   \label{sec:edm-accessors} *}
 
-(* 99 ************************************ 634 + 1 *)
+(* 100 ************************************ 641 + 1 *)
 text{*  *}
 
-(* 100 ************************************ 635 + 1 *)
+(* 101 ************************************ 642 + 1 *)
 subsection{* Definition *}
 
-(* 101 ************************************ 636 + 1 *)
+(* 102 ************************************ 643 + 1 *)
 text{*  *}
 
-(* 102 ************************************ 637 + 1 *)
+(* 103 ************************************ 644 + 1 *)
 ML{* val oidPerson_0_boss = 0 *}
 
-(* 103 ************************************ 638 + 1 *)
+(* 104 ************************************ 645 + 1 *)
 definition "oid\<^sub>P\<^sub>e\<^sub>r\<^sub>s\<^sub>o\<^sub>n_0_\<B>\<O>\<S>\<S> = 0"
 
-(* 104 ************************************ 639 + 1 *)
+(* 105 ************************************ 646 + 1 *)
 text{*  *}
 
-(* 105 ************************************ 640 + 4 *)
+(* 106 ************************************ 647 + 4 *)
 definition "eval_extract x f = (\<lambda>\<tau>. (case x \<tau> of \<lfloor>\<lfloor>obj\<rfloor>\<rfloor> \<Rightarrow> (f ((oid_of (obj))) (\<tau>))
     | _ \<Rightarrow> invalid \<tau>))"
 definition "in_pre_state = fst"
 definition "in_post_state = snd"
 definition "reconst_basetype = id"
 
-(* 106 ************************************ 644 + 1 *)
+(* 107 ************************************ 651 + 1 *)
 text{*  *}
 
-(* 107 ************************************ 645 + 2 *)
+(* 108 ************************************ 652 + 2 *)
 ML{* val switch2_01 = (fn [x0 , x1] => (x0 , x1)) *}
 ML{* val switch2_10 = (fn [x0 , x1] => (x1 , x0)) *}
 
-(* 108 ************************************ 647 + 4 *)
+(* 109 ************************************ 654 + 4 *)
 definition "switch\<^sub>2_01 = (\<lambda> [x0 , x1] \<Rightarrow> (x0 , x1))"
 definition "switch\<^sub>2_10 = (\<lambda> [x0 , x1] \<Rightarrow> (x1 , x0))"
 definition "List_flatten = (\<lambda>l. (foldl ((\<lambda>acc. (\<lambda>l. (foldl ((\<lambda>acc. (\<lambda>l. (Cons (l) (acc))))) (acc) ((rev (l))))))) (Nil) ((rev (l)))))"
 definition "deref_assocs pre_post to_from assoc_oid f oid = (\<lambda>\<tau>. (case (assocs ((pre_post (\<tau>))) (assoc_oid)) of \<lfloor>S\<rfloor> \<Rightarrow> (f ((deref_assocs_list (to_from) (oid) (S))) (\<tau>))
     | _ \<Rightarrow> (invalid (\<tau>))))"
 
-(* 109 ************************************ 651 + 4 *)
+(* 110 ************************************ 658 + 4 *)
 definition "deref_oid\<^sub>P\<^sub>e\<^sub>r\<^sub>s\<^sub>o\<^sub>n fst_snd f oid = (\<lambda>\<tau>. (case (heap (fst_snd \<tau>) (oid)) of \<lfloor>in\<^sub>P\<^sub>e\<^sub>r\<^sub>s\<^sub>o\<^sub>n obj\<rfloor> \<Rightarrow> f obj \<tau>
     | _ \<Rightarrow> invalid \<tau>))"
 definition "deref_oid\<^sub>P\<^sub>l\<^sub>a\<^sub>n\<^sub>e\<^sub>t fst_snd f oid = (\<lambda>\<tau>. (case (heap (fst_snd \<tau>) (oid)) of \<lfloor>in\<^sub>P\<^sub>l\<^sub>a\<^sub>n\<^sub>e\<^sub>t obj\<rfloor> \<Rightarrow> f obj \<tau>
@@ -2674,21 +2707,21 @@ definition "deref_oid\<^sub>G\<^sub>a\<^sub>l\<^sub>a\<^sub>x\<^sub>y fst_snd f 
 definition "deref_oid\<^sub>O\<^sub>c\<^sub>l\<^sub>A\<^sub>n\<^sub>y fst_snd f oid = (\<lambda>\<tau>. (case (heap (fst_snd \<tau>) (oid)) of \<lfloor>in\<^sub>O\<^sub>c\<^sub>l\<^sub>A\<^sub>n\<^sub>y obj\<rfloor> \<Rightarrow> f obj \<tau>
     | _ \<Rightarrow> invalid \<tau>))"
 
-(* 110 ************************************ 655 + 0 *)
+(* 111 ************************************ 662 + 0 *)
 
-(* 111 ************************************ 655 + 1 *)
+(* 112 ************************************ 662 + 1 *)
 text{*  *}
 
-(* 112 ************************************ 656 + 3 *)
+(* 113 ************************************ 663 + 3 *)
 definition "select_object mt incl smash deref l = (smash ((foldl (incl) (mt) ((List.map (deref) (l))))))"
-definition "select_object_set f p = (select_object (mtSet) (OclIncluding) (id) ((f (p))))"
+definition "select_object_set f p = (select_object (mtSet) (UML_Set.OclIncluding) (id) ((f (p))))"
 definition "select_object_set_any f p s_set = (OclANY ((select_object_set (f) (p) (s_set))))"
 
-(* 113 ************************************ 659 + 1 *)
+(* 114 ************************************ 666 + 1 *)
 text{* 
    pointer undefined in state or not referencing a type conform object representation  *}
 
-(* 114 ************************************ 660 + 12 *)
+(* 115 ************************************ 667 + 12 *)
 definition "select\<^sub>P\<^sub>e\<^sub>r\<^sub>s\<^sub>o\<^sub>n\<B>\<O>\<S>\<S> f = (\<lambda> (mkoid\<^sub>P\<^sub>e\<^sub>r\<^sub>s\<^sub>o\<^sub>n (_) (\<bottom>) (_)) \<Rightarrow> null
     | (mkoid\<^sub>P\<^sub>e\<^sub>r\<^sub>s\<^sub>o\<^sub>n (_) (\<lfloor>boss\<rfloor>) (_)) \<Rightarrow> (f ((\<lambda>x _. \<lfloor>\<lfloor>x\<rfloor>\<rfloor>)) (boss)))"
 definition "select\<^sub>P\<^sub>e\<^sub>r\<^sub>s\<^sub>o\<^sub>n\<S>\<A>\<L>\<A>\<R>\<Y> f = (\<lambda> (mkoid\<^sub>P\<^sub>e\<^sub>r\<^sub>s\<^sub>o\<^sub>n (_) (_) (\<bottom>)) \<Rightarrow> null
@@ -2716,9 +2749,9 @@ definition "select\<^sub>P\<^sub>l\<^sub>a\<^sub>n\<^sub>e\<^sub>t\<M>\<O>\<V>\<
     | (mkoid\<^sub>P\<^sub>l\<^sub>a\<^sub>n\<^sub>e\<^sub>t ((mk\<^sub>P\<^sub>l\<^sub>a\<^sub>n\<^sub>e\<^sub>t (_) (_) (\<lfloor>moving\<rfloor>))) (_) (_)) \<Rightarrow> (f ((\<lambda>x _. \<lfloor>\<lfloor>x\<rfloor>\<rfloor>)) (moving))
     | (mkoid\<^sub>P\<^sub>l\<^sub>a\<^sub>n\<^sub>e\<^sub>t ((mk\<^sub>P\<^sub>l\<^sub>a\<^sub>n\<^sub>e\<^sub>t_\<^sub>P\<^sub>e\<^sub>r\<^sub>s\<^sub>o\<^sub>n (person))) (_) (_)) \<Rightarrow> (select\<^sub>P\<^sub>e\<^sub>r\<^sub>s\<^sub>o\<^sub>n\<M>\<O>\<V>\<I>\<N>\<G> (f) (person)))"
 
-(* 115 ************************************ 672 + 0 *)
+(* 116 ************************************ 679 + 0 *)
 
-(* 116 ************************************ 672 + 12 *)
+(* 117 ************************************ 679 + 12 *)
 consts dot_0_\<B>\<O>\<S>\<S> :: "(\<AA>, '\<alpha>) val \<Rightarrow> Person" ("(_) .boss")
 consts dot_0_\<B>\<O>\<S>\<S>at_pre :: "(\<AA>, '\<alpha>) val \<Rightarrow> Person" ("(_) .boss@pre")
 consts dot\<S>\<A>\<L>\<A>\<R>\<Y> :: "(\<AA>, '\<alpha>) val \<Rightarrow> (\<AA>, int option option) val" ("(_) .salary")
@@ -2732,7 +2765,7 @@ consts dot\<S>\<O>\<U>\<N>\<D>at_pre :: "(\<AA>, '\<alpha>) val \<Rightarrow> (\
 consts dot\<M>\<O>\<V>\<I>\<N>\<G> :: "(\<AA>, '\<alpha>) val \<Rightarrow> (\<AA>, bool option option) val" ("(_) .moving")
 consts dot\<M>\<O>\<V>\<I>\<N>\<G>at_pre :: "(\<AA>, '\<alpha>) val \<Rightarrow> (\<AA>, bool option option) val" ("(_) .moving@pre")
 
-(* 117 ************************************ 684 + 24 *)
+(* 118 ************************************ 691 + 24 *)
 defs(overloaded) dot\<^sub>P\<^sub>e\<^sub>r\<^sub>s\<^sub>o\<^sub>n_0_\<B>\<O>\<S>\<S> : "(x::Person) .boss \<equiv> (eval_extract (x) ((deref_oid\<^sub>P\<^sub>e\<^sub>r\<^sub>s\<^sub>o\<^sub>n (in_post_state) ((select\<^sub>P\<^sub>e\<^sub>r\<^sub>s\<^sub>o\<^sub>n\<B>\<O>\<S>\<S> ((select_object_set_any ((deref_oid\<^sub>P\<^sub>e\<^sub>r\<^sub>s\<^sub>o\<^sub>n (in_post_state))))))))))"
 defs(overloaded) dot\<^sub>P\<^sub>e\<^sub>r\<^sub>s\<^sub>o\<^sub>n\<S>\<A>\<L>\<A>\<R>\<Y> : "(x::Person) .salary \<equiv> (eval_extract (x) ((deref_oid\<^sub>P\<^sub>e\<^sub>r\<^sub>s\<^sub>o\<^sub>n (in_post_state) ((select\<^sub>P\<^sub>e\<^sub>r\<^sub>s\<^sub>o\<^sub>n\<S>\<A>\<L>\<A>\<R>\<Y> (reconst_basetype))))))"
 defs(overloaded) dot\<^sub>P\<^sub>e\<^sub>r\<^sub>s\<^sub>o\<^sub>n_0_\<B>\<O>\<S>\<S>at_pre : "(x::Person) .boss@pre \<equiv> (eval_extract (x) ((deref_oid\<^sub>P\<^sub>e\<^sub>r\<^sub>s\<^sub>o\<^sub>n (in_pre_state) ((select\<^sub>P\<^sub>e\<^sub>r\<^sub>s\<^sub>o\<^sub>n\<B>\<O>\<S>\<S> ((select_object_set_any ((deref_oid\<^sub>P\<^sub>e\<^sub>r\<^sub>s\<^sub>o\<^sub>n (in_pre_state))))))))))"
@@ -2758,8 +2791,8 @@ defs(overloaded) dot\<^sub>P\<^sub>l\<^sub>a\<^sub>n\<^sub>e\<^sub>t\<M>\<O>\<V>
 defs(overloaded) dot\<^sub>P\<^sub>l\<^sub>a\<^sub>n\<^sub>e\<^sub>t\<S>\<O>\<U>\<N>\<D>at_pre : "(x::Planet) .sound@pre \<equiv> (eval_extract (x) ((deref_oid\<^sub>P\<^sub>l\<^sub>a\<^sub>n\<^sub>e\<^sub>t (in_pre_state) ((select\<^sub>P\<^sub>l\<^sub>a\<^sub>n\<^sub>e\<^sub>t\<S>\<O>\<U>\<N>\<D> (reconst_basetype))))))"
 defs(overloaded) dot\<^sub>P\<^sub>l\<^sub>a\<^sub>n\<^sub>e\<^sub>t\<M>\<O>\<V>\<I>\<N>\<G>at_pre : "(x::Planet) .moving@pre \<equiv> (eval_extract (x) ((deref_oid\<^sub>P\<^sub>l\<^sub>a\<^sub>n\<^sub>e\<^sub>t (in_pre_state) ((select\<^sub>P\<^sub>l\<^sub>a\<^sub>n\<^sub>e\<^sub>t\<M>\<O>\<V>\<I>\<N>\<G> (reconst_basetype))))))"
 
-(* 118 ************************************ 708 + 1 *)
-lemmas [simp,code_unfold] = dot\<^sub>P\<^sub>e\<^sub>r\<^sub>s\<^sub>o\<^sub>n_0_\<B>\<O>\<S>\<S>
+(* 119 ************************************ 715 + 1 *)
+lemmas dot_accessor = dot\<^sub>P\<^sub>e\<^sub>r\<^sub>s\<^sub>o\<^sub>n_0_\<B>\<O>\<S>\<S>
                             dot\<^sub>P\<^sub>e\<^sub>r\<^sub>s\<^sub>o\<^sub>n\<S>\<A>\<L>\<A>\<R>\<Y>
                             dot\<^sub>P\<^sub>e\<^sub>r\<^sub>s\<^sub>o\<^sub>n_0_\<B>\<O>\<S>\<S>at_pre
                             dot\<^sub>P\<^sub>e\<^sub>r\<^sub>s\<^sub>o\<^sub>n\<S>\<A>\<L>\<A>\<R>\<Y>at_pre
@@ -2784,64 +2817,64 @@ lemmas [simp,code_unfold] = dot\<^sub>P\<^sub>e\<^sub>r\<^sub>s\<^sub>o\<^sub>n_
                             dot\<^sub>P\<^sub>l\<^sub>a\<^sub>n\<^sub>e\<^sub>t\<S>\<O>\<U>\<N>\<D>at_pre
                             dot\<^sub>P\<^sub>l\<^sub>a\<^sub>n\<^sub>e\<^sub>t\<M>\<O>\<V>\<I>\<N>\<G>at_pre
 
-(* 119 ************************************ 709 + 1 *)
+(* 120 ************************************ 716 + 1 *)
 subsection{* Context Passing *}
 
-(* 120 ************************************ 710 + 1 *)
-lemmas [simp,code_unfold] = eval_extract_def
+(* 121 ************************************ 717 + 1 *)
+lemmas[simp,code_unfold] = eval_extract_def
 
-(* 121 ************************************ 711 + 24 *)
+(* 122 ************************************ 718 + 24 *)
 lemma cp_dot\<^sub>P\<^sub>e\<^sub>r\<^sub>s\<^sub>o\<^sub>n_0_\<B>\<O>\<S>\<S> : "(cp ((\<lambda>X. (X::Person) .boss)))"
-by(auto simp: cp_def)
+by(auto simp: dot_accessor cp_def)
 lemma cp_dot\<^sub>P\<^sub>e\<^sub>r\<^sub>s\<^sub>o\<^sub>n\<S>\<A>\<L>\<A>\<R>\<Y> : "(cp ((\<lambda>X. (X::Person) .salary)))"
-by(auto simp: cp_def)
+by(auto simp: dot_accessor cp_def)
 lemma cp_dot\<^sub>P\<^sub>e\<^sub>r\<^sub>s\<^sub>o\<^sub>n_0_\<B>\<O>\<S>\<S>at_pre : "(cp ((\<lambda>X. (X::Person) .boss@pre)))"
-by(auto simp: cp_def)
+by(auto simp: dot_accessor cp_def)
 lemma cp_dot\<^sub>P\<^sub>e\<^sub>r\<^sub>s\<^sub>o\<^sub>n\<S>\<A>\<L>\<A>\<R>\<Y>at_pre : "(cp ((\<lambda>X. (X::Person) .salary@pre)))"
-by(auto simp: cp_def)
+by(auto simp: dot_accessor cp_def)
 lemma cp_dot\<^sub>P\<^sub>l\<^sub>a\<^sub>n\<^sub>e\<^sub>t\<W>\<O>\<R>\<M>\<H>\<O>\<L>\<E> : "(cp ((\<lambda>X. (X::Planet) .wormhole)))"
-by(auto simp: cp_def)
+by(auto simp: dot_accessor cp_def)
 lemma cp_dot\<^sub>P\<^sub>l\<^sub>a\<^sub>n\<^sub>e\<^sub>t\<W>\<E>\<I>\<G>\<H>\<T> : "(cp ((\<lambda>X. (X::Planet) .weight)))"
-by(auto simp: cp_def)
+by(auto simp: dot_accessor cp_def)
 lemma cp_dot\<^sub>P\<^sub>l\<^sub>a\<^sub>n\<^sub>e\<^sub>t\<W>\<O>\<R>\<M>\<H>\<O>\<L>\<E>at_pre : "(cp ((\<lambda>X. (X::Planet) .wormhole@pre)))"
-by(auto simp: cp_def)
+by(auto simp: dot_accessor cp_def)
 lemma cp_dot\<^sub>P\<^sub>l\<^sub>a\<^sub>n\<^sub>e\<^sub>t\<W>\<E>\<I>\<G>\<H>\<T>at_pre : "(cp ((\<lambda>X. (X::Planet) .weight@pre)))"
-by(auto simp: cp_def)
+by(auto simp: dot_accessor cp_def)
 lemma cp_dot\<^sub>G\<^sub>a\<^sub>l\<^sub>a\<^sub>x\<^sub>y\<S>\<O>\<U>\<N>\<D> : "(cp ((\<lambda>X. (X::Galaxy) .sound)))"
-by(auto simp: cp_def)
+by(auto simp: dot_accessor cp_def)
 lemma cp_dot\<^sub>G\<^sub>a\<^sub>l\<^sub>a\<^sub>x\<^sub>y\<M>\<O>\<V>\<I>\<N>\<G> : "(cp ((\<lambda>X. (X::Galaxy) .moving)))"
-by(auto simp: cp_def)
+by(auto simp: dot_accessor cp_def)
 lemma cp_dot\<^sub>G\<^sub>a\<^sub>l\<^sub>a\<^sub>x\<^sub>y\<S>\<O>\<U>\<N>\<D>at_pre : "(cp ((\<lambda>X. (X::Galaxy) .sound@pre)))"
-by(auto simp: cp_def)
+by(auto simp: dot_accessor cp_def)
 lemma cp_dot\<^sub>G\<^sub>a\<^sub>l\<^sub>a\<^sub>x\<^sub>y\<M>\<O>\<V>\<I>\<N>\<G>at_pre : "(cp ((\<lambda>X. (X::Galaxy) .moving@pre)))"
-by(auto simp: cp_def)
+by(auto simp: dot_accessor cp_def)
 lemma cp_dot\<^sub>P\<^sub>e\<^sub>r\<^sub>s\<^sub>o\<^sub>n\<W>\<O>\<R>\<M>\<H>\<O>\<L>\<E> : "(cp ((\<lambda>X. (X::Person) .wormhole)))"
-by(auto simp: cp_def)
+by(auto simp: dot_accessor cp_def)
 lemma cp_dot\<^sub>P\<^sub>e\<^sub>r\<^sub>s\<^sub>o\<^sub>n\<W>\<E>\<I>\<G>\<H>\<T> : "(cp ((\<lambda>X. (X::Person) .weight)))"
-by(auto simp: cp_def)
+by(auto simp: dot_accessor cp_def)
 lemma cp_dot\<^sub>P\<^sub>e\<^sub>r\<^sub>s\<^sub>o\<^sub>n\<S>\<O>\<U>\<N>\<D> : "(cp ((\<lambda>X. (X::Person) .sound)))"
-by(auto simp: cp_def)
+by(auto simp: dot_accessor cp_def)
 lemma cp_dot\<^sub>P\<^sub>e\<^sub>r\<^sub>s\<^sub>o\<^sub>n\<M>\<O>\<V>\<I>\<N>\<G> : "(cp ((\<lambda>X. (X::Person) .moving)))"
-by(auto simp: cp_def)
+by(auto simp: dot_accessor cp_def)
 lemma cp_dot\<^sub>P\<^sub>e\<^sub>r\<^sub>s\<^sub>o\<^sub>n\<W>\<O>\<R>\<M>\<H>\<O>\<L>\<E>at_pre : "(cp ((\<lambda>X. (X::Person) .wormhole@pre)))"
-by(auto simp: cp_def)
+by(auto simp: dot_accessor cp_def)
 lemma cp_dot\<^sub>P\<^sub>e\<^sub>r\<^sub>s\<^sub>o\<^sub>n\<W>\<E>\<I>\<G>\<H>\<T>at_pre : "(cp ((\<lambda>X. (X::Person) .weight@pre)))"
-by(auto simp: cp_def)
+by(auto simp: dot_accessor cp_def)
 lemma cp_dot\<^sub>P\<^sub>e\<^sub>r\<^sub>s\<^sub>o\<^sub>n\<S>\<O>\<U>\<N>\<D>at_pre : "(cp ((\<lambda>X. (X::Person) .sound@pre)))"
-by(auto simp: cp_def)
+by(auto simp: dot_accessor cp_def)
 lemma cp_dot\<^sub>P\<^sub>e\<^sub>r\<^sub>s\<^sub>o\<^sub>n\<M>\<O>\<V>\<I>\<N>\<G>at_pre : "(cp ((\<lambda>X. (X::Person) .moving@pre)))"
-by(auto simp: cp_def)
+by(auto simp: dot_accessor cp_def)
 lemma cp_dot\<^sub>P\<^sub>l\<^sub>a\<^sub>n\<^sub>e\<^sub>t\<S>\<O>\<U>\<N>\<D> : "(cp ((\<lambda>X. (X::Planet) .sound)))"
-by(auto simp: cp_def)
+by(auto simp: dot_accessor cp_def)
 lemma cp_dot\<^sub>P\<^sub>l\<^sub>a\<^sub>n\<^sub>e\<^sub>t\<M>\<O>\<V>\<I>\<N>\<G> : "(cp ((\<lambda>X. (X::Planet) .moving)))"
-by(auto simp: cp_def)
+by(auto simp: dot_accessor cp_def)
 lemma cp_dot\<^sub>P\<^sub>l\<^sub>a\<^sub>n\<^sub>e\<^sub>t\<S>\<O>\<U>\<N>\<D>at_pre : "(cp ((\<lambda>X. (X::Planet) .sound@pre)))"
-by(auto simp: cp_def)
+by(auto simp: dot_accessor cp_def)
 lemma cp_dot\<^sub>P\<^sub>l\<^sub>a\<^sub>n\<^sub>e\<^sub>t\<M>\<O>\<V>\<I>\<N>\<G>at_pre : "(cp ((\<lambda>X. (X::Planet) .moving@pre)))"
-by(auto simp: cp_def)
+by(auto simp: dot_accessor cp_def)
 
-(* 122 ************************************ 735 + 1 *)
-lemmas [simp,code_unfold] = cp_dot\<^sub>P\<^sub>e\<^sub>r\<^sub>s\<^sub>o\<^sub>n_0_\<B>\<O>\<S>\<S>
+(* 123 ************************************ 742 + 1 *)
+lemmas[simp,code_unfold] = cp_dot\<^sub>P\<^sub>e\<^sub>r\<^sub>s\<^sub>o\<^sub>n_0_\<B>\<O>\<S>\<S>
                             cp_dot\<^sub>P\<^sub>e\<^sub>r\<^sub>s\<^sub>o\<^sub>n\<S>\<A>\<L>\<A>\<R>\<Y>
                             cp_dot\<^sub>P\<^sub>e\<^sub>r\<^sub>s\<^sub>o\<^sub>n_0_\<B>\<O>\<S>\<S>at_pre
                             cp_dot\<^sub>P\<^sub>e\<^sub>r\<^sub>s\<^sub>o\<^sub>n\<S>\<A>\<L>\<A>\<R>\<Y>at_pre
@@ -2866,111 +2899,111 @@ lemmas [simp,code_unfold] = cp_dot\<^sub>P\<^sub>e\<^sub>r\<^sub>s\<^sub>o\<^sub
                             cp_dot\<^sub>P\<^sub>l\<^sub>a\<^sub>n\<^sub>e\<^sub>t\<S>\<O>\<U>\<N>\<D>at_pre
                             cp_dot\<^sub>P\<^sub>l\<^sub>a\<^sub>n\<^sub>e\<^sub>t\<M>\<O>\<V>\<I>\<N>\<G>at_pre
 
-(* 123 ************************************ 736 + 1 *)
+(* 124 ************************************ 743 + 1 *)
 subsection{* Execution with Invalid or Null as Argument *}
 
-(* 124 ************************************ 737 + 48 *)
+(* 125 ************************************ 744 + 48 *)
 lemma dot\<^sub>P\<^sub>e\<^sub>r\<^sub>s\<^sub>o\<^sub>n_0_\<B>\<O>\<S>\<S>_invalid : "(invalid::Person) .boss = invalid"
-by(rule ext, simp add: bot_option_def invalid_def)
+by(rule ext, simp add: dot_accessor bot_option_def invalid_def)
 lemma dot\<^sub>P\<^sub>e\<^sub>r\<^sub>s\<^sub>o\<^sub>n_0_\<B>\<O>\<S>\<S>_null : "(null::Person) .boss = invalid"
-by(rule ext, simp add: bot_option_def null_fun_def null_option_def)
+by(rule ext, simp add: dot_accessor bot_option_def null_fun_def null_option_def)
 lemma dot\<^sub>P\<^sub>e\<^sub>r\<^sub>s\<^sub>o\<^sub>n\<S>\<A>\<L>\<A>\<R>\<Y>_invalid : "(invalid::Person) .salary = invalid"
-by(rule ext, simp add: bot_option_def invalid_def)
+by(rule ext, simp add: dot_accessor bot_option_def invalid_def)
 lemma dot\<^sub>P\<^sub>e\<^sub>r\<^sub>s\<^sub>o\<^sub>n\<S>\<A>\<L>\<A>\<R>\<Y>_null : "(null::Person) .salary = invalid"
-by(rule ext, simp add: bot_option_def null_fun_def null_option_def)
+by(rule ext, simp add: dot_accessor bot_option_def null_fun_def null_option_def)
 lemma dot\<^sub>P\<^sub>e\<^sub>r\<^sub>s\<^sub>o\<^sub>n_0_\<B>\<O>\<S>\<S>at_pre_invalid : "(invalid::Person) .boss@pre = invalid"
-by(rule ext, simp add: bot_option_def invalid_def)
+by(rule ext, simp add: dot_accessor bot_option_def invalid_def)
 lemma dot\<^sub>P\<^sub>e\<^sub>r\<^sub>s\<^sub>o\<^sub>n_0_\<B>\<O>\<S>\<S>at_pre_null : "(null::Person) .boss@pre = invalid"
-by(rule ext, simp add: bot_option_def null_fun_def null_option_def)
+by(rule ext, simp add: dot_accessor bot_option_def null_fun_def null_option_def)
 lemma dot\<^sub>P\<^sub>e\<^sub>r\<^sub>s\<^sub>o\<^sub>n\<S>\<A>\<L>\<A>\<R>\<Y>at_pre_invalid : "(invalid::Person) .salary@pre = invalid"
-by(rule ext, simp add: bot_option_def invalid_def)
+by(rule ext, simp add: dot_accessor bot_option_def invalid_def)
 lemma dot\<^sub>P\<^sub>e\<^sub>r\<^sub>s\<^sub>o\<^sub>n\<S>\<A>\<L>\<A>\<R>\<Y>at_pre_null : "(null::Person) .salary@pre = invalid"
-by(rule ext, simp add: bot_option_def null_fun_def null_option_def)
+by(rule ext, simp add: dot_accessor bot_option_def null_fun_def null_option_def)
 lemma dot\<^sub>P\<^sub>l\<^sub>a\<^sub>n\<^sub>e\<^sub>t\<W>\<O>\<R>\<M>\<H>\<O>\<L>\<E>_invalid : "(invalid::Planet) .wormhole = invalid"
-by(rule ext, simp add: bot_option_def invalid_def)
+by(rule ext, simp add: dot_accessor bot_option_def invalid_def)
 lemma dot\<^sub>P\<^sub>l\<^sub>a\<^sub>n\<^sub>e\<^sub>t\<W>\<O>\<R>\<M>\<H>\<O>\<L>\<E>_null : "(null::Planet) .wormhole = invalid"
-by(rule ext, simp add: bot_option_def null_fun_def null_option_def)
+by(rule ext, simp add: dot_accessor bot_option_def null_fun_def null_option_def)
 lemma dot\<^sub>P\<^sub>l\<^sub>a\<^sub>n\<^sub>e\<^sub>t\<W>\<E>\<I>\<G>\<H>\<T>_invalid : "(invalid::Planet) .weight = invalid"
-by(rule ext, simp add: bot_option_def invalid_def)
+by(rule ext, simp add: dot_accessor bot_option_def invalid_def)
 lemma dot\<^sub>P\<^sub>l\<^sub>a\<^sub>n\<^sub>e\<^sub>t\<W>\<E>\<I>\<G>\<H>\<T>_null : "(null::Planet) .weight = invalid"
-by(rule ext, simp add: bot_option_def null_fun_def null_option_def)
+by(rule ext, simp add: dot_accessor bot_option_def null_fun_def null_option_def)
 lemma dot\<^sub>P\<^sub>l\<^sub>a\<^sub>n\<^sub>e\<^sub>t\<W>\<O>\<R>\<M>\<H>\<O>\<L>\<E>at_pre_invalid : "(invalid::Planet) .wormhole@pre = invalid"
-by(rule ext, simp add: bot_option_def invalid_def)
+by(rule ext, simp add: dot_accessor bot_option_def invalid_def)
 lemma dot\<^sub>P\<^sub>l\<^sub>a\<^sub>n\<^sub>e\<^sub>t\<W>\<O>\<R>\<M>\<H>\<O>\<L>\<E>at_pre_null : "(null::Planet) .wormhole@pre = invalid"
-by(rule ext, simp add: bot_option_def null_fun_def null_option_def)
+by(rule ext, simp add: dot_accessor bot_option_def null_fun_def null_option_def)
 lemma dot\<^sub>P\<^sub>l\<^sub>a\<^sub>n\<^sub>e\<^sub>t\<W>\<E>\<I>\<G>\<H>\<T>at_pre_invalid : "(invalid::Planet) .weight@pre = invalid"
-by(rule ext, simp add: bot_option_def invalid_def)
+by(rule ext, simp add: dot_accessor bot_option_def invalid_def)
 lemma dot\<^sub>P\<^sub>l\<^sub>a\<^sub>n\<^sub>e\<^sub>t\<W>\<E>\<I>\<G>\<H>\<T>at_pre_null : "(null::Planet) .weight@pre = invalid"
-by(rule ext, simp add: bot_option_def null_fun_def null_option_def)
+by(rule ext, simp add: dot_accessor bot_option_def null_fun_def null_option_def)
 lemma dot\<^sub>G\<^sub>a\<^sub>l\<^sub>a\<^sub>x\<^sub>y\<S>\<O>\<U>\<N>\<D>_invalid : "(invalid::Galaxy) .sound = invalid"
-by(rule ext, simp add: bot_option_def invalid_def)
+by(rule ext, simp add: dot_accessor bot_option_def invalid_def)
 lemma dot\<^sub>G\<^sub>a\<^sub>l\<^sub>a\<^sub>x\<^sub>y\<S>\<O>\<U>\<N>\<D>_null : "(null::Galaxy) .sound = invalid"
-by(rule ext, simp add: bot_option_def null_fun_def null_option_def)
+by(rule ext, simp add: dot_accessor bot_option_def null_fun_def null_option_def)
 lemma dot\<^sub>G\<^sub>a\<^sub>l\<^sub>a\<^sub>x\<^sub>y\<M>\<O>\<V>\<I>\<N>\<G>_invalid : "(invalid::Galaxy) .moving = invalid"
-by(rule ext, simp add: bot_option_def invalid_def)
+by(rule ext, simp add: dot_accessor bot_option_def invalid_def)
 lemma dot\<^sub>G\<^sub>a\<^sub>l\<^sub>a\<^sub>x\<^sub>y\<M>\<O>\<V>\<I>\<N>\<G>_null : "(null::Galaxy) .moving = invalid"
-by(rule ext, simp add: bot_option_def null_fun_def null_option_def)
+by(rule ext, simp add: dot_accessor bot_option_def null_fun_def null_option_def)
 lemma dot\<^sub>G\<^sub>a\<^sub>l\<^sub>a\<^sub>x\<^sub>y\<S>\<O>\<U>\<N>\<D>at_pre_invalid : "(invalid::Galaxy) .sound@pre = invalid"
-by(rule ext, simp add: bot_option_def invalid_def)
+by(rule ext, simp add: dot_accessor bot_option_def invalid_def)
 lemma dot\<^sub>G\<^sub>a\<^sub>l\<^sub>a\<^sub>x\<^sub>y\<S>\<O>\<U>\<N>\<D>at_pre_null : "(null::Galaxy) .sound@pre = invalid"
-by(rule ext, simp add: bot_option_def null_fun_def null_option_def)
+by(rule ext, simp add: dot_accessor bot_option_def null_fun_def null_option_def)
 lemma dot\<^sub>G\<^sub>a\<^sub>l\<^sub>a\<^sub>x\<^sub>y\<M>\<O>\<V>\<I>\<N>\<G>at_pre_invalid : "(invalid::Galaxy) .moving@pre = invalid"
-by(rule ext, simp add: bot_option_def invalid_def)
+by(rule ext, simp add: dot_accessor bot_option_def invalid_def)
 lemma dot\<^sub>G\<^sub>a\<^sub>l\<^sub>a\<^sub>x\<^sub>y\<M>\<O>\<V>\<I>\<N>\<G>at_pre_null : "(null::Galaxy) .moving@pre = invalid"
-by(rule ext, simp add: bot_option_def null_fun_def null_option_def)
+by(rule ext, simp add: dot_accessor bot_option_def null_fun_def null_option_def)
 lemma dot\<^sub>P\<^sub>e\<^sub>r\<^sub>s\<^sub>o\<^sub>n\<W>\<O>\<R>\<M>\<H>\<O>\<L>\<E>_invalid : "(invalid::Person) .wormhole = invalid"
-by(rule ext, simp add: bot_option_def invalid_def)
+by(rule ext, simp add: dot_accessor bot_option_def invalid_def)
 lemma dot\<^sub>P\<^sub>e\<^sub>r\<^sub>s\<^sub>o\<^sub>n\<W>\<O>\<R>\<M>\<H>\<O>\<L>\<E>_null : "(null::Person) .wormhole = invalid"
-by(rule ext, simp add: bot_option_def null_fun_def null_option_def)
+by(rule ext, simp add: dot_accessor bot_option_def null_fun_def null_option_def)
 lemma dot\<^sub>P\<^sub>e\<^sub>r\<^sub>s\<^sub>o\<^sub>n\<W>\<E>\<I>\<G>\<H>\<T>_invalid : "(invalid::Person) .weight = invalid"
-by(rule ext, simp add: bot_option_def invalid_def)
+by(rule ext, simp add: dot_accessor bot_option_def invalid_def)
 lemma dot\<^sub>P\<^sub>e\<^sub>r\<^sub>s\<^sub>o\<^sub>n\<W>\<E>\<I>\<G>\<H>\<T>_null : "(null::Person) .weight = invalid"
-by(rule ext, simp add: bot_option_def null_fun_def null_option_def)
+by(rule ext, simp add: dot_accessor bot_option_def null_fun_def null_option_def)
 lemma dot\<^sub>P\<^sub>e\<^sub>r\<^sub>s\<^sub>o\<^sub>n\<S>\<O>\<U>\<N>\<D>_invalid : "(invalid::Person) .sound = invalid"
-by(rule ext, simp add: bot_option_def invalid_def)
+by(rule ext, simp add: dot_accessor bot_option_def invalid_def)
 lemma dot\<^sub>P\<^sub>e\<^sub>r\<^sub>s\<^sub>o\<^sub>n\<S>\<O>\<U>\<N>\<D>_null : "(null::Person) .sound = invalid"
-by(rule ext, simp add: bot_option_def null_fun_def null_option_def)
+by(rule ext, simp add: dot_accessor bot_option_def null_fun_def null_option_def)
 lemma dot\<^sub>P\<^sub>e\<^sub>r\<^sub>s\<^sub>o\<^sub>n\<M>\<O>\<V>\<I>\<N>\<G>_invalid : "(invalid::Person) .moving = invalid"
-by(rule ext, simp add: bot_option_def invalid_def)
+by(rule ext, simp add: dot_accessor bot_option_def invalid_def)
 lemma dot\<^sub>P\<^sub>e\<^sub>r\<^sub>s\<^sub>o\<^sub>n\<M>\<O>\<V>\<I>\<N>\<G>_null : "(null::Person) .moving = invalid"
-by(rule ext, simp add: bot_option_def null_fun_def null_option_def)
+by(rule ext, simp add: dot_accessor bot_option_def null_fun_def null_option_def)
 lemma dot\<^sub>P\<^sub>e\<^sub>r\<^sub>s\<^sub>o\<^sub>n\<W>\<O>\<R>\<M>\<H>\<O>\<L>\<E>at_pre_invalid : "(invalid::Person) .wormhole@pre = invalid"
-by(rule ext, simp add: bot_option_def invalid_def)
+by(rule ext, simp add: dot_accessor bot_option_def invalid_def)
 lemma dot\<^sub>P\<^sub>e\<^sub>r\<^sub>s\<^sub>o\<^sub>n\<W>\<O>\<R>\<M>\<H>\<O>\<L>\<E>at_pre_null : "(null::Person) .wormhole@pre = invalid"
-by(rule ext, simp add: bot_option_def null_fun_def null_option_def)
+by(rule ext, simp add: dot_accessor bot_option_def null_fun_def null_option_def)
 lemma dot\<^sub>P\<^sub>e\<^sub>r\<^sub>s\<^sub>o\<^sub>n\<W>\<E>\<I>\<G>\<H>\<T>at_pre_invalid : "(invalid::Person) .weight@pre = invalid"
-by(rule ext, simp add: bot_option_def invalid_def)
+by(rule ext, simp add: dot_accessor bot_option_def invalid_def)
 lemma dot\<^sub>P\<^sub>e\<^sub>r\<^sub>s\<^sub>o\<^sub>n\<W>\<E>\<I>\<G>\<H>\<T>at_pre_null : "(null::Person) .weight@pre = invalid"
-by(rule ext, simp add: bot_option_def null_fun_def null_option_def)
+by(rule ext, simp add: dot_accessor bot_option_def null_fun_def null_option_def)
 lemma dot\<^sub>P\<^sub>e\<^sub>r\<^sub>s\<^sub>o\<^sub>n\<S>\<O>\<U>\<N>\<D>at_pre_invalid : "(invalid::Person) .sound@pre = invalid"
-by(rule ext, simp add: bot_option_def invalid_def)
+by(rule ext, simp add: dot_accessor bot_option_def invalid_def)
 lemma dot\<^sub>P\<^sub>e\<^sub>r\<^sub>s\<^sub>o\<^sub>n\<S>\<O>\<U>\<N>\<D>at_pre_null : "(null::Person) .sound@pre = invalid"
-by(rule ext, simp add: bot_option_def null_fun_def null_option_def)
+by(rule ext, simp add: dot_accessor bot_option_def null_fun_def null_option_def)
 lemma dot\<^sub>P\<^sub>e\<^sub>r\<^sub>s\<^sub>o\<^sub>n\<M>\<O>\<V>\<I>\<N>\<G>at_pre_invalid : "(invalid::Person) .moving@pre = invalid"
-by(rule ext, simp add: bot_option_def invalid_def)
+by(rule ext, simp add: dot_accessor bot_option_def invalid_def)
 lemma dot\<^sub>P\<^sub>e\<^sub>r\<^sub>s\<^sub>o\<^sub>n\<M>\<O>\<V>\<I>\<N>\<G>at_pre_null : "(null::Person) .moving@pre = invalid"
-by(rule ext, simp add: bot_option_def null_fun_def null_option_def)
+by(rule ext, simp add: dot_accessor bot_option_def null_fun_def null_option_def)
 lemma dot\<^sub>P\<^sub>l\<^sub>a\<^sub>n\<^sub>e\<^sub>t\<S>\<O>\<U>\<N>\<D>_invalid : "(invalid::Planet) .sound = invalid"
-by(rule ext, simp add: bot_option_def invalid_def)
+by(rule ext, simp add: dot_accessor bot_option_def invalid_def)
 lemma dot\<^sub>P\<^sub>l\<^sub>a\<^sub>n\<^sub>e\<^sub>t\<S>\<O>\<U>\<N>\<D>_null : "(null::Planet) .sound = invalid"
-by(rule ext, simp add: bot_option_def null_fun_def null_option_def)
+by(rule ext, simp add: dot_accessor bot_option_def null_fun_def null_option_def)
 lemma dot\<^sub>P\<^sub>l\<^sub>a\<^sub>n\<^sub>e\<^sub>t\<M>\<O>\<V>\<I>\<N>\<G>_invalid : "(invalid::Planet) .moving = invalid"
-by(rule ext, simp add: bot_option_def invalid_def)
+by(rule ext, simp add: dot_accessor bot_option_def invalid_def)
 lemma dot\<^sub>P\<^sub>l\<^sub>a\<^sub>n\<^sub>e\<^sub>t\<M>\<O>\<V>\<I>\<N>\<G>_null : "(null::Planet) .moving = invalid"
-by(rule ext, simp add: bot_option_def null_fun_def null_option_def)
+by(rule ext, simp add: dot_accessor bot_option_def null_fun_def null_option_def)
 lemma dot\<^sub>P\<^sub>l\<^sub>a\<^sub>n\<^sub>e\<^sub>t\<S>\<O>\<U>\<N>\<D>at_pre_invalid : "(invalid::Planet) .sound@pre = invalid"
-by(rule ext, simp add: bot_option_def invalid_def)
+by(rule ext, simp add: dot_accessor bot_option_def invalid_def)
 lemma dot\<^sub>P\<^sub>l\<^sub>a\<^sub>n\<^sub>e\<^sub>t\<S>\<O>\<U>\<N>\<D>at_pre_null : "(null::Planet) .sound@pre = invalid"
-by(rule ext, simp add: bot_option_def null_fun_def null_option_def)
+by(rule ext, simp add: dot_accessor bot_option_def null_fun_def null_option_def)
 lemma dot\<^sub>P\<^sub>l\<^sub>a\<^sub>n\<^sub>e\<^sub>t\<M>\<O>\<V>\<I>\<N>\<G>at_pre_invalid : "(invalid::Planet) .moving@pre = invalid"
-by(rule ext, simp add: bot_option_def invalid_def)
+by(rule ext, simp add: dot_accessor bot_option_def invalid_def)
 lemma dot\<^sub>P\<^sub>l\<^sub>a\<^sub>n\<^sub>e\<^sub>t\<M>\<O>\<V>\<I>\<N>\<G>at_pre_null : "(null::Planet) .moving@pre = invalid"
-by(rule ext, simp add: bot_option_def null_fun_def null_option_def)
+by(rule ext, simp add: dot_accessor bot_option_def null_fun_def null_option_def)
 
-(* 125 ************************************ 785 + 1 *)
+(* 126 ************************************ 792 + 1 *)
 section{* A Little Infra-structure on Example States *}
 
-(* 126 ************************************ 786 + 1 *)
+(* 127 ************************************ 793 + 1 *)
 text{* 
 
 The example we are defining in this section comes from the figure~\ref{fig:edm1_system-states}.
@@ -2982,15 +3015,15 @@ The example we are defining in this section comes from the figure~\ref{fig:edm1_
 \end{figure}
  *}
 
-(* 127 ************************************ 787 + 1 *)
+(* 128 ************************************ 794 + 1 *)
 text{*  *}
 
-(* 128 ************************************ 788 + 1 *)
+(* 129 ************************************ 795 + 1 *)
 lemmas [simp,code_unfold] = state.defs
                             const_ss
 
-(* 129 ************************************ 789 + 1 *)
-lemmas [simp,code_unfold] = OclAsType\<^sub>P\<^sub>e\<^sub>r\<^sub>s\<^sub>o\<^sub>n_Planet
+(* 130 ************************************ 796 + 1 *)
+lemmas[simp,code_unfold] = OclAsType\<^sub>P\<^sub>e\<^sub>r\<^sub>s\<^sub>o\<^sub>n_Planet
                             OclAsType\<^sub>P\<^sub>e\<^sub>r\<^sub>s\<^sub>o\<^sub>n_Galaxy
                             OclAsType\<^sub>P\<^sub>e\<^sub>r\<^sub>s\<^sub>o\<^sub>n_OclAny
                             OclAsType\<^sub>P\<^sub>l\<^sub>a\<^sub>n\<^sub>e\<^sub>t_Galaxy
@@ -3003,25 +3036,7 @@ lemmas [simp,code_unfold] = OclAsType\<^sub>P\<^sub>e\<^sub>r\<^sub>s\<^sub>o\<^
                             OclAsType\<^sub>O\<^sub>c\<^sub>l\<^sub>A\<^sub>n\<^sub>y_Planet
                             OclAsType\<^sub>O\<^sub>c\<^sub>l\<^sub>A\<^sub>n\<^sub>y_Galaxy
 
-(* 130 ************************************ 790 + 8 *)
-definition OclInt1000 ("\<one>\<zero>\<zero>\<zero>")
-  where "OclInt1000 = (\<lambda>_. \<lfloor>\<lfloor>1000\<rfloor>\<rfloor>)"
-definition OclInt1200 ("\<one>\<two>\<zero>\<zero>")
-  where "OclInt1200 = (\<lambda>_. \<lfloor>\<lfloor>1200\<rfloor>\<rfloor>)"
-definition OclInt1300 ("\<one>\<three>\<zero>\<zero>")
-  where "OclInt1300 = (\<lambda>_. \<lfloor>\<lfloor>1300\<rfloor>\<rfloor>)"
-definition OclInt1800 ("\<one>\<eight>\<zero>\<zero>")
-  where "OclInt1800 = (\<lambda>_. \<lfloor>\<lfloor>1800\<rfloor>\<rfloor>)"
-definition OclInt2600 ("\<two>\<six>\<zero>\<zero>")
-  where "OclInt2600 = (\<lambda>_. \<lfloor>\<lfloor>2600\<rfloor>\<rfloor>)"
-definition OclInt2900 ("\<two>\<nine>\<zero>\<zero>")
-  where "OclInt2900 = (\<lambda>_. \<lfloor>\<lfloor>2900\<rfloor>\<rfloor>)"
-definition OclInt3200 ("\<three>\<two>\<zero>\<zero>")
-  where "OclInt3200 = (\<lambda>_. \<lfloor>\<lfloor>3200\<rfloor>\<rfloor>)"
-definition OclInt3500 ("\<three>\<five>\<zero>\<zero>")
-  where "OclInt3500 = (\<lambda>_. \<lfloor>\<lfloor>3500\<rfloor>\<rfloor>)"
-
-(* 131 ************************************ 798 + 10 *)
+(* 131 ************************************ 797 + 10 *)
 definition "oid1 = 1"
 definition "oid2 = 2"
 definition "oid3 = 3"
@@ -3034,7 +3049,7 @@ definition "oid9 = 9"
 definition "inst_assoc1 = (\<lambda>oid_class to_from oid. ((case (deref_assocs_list ((to_from::oid list list \<Rightarrow> oid list \<times> oid list)) ((oid::oid)) ((drop ((((map_of_list ([(oid\<^sub>P\<^sub>e\<^sub>r\<^sub>s\<^sub>o\<^sub>n_0_\<B>\<O>\<S>\<S> , (List.map ((\<lambda>(x , y). [x , y]) o switch\<^sub>2_01) ([[[oid7] , [oid7]] , [[oid6] , [oid7]] , [[oid2] , [oid2]] , [[oid1] , [oid2]]])))]))) ((oid_class::oid))))))) of Nil \<Rightarrow> None
     | l \<Rightarrow> (Some (l)))::oid list option))"
 
-(* 132 ************************************ 808 + 18 *)
+(* 132 ************************************ 807 + 18 *)
 definition "X\<^sub>P\<^sub>e\<^sub>r\<^sub>s\<^sub>o\<^sub>n1\<^sub>P\<^sub>e\<^sub>r\<^sub>s\<^sub>o\<^sub>n inst_assoc = (mkoid\<^sub>P\<^sub>e\<^sub>r\<^sub>s\<^sub>o\<^sub>n ((mk\<^sub>P\<^sub>e\<^sub>r\<^sub>s\<^sub>o\<^sub>n (oid1) (None) (None) (None) (None))) (((inst_assoc) (oid\<^sub>P\<^sub>e\<^sub>r\<^sub>s\<^sub>o\<^sub>n_0_\<B>\<O>\<S>\<S>) (switch\<^sub>2_01) (oid1))) (\<lfloor>1300\<rfloor>))"
 definition "X\<^sub>P\<^sub>e\<^sub>r\<^sub>s\<^sub>o\<^sub>n2\<^sub>P\<^sub>e\<^sub>r\<^sub>s\<^sub>o\<^sub>n inst_assoc = (mkoid\<^sub>P\<^sub>e\<^sub>r\<^sub>s\<^sub>o\<^sub>n ((mk\<^sub>P\<^sub>e\<^sub>r\<^sub>s\<^sub>o\<^sub>n (oid2) (None) (None) (None) (None))) (((inst_assoc) (oid\<^sub>P\<^sub>e\<^sub>r\<^sub>s\<^sub>o\<^sub>n_0_\<B>\<O>\<S>\<S>) (switch\<^sub>2_01) (oid2))) (\<lfloor>1800\<rfloor>))"
 definition "X\<^sub>P\<^sub>e\<^sub>r\<^sub>s\<^sub>o\<^sub>n3\<^sub>P\<^sub>e\<^sub>r\<^sub>s\<^sub>o\<^sub>n inst_assoc = (mkoid\<^sub>P\<^sub>e\<^sub>r\<^sub>s\<^sub>o\<^sub>n ((mk\<^sub>P\<^sub>e\<^sub>r\<^sub>s\<^sub>o\<^sub>n (oid3) (None) (None) (None) (None))) (((inst_assoc) (oid\<^sub>P\<^sub>e\<^sub>r\<^sub>s\<^sub>o\<^sub>n_0_\<B>\<O>\<S>\<S>) (switch\<^sub>2_01) (oid3))) (None))"
@@ -3054,28 +3069,28 @@ definition "(X\<^sub>P\<^sub>e\<^sub>r\<^sub>s\<^sub>o\<^sub>n7::OclAny) = (\<la
 definition "(X\<^sub>P\<^sub>e\<^sub>r\<^sub>s\<^sub>o\<^sub>n8::OclAny) = (\<lambda>_. \<lfloor>\<lfloor>(X\<^sub>P\<^sub>e\<^sub>r\<^sub>s\<^sub>o\<^sub>n8\<^sub>O\<^sub>c\<^sub>l\<^sub>A\<^sub>n\<^sub>y (inst_assoc1))\<rfloor>\<rfloor>)"
 definition "(X\<^sub>P\<^sub>e\<^sub>r\<^sub>s\<^sub>o\<^sub>n9::Person) = (\<lambda>_. \<lfloor>\<lfloor>(X\<^sub>P\<^sub>e\<^sub>r\<^sub>s\<^sub>o\<^sub>n9\<^sub>P\<^sub>e\<^sub>r\<^sub>s\<^sub>o\<^sub>n (inst_assoc1))\<rfloor>\<rfloor>)"
 
-(* 133 ************************************ 826 + 1 *)
+(* 133 ************************************ 825 + 1 *)
 ML{* (Ty'.check ([(OCL.Writeln , "X\<^sub>P\<^sub>e\<^sub>r\<^sub>s\<^sub>o\<^sub>n1 .boss = Set{ X\<^sub>P\<^sub>e\<^sub>r\<^sub>s\<^sub>o\<^sub>n2 }") , (OCL.Writeln , "X\<^sub>P\<^sub>e\<^sub>r\<^sub>s\<^sub>o\<^sub>n1 /* unnamed attribute */ = Set{}") , (OCL.Writeln , "X\<^sub>P\<^sub>e\<^sub>r\<^sub>s\<^sub>o\<^sub>n2 .boss = Set{ X\<^sub>P\<^sub>e\<^sub>r\<^sub>s\<^sub>o\<^sub>n2 }") , (OCL.Writeln , "X\<^sub>P\<^sub>e\<^sub>r\<^sub>s\<^sub>o\<^sub>n2 /* unnamed attribute */ = Set{ X\<^sub>P\<^sub>e\<^sub>r\<^sub>s\<^sub>o\<^sub>n1 , X\<^sub>P\<^sub>e\<^sub>r\<^sub>s\<^sub>o\<^sub>n2 }") , (OCL.Writeln , "X\<^sub>P\<^sub>e\<^sub>r\<^sub>s\<^sub>o\<^sub>n3 .boss = Set{}") , (OCL.Writeln , "X\<^sub>P\<^sub>e\<^sub>r\<^sub>s\<^sub>o\<^sub>n3 /* unnamed attribute */ = Set{}") , (OCL.Writeln , "X\<^sub>P\<^sub>e\<^sub>r\<^sub>s\<^sub>o\<^sub>n4 .boss = Set{}") , (OCL.Writeln , "X\<^sub>P\<^sub>e\<^sub>r\<^sub>s\<^sub>o\<^sub>n4 /* unnamed attribute */ = Set{}") , (OCL.Writeln , "X\<^sub>P\<^sub>e\<^sub>r\<^sub>s\<^sub>o\<^sub>n5 .boss = Set{}") , (OCL.Writeln , "X\<^sub>P\<^sub>e\<^sub>r\<^sub>s\<^sub>o\<^sub>n5 /* unnamed attribute */ = Set{}") , (OCL.Writeln , "X\<^sub>P\<^sub>e\<^sub>r\<^sub>s\<^sub>o\<^sub>n6 .boss = Set{ X\<^sub>P\<^sub>e\<^sub>r\<^sub>s\<^sub>o\<^sub>n7 }") , (OCL.Writeln , "X\<^sub>P\<^sub>e\<^sub>r\<^sub>s\<^sub>o\<^sub>n6 /* unnamed attribute */ = Set{}") , (OCL.Writeln , "X\<^sub>P\<^sub>e\<^sub>r\<^sub>s\<^sub>o\<^sub>n7 .boss = Set{ X\<^sub>P\<^sub>e\<^sub>r\<^sub>s\<^sub>o\<^sub>n7 }") , (OCL.Writeln , "X\<^sub>P\<^sub>e\<^sub>r\<^sub>s\<^sub>o\<^sub>n7 /* unnamed attribute */ = Set{ X\<^sub>P\<^sub>e\<^sub>r\<^sub>s\<^sub>o\<^sub>n6 , X\<^sub>P\<^sub>e\<^sub>r\<^sub>s\<^sub>o\<^sub>n7 }") , (OCL.Writeln , "X\<^sub>P\<^sub>e\<^sub>r\<^sub>s\<^sub>o\<^sub>n9 .boss = Set{}") , (OCL.Writeln , "X\<^sub>P\<^sub>e\<^sub>r\<^sub>s\<^sub>o\<^sub>n9 /* unnamed attribute */ = Set{}")]) (" error(s) in multiplicity constraints")) *}
 
-(* 134 ************************************ 827 + 1 *)
+(* 134 ************************************ 826 + 1 *)
 definition "inst_assoc\<sigma>\<^sub>1 = (\<lambda>oid_class to_from oid. ((case (deref_assocs_list ((to_from::oid list list \<Rightarrow> oid list \<times> oid list)) ((oid::oid)) ((drop ((((map_of_list ([(oid\<^sub>P\<^sub>e\<^sub>r\<^sub>s\<^sub>o\<^sub>n_0_\<B>\<O>\<S>\<S> , (List.map ((\<lambda>(x , y). [x , y]) o switch\<^sub>2_01) ([[[oid6] , [oid4]] , [[oid4] , [oid5]] , [[oid1] , [oid2]]])))]))) ((oid_class::oid))))))) of Nil \<Rightarrow> None
     | l \<Rightarrow> (Some (l)))::oid list option))"
 
-(* 135 ************************************ 828 + 1 *)
+(* 135 ************************************ 827 + 1 *)
 definition "\<sigma>\<^sub>1 = (state.make ((Map.empty (oid1 \<mapsto> (in\<^sub>P\<^sub>e\<^sub>r\<^sub>s\<^sub>o\<^sub>n ((mkoid\<^sub>P\<^sub>e\<^sub>r\<^sub>s\<^sub>o\<^sub>n ((mk\<^sub>P\<^sub>e\<^sub>r\<^sub>s\<^sub>o\<^sub>n (oid1) (None) (None) (None) (None))) (((inst_assoc\<sigma>\<^sub>1) (oid\<^sub>P\<^sub>e\<^sub>r\<^sub>s\<^sub>o\<^sub>n_0_\<B>\<O>\<S>\<S>) (switch\<^sub>2_01) (oid1))) (\<lfloor>1000\<rfloor>))))) (oid2 \<mapsto> (in\<^sub>P\<^sub>e\<^sub>r\<^sub>s\<^sub>o\<^sub>n ((mkoid\<^sub>P\<^sub>e\<^sub>r\<^sub>s\<^sub>o\<^sub>n ((mk\<^sub>P\<^sub>e\<^sub>r\<^sub>s\<^sub>o\<^sub>n (oid2) (None) (None) (None) (None))) (((inst_assoc\<sigma>\<^sub>1) (oid\<^sub>P\<^sub>e\<^sub>r\<^sub>s\<^sub>o\<^sub>n_0_\<B>\<O>\<S>\<S>) (switch\<^sub>2_01) (oid2))) (\<lfloor>1200\<rfloor>))))) (oid4 \<mapsto> (in\<^sub>P\<^sub>e\<^sub>r\<^sub>s\<^sub>o\<^sub>n ((mkoid\<^sub>P\<^sub>e\<^sub>r\<^sub>s\<^sub>o\<^sub>n ((mk\<^sub>P\<^sub>e\<^sub>r\<^sub>s\<^sub>o\<^sub>n (oid4) (None) (None) (None) (None))) (((inst_assoc\<sigma>\<^sub>1) (oid\<^sub>P\<^sub>e\<^sub>r\<^sub>s\<^sub>o\<^sub>n_0_\<B>\<O>\<S>\<S>) (switch\<^sub>2_01) (oid4))) (\<lfloor>2600\<rfloor>))))) (oid5 \<mapsto> (in\<^sub>P\<^sub>e\<^sub>r\<^sub>s\<^sub>o\<^sub>n ((X\<^sub>P\<^sub>e\<^sub>r\<^sub>s\<^sub>o\<^sub>n5\<^sub>P\<^sub>e\<^sub>r\<^sub>s\<^sub>o\<^sub>n (inst_assoc\<sigma>\<^sub>1))))) (oid6 \<mapsto> (in\<^sub>P\<^sub>e\<^sub>r\<^sub>s\<^sub>o\<^sub>n ((mkoid\<^sub>P\<^sub>e\<^sub>r\<^sub>s\<^sub>o\<^sub>n ((mk\<^sub>P\<^sub>e\<^sub>r\<^sub>s\<^sub>o\<^sub>n (oid6) (None) (None) (None) (None))) (((inst_assoc\<sigma>\<^sub>1) (oid\<^sub>P\<^sub>e\<^sub>r\<^sub>s\<^sub>o\<^sub>n_0_\<B>\<O>\<S>\<S>) (switch\<^sub>2_01) (oid6))) (\<lfloor>2300\<rfloor>))))) (oid9 \<mapsto> (in\<^sub>P\<^sub>e\<^sub>r\<^sub>s\<^sub>o\<^sub>n ((X\<^sub>P\<^sub>e\<^sub>r\<^sub>s\<^sub>o\<^sub>n9\<^sub>P\<^sub>e\<^sub>r\<^sub>s\<^sub>o\<^sub>n (inst_assoc\<sigma>\<^sub>1))))))) (Map.empty))"
 
-(* 136 ************************************ 829 + 2 *)
+(* 136 ************************************ 828 + 2 *)
 definition "(X\<^sub>P\<^sub>e\<^sub>r\<^sub>s\<^sub>o\<^sub>n5\<sigma>\<^sub>1::Person) = (\<lambda>_. \<lfloor>\<lfloor>(X\<^sub>P\<^sub>e\<^sub>r\<^sub>s\<^sub>o\<^sub>n5\<^sub>P\<^sub>e\<^sub>r\<^sub>s\<^sub>o\<^sub>n (inst_assoc\<sigma>\<^sub>1))\<rfloor>\<rfloor>)"
 definition "(X\<^sub>P\<^sub>e\<^sub>r\<^sub>s\<^sub>o\<^sub>n9\<sigma>\<^sub>1::Person) = (\<lambda>_. \<lfloor>\<lfloor>(X\<^sub>P\<^sub>e\<^sub>r\<^sub>s\<^sub>o\<^sub>n9\<^sub>P\<^sub>e\<^sub>r\<^sub>s\<^sub>o\<^sub>n (inst_assoc\<sigma>\<^sub>1))\<rfloor>\<rfloor>)"
 
-(* 137 ************************************ 831 + 1 *)
+(* 137 ************************************ 830 + 1 *)
 lemma dom_\<sigma>\<^sub>1 : "(dom ((heap (\<sigma>\<^sub>1)))) = {oid1 , oid2 , oid4 , oid5 , oid6 , oid9}"
 by(auto simp: \<sigma>\<^sub>1_def)
 
-(* 138 ************************************ 832 + 1 *)
-lemmas [simp,code_unfold] = dom_\<sigma>\<^sub>1
+(* 138 ************************************ 831 + 1 *)
+lemmas[simp,code_unfold] = dom_\<sigma>\<^sub>1
 
-(* 139 ************************************ 833 + 1 *)
+(* 139 ************************************ 832 + 1 *)
 lemma perm_\<sigma>\<^sub>1 : "\<sigma>\<^sub>1 = (state.make ((Map.empty (oid9 \<mapsto> (in\<^sub>P\<^sub>e\<^sub>r\<^sub>s\<^sub>o\<^sub>n ((X\<^sub>P\<^sub>e\<^sub>r\<^sub>s\<^sub>o\<^sub>n9\<^sub>P\<^sub>e\<^sub>r\<^sub>s\<^sub>o\<^sub>n (inst_assoc\<sigma>\<^sub>1))))) (oid6 \<mapsto> (in\<^sub>P\<^sub>e\<^sub>r\<^sub>s\<^sub>o\<^sub>n ((mkoid\<^sub>P\<^sub>e\<^sub>r\<^sub>s\<^sub>o\<^sub>n ((mk\<^sub>P\<^sub>e\<^sub>r\<^sub>s\<^sub>o\<^sub>n (oid6) (None) (None) (None) (None))) (((inst_assoc\<sigma>\<^sub>1) (oid\<^sub>P\<^sub>e\<^sub>r\<^sub>s\<^sub>o\<^sub>n_0_\<B>\<O>\<S>\<S>) (switch\<^sub>2_01) (oid6))) (\<lfloor>2300\<rfloor>))))) (oid5 \<mapsto> (in\<^sub>P\<^sub>e\<^sub>r\<^sub>s\<^sub>o\<^sub>n ((X\<^sub>P\<^sub>e\<^sub>r\<^sub>s\<^sub>o\<^sub>n5\<^sub>P\<^sub>e\<^sub>r\<^sub>s\<^sub>o\<^sub>n (inst_assoc\<sigma>\<^sub>1))))) (oid4 \<mapsto> (in\<^sub>P\<^sub>e\<^sub>r\<^sub>s\<^sub>o\<^sub>n ((mkoid\<^sub>P\<^sub>e\<^sub>r\<^sub>s\<^sub>o\<^sub>n ((mk\<^sub>P\<^sub>e\<^sub>r\<^sub>s\<^sub>o\<^sub>n (oid4) (None) (None) (None) (None))) (((inst_assoc\<sigma>\<^sub>1) (oid\<^sub>P\<^sub>e\<^sub>r\<^sub>s\<^sub>o\<^sub>n_0_\<B>\<O>\<S>\<S>) (switch\<^sub>2_01) (oid4))) (\<lfloor>2600\<rfloor>))))) (oid2 \<mapsto> (in\<^sub>P\<^sub>e\<^sub>r\<^sub>s\<^sub>o\<^sub>n ((mkoid\<^sub>P\<^sub>e\<^sub>r\<^sub>s\<^sub>o\<^sub>n ((mk\<^sub>P\<^sub>e\<^sub>r\<^sub>s\<^sub>o\<^sub>n (oid2) (None) (None) (None) (None))) (((inst_assoc\<sigma>\<^sub>1) (oid\<^sub>P\<^sub>e\<^sub>r\<^sub>s\<^sub>o\<^sub>n_0_\<B>\<O>\<S>\<S>) (switch\<^sub>2_01) (oid2))) (\<lfloor>1200\<rfloor>))))) (oid1 \<mapsto> (in\<^sub>P\<^sub>e\<^sub>r\<^sub>s\<^sub>o\<^sub>n ((mkoid\<^sub>P\<^sub>e\<^sub>r\<^sub>s\<^sub>o\<^sub>n ((mk\<^sub>P\<^sub>e\<^sub>r\<^sub>s\<^sub>o\<^sub>n (oid1) (None) (None) (None) (None))) (((inst_assoc\<sigma>\<^sub>1) (oid\<^sub>P\<^sub>e\<^sub>r\<^sub>s\<^sub>o\<^sub>n_0_\<B>\<O>\<S>\<S>) (switch\<^sub>2_01) (oid1))) (\<lfloor>1000\<rfloor>))))))) ((assocs (\<sigma>\<^sub>1))))"
   apply(simp add: \<sigma>\<^sub>1_def oid1_def oid2_def oid4_def oid5_def oid6_def oid9_def)
   apply(subst (1) fun_upd_twist, simp)
@@ -3095,7 +3110,7 @@ lemma perm_\<sigma>\<^sub>1 : "\<sigma>\<^sub>1 = (state.make ((Map.empty (oid9 
   apply(subst (1) fun_upd_twist, simp)
 by(simp)
 
-(* 140 ************************************ 834 + 12 *)
+(* 140 ************************************ 833 + 12 *)
 lemma \<sigma>\<^sub>1_OclAllInstances_generic_exec_Person : 
 assumes [simp]: "(\<And>a. (pre_post ((mk (a)))) = a)"
 shows "(mk (\<sigma>\<^sub>1)) \<Turnstile> (OclAllInstances_generic (pre_post) (Person)) \<doteq> Set{(\<lambda>_. \<lfloor>\<lfloor>(mkoid\<^sub>P\<^sub>e\<^sub>r\<^sub>s\<^sub>o\<^sub>n ((mk\<^sub>P\<^sub>e\<^sub>r\<^sub>s\<^sub>o\<^sub>n (oid1) (None) (None) (None) (None))) (((inst_assoc\<sigma>\<^sub>1) (oid\<^sub>P\<^sub>e\<^sub>r\<^sub>s\<^sub>o\<^sub>n_0_\<B>\<O>\<S>\<S>) (switch\<^sub>2_01) (oid1))) (\<lfloor>1000\<rfloor>))\<rfloor>\<rfloor>) , (\<lambda>_. \<lfloor>\<lfloor>(mkoid\<^sub>P\<^sub>e\<^sub>r\<^sub>s\<^sub>o\<^sub>n ((mk\<^sub>P\<^sub>e\<^sub>r\<^sub>s\<^sub>o\<^sub>n (oid2) (None) (None) (None) (None))) (((inst_assoc\<sigma>\<^sub>1) (oid\<^sub>P\<^sub>e\<^sub>r\<^sub>s\<^sub>o\<^sub>n_0_\<B>\<O>\<S>\<S>) (switch\<^sub>2_01) (oid2))) (\<lfloor>1200\<rfloor>))\<rfloor>\<rfloor>) , (\<lambda>_. \<lfloor>\<lfloor>(mkoid\<^sub>P\<^sub>e\<^sub>r\<^sub>s\<^sub>o\<^sub>n ((mk\<^sub>P\<^sub>e\<^sub>r\<^sub>s\<^sub>o\<^sub>n (oid4) (None) (None) (None) (None))) (((inst_assoc\<sigma>\<^sub>1) (oid\<^sub>P\<^sub>e\<^sub>r\<^sub>s\<^sub>o\<^sub>n_0_\<B>\<O>\<S>\<S>) (switch\<^sub>2_01) (oid4))) (\<lfloor>2600\<rfloor>))\<rfloor>\<rfloor>) , X\<^sub>P\<^sub>e\<^sub>r\<^sub>s\<^sub>o\<^sub>n5\<sigma>\<^sub>1 , (\<lambda>_. \<lfloor>\<lfloor>(mkoid\<^sub>P\<^sub>e\<^sub>r\<^sub>s\<^sub>o\<^sub>n ((mk\<^sub>P\<^sub>e\<^sub>r\<^sub>s\<^sub>o\<^sub>n (oid6) (None) (None) (None) (None))) (((inst_assoc\<sigma>\<^sub>1) (oid\<^sub>P\<^sub>e\<^sub>r\<^sub>s\<^sub>o\<^sub>n_0_\<B>\<O>\<S>\<S>) (switch\<^sub>2_01) (oid6))) (\<lfloor>2300\<rfloor>))\<rfloor>\<rfloor>) , X\<^sub>P\<^sub>e\<^sub>r\<^sub>s\<^sub>o\<^sub>n9\<sigma>\<^sub>1}"
@@ -3108,7 +3123,7 @@ shows "(mk (\<sigma>\<^sub>1)) \<Turnstile> (OclAllInstances_generic (pre_post) 
   apply(subst state_update_vs_allInstances_generic_tc, simp, simp, simp add: OclAsType\<^sub>P\<^sub>e\<^sub>r\<^sub>s\<^sub>o\<^sub>n_\<AA>_def, simp, rule const_StrictRefEq\<^sub>S\<^sub>e\<^sub>t_including, simp, simp, simp, rule OclIncluding_cong, simp, simp)
   apply(subst state_update_vs_allInstances_generic_tc, simp, simp, simp add: OclAsType\<^sub>P\<^sub>e\<^sub>r\<^sub>s\<^sub>o\<^sub>n_\<AA>_def, simp, rule const_StrictRefEq\<^sub>S\<^sub>e\<^sub>t_including, simp, simp, simp, rule OclIncluding_cong, simp, simp)
   apply(rule state_update_vs_allInstances_generic_empty)
-by((simp add: OclAsType\<^sub>P\<^sub>e\<^sub>r\<^sub>s\<^sub>o\<^sub>n_\<AA>_def)+) 
+by(simp_all add: OclAsType\<^sub>P\<^sub>e\<^sub>r\<^sub>s\<^sub>o\<^sub>n_\<AA>_def) 
 lemma \<sigma>\<^sub>1_OclAllInstances_at_post_exec_Person : 
 shows "(st , \<sigma>\<^sub>1) \<Turnstile> (OclAllInstances_at_post (Person)) \<doteq> Set{(\<lambda>_. \<lfloor>\<lfloor>(mkoid\<^sub>P\<^sub>e\<^sub>r\<^sub>s\<^sub>o\<^sub>n ((mk\<^sub>P\<^sub>e\<^sub>r\<^sub>s\<^sub>o\<^sub>n (oid1) (None) (None) (None) (None))) (((inst_assoc\<sigma>\<^sub>1) (oid\<^sub>P\<^sub>e\<^sub>r\<^sub>s\<^sub>o\<^sub>n_0_\<B>\<O>\<S>\<S>) (switch\<^sub>2_01) (oid1))) (\<lfloor>1000\<rfloor>))\<rfloor>\<rfloor>) , (\<lambda>_. \<lfloor>\<lfloor>(mkoid\<^sub>P\<^sub>e\<^sub>r\<^sub>s\<^sub>o\<^sub>n ((mk\<^sub>P\<^sub>e\<^sub>r\<^sub>s\<^sub>o\<^sub>n (oid2) (None) (None) (None) (None))) (((inst_assoc\<sigma>\<^sub>1) (oid\<^sub>P\<^sub>e\<^sub>r\<^sub>s\<^sub>o\<^sub>n_0_\<B>\<O>\<S>\<S>) (switch\<^sub>2_01) (oid2))) (\<lfloor>1200\<rfloor>))\<rfloor>\<rfloor>) , (\<lambda>_. \<lfloor>\<lfloor>(mkoid\<^sub>P\<^sub>e\<^sub>r\<^sub>s\<^sub>o\<^sub>n ((mk\<^sub>P\<^sub>e\<^sub>r\<^sub>s\<^sub>o\<^sub>n (oid4) (None) (None) (None) (None))) (((inst_assoc\<sigma>\<^sub>1) (oid\<^sub>P\<^sub>e\<^sub>r\<^sub>s\<^sub>o\<^sub>n_0_\<B>\<O>\<S>\<S>) (switch\<^sub>2_01) (oid4))) (\<lfloor>2600\<rfloor>))\<rfloor>\<rfloor>) , X\<^sub>P\<^sub>e\<^sub>r\<^sub>s\<^sub>o\<^sub>n5\<sigma>\<^sub>1 , (\<lambda>_. \<lfloor>\<lfloor>(mkoid\<^sub>P\<^sub>e\<^sub>r\<^sub>s\<^sub>o\<^sub>n ((mk\<^sub>P\<^sub>e\<^sub>r\<^sub>s\<^sub>o\<^sub>n (oid6) (None) (None) (None) (None))) (((inst_assoc\<sigma>\<^sub>1) (oid\<^sub>P\<^sub>e\<^sub>r\<^sub>s\<^sub>o\<^sub>n_0_\<B>\<O>\<S>\<S>) (switch\<^sub>2_01) (oid6))) (\<lfloor>2300\<rfloor>))\<rfloor>\<rfloor>) , X\<^sub>P\<^sub>e\<^sub>r\<^sub>s\<^sub>o\<^sub>n9\<sigma>\<^sub>1}"
   unfolding OclAllInstances_at_post_def
@@ -3129,7 +3144,7 @@ shows "(mk (\<sigma>\<^sub>1)) \<Turnstile> (OclAllInstances_generic (pre_post) 
   apply(subst state_update_vs_allInstances_generic_tc, simp, simp, simp add: OclAsType\<^sub>P\<^sub>l\<^sub>a\<^sub>n\<^sub>e\<^sub>t_\<AA>_def, simp, rule const_StrictRefEq\<^sub>S\<^sub>e\<^sub>t_including, simp, simp, simp, rule OclIncluding_cong, simp, simp)
   apply(subst state_update_vs_allInstances_generic_tc, simp, simp, simp add: OclAsType\<^sub>P\<^sub>l\<^sub>a\<^sub>n\<^sub>e\<^sub>t_\<AA>_def, simp, rule const_StrictRefEq\<^sub>S\<^sub>e\<^sub>t_including, simp, simp, simp, rule OclIncluding_cong, simp, simp)
   apply(rule state_update_vs_allInstances_generic_empty)
-by((simp add: OclAsType\<^sub>P\<^sub>l\<^sub>a\<^sub>n\<^sub>e\<^sub>t_\<AA>_def)+) 
+by(simp_all add: OclAsType\<^sub>P\<^sub>l\<^sub>a\<^sub>n\<^sub>e\<^sub>t_\<AA>_def) 
 lemma \<sigma>\<^sub>1_OclAllInstances_at_post_exec_Planet : 
 shows "(st , \<sigma>\<^sub>1) \<Turnstile> (OclAllInstances_at_post (Planet)) \<doteq> Set{((\<lambda>_. \<lfloor>\<lfloor>(mkoid\<^sub>P\<^sub>e\<^sub>r\<^sub>s\<^sub>o\<^sub>n ((mk\<^sub>P\<^sub>e\<^sub>r\<^sub>s\<^sub>o\<^sub>n (oid1) (None) (None) (None) (None))) (((inst_assoc\<sigma>\<^sub>1) (oid\<^sub>P\<^sub>e\<^sub>r\<^sub>s\<^sub>o\<^sub>n_0_\<B>\<O>\<S>\<S>) (switch\<^sub>2_01) (oid1))) (\<lfloor>1000\<rfloor>))\<rfloor>\<rfloor>)::Person) .oclAsType(Planet) , ((\<lambda>_. \<lfloor>\<lfloor>(mkoid\<^sub>P\<^sub>e\<^sub>r\<^sub>s\<^sub>o\<^sub>n ((mk\<^sub>P\<^sub>e\<^sub>r\<^sub>s\<^sub>o\<^sub>n (oid2) (None) (None) (None) (None))) (((inst_assoc\<sigma>\<^sub>1) (oid\<^sub>P\<^sub>e\<^sub>r\<^sub>s\<^sub>o\<^sub>n_0_\<B>\<O>\<S>\<S>) (switch\<^sub>2_01) (oid2))) (\<lfloor>1200\<rfloor>))\<rfloor>\<rfloor>)::Person) .oclAsType(Planet) , ((\<lambda>_. \<lfloor>\<lfloor>(mkoid\<^sub>P\<^sub>e\<^sub>r\<^sub>s\<^sub>o\<^sub>n ((mk\<^sub>P\<^sub>e\<^sub>r\<^sub>s\<^sub>o\<^sub>n (oid4) (None) (None) (None) (None))) (((inst_assoc\<sigma>\<^sub>1) (oid\<^sub>P\<^sub>e\<^sub>r\<^sub>s\<^sub>o\<^sub>n_0_\<B>\<O>\<S>\<S>) (switch\<^sub>2_01) (oid4))) (\<lfloor>2600\<rfloor>))\<rfloor>\<rfloor>)::Person) .oclAsType(Planet) , X\<^sub>P\<^sub>e\<^sub>r\<^sub>s\<^sub>o\<^sub>n5\<sigma>\<^sub>1 .oclAsType(Planet) , ((\<lambda>_. \<lfloor>\<lfloor>(mkoid\<^sub>P\<^sub>e\<^sub>r\<^sub>s\<^sub>o\<^sub>n ((mk\<^sub>P\<^sub>e\<^sub>r\<^sub>s\<^sub>o\<^sub>n (oid6) (None) (None) (None) (None))) (((inst_assoc\<sigma>\<^sub>1) (oid\<^sub>P\<^sub>e\<^sub>r\<^sub>s\<^sub>o\<^sub>n_0_\<B>\<O>\<S>\<S>) (switch\<^sub>2_01) (oid6))) (\<lfloor>2300\<rfloor>))\<rfloor>\<rfloor>)::Person) .oclAsType(Planet) , X\<^sub>P\<^sub>e\<^sub>r\<^sub>s\<^sub>o\<^sub>n9\<sigma>\<^sub>1 .oclAsType(Planet)}"
   unfolding OclAllInstances_at_post_def
@@ -3150,7 +3165,7 @@ shows "(mk (\<sigma>\<^sub>1)) \<Turnstile> (OclAllInstances_generic (pre_post) 
   apply(subst state_update_vs_allInstances_generic_tc, simp, simp, simp add: OclAsType\<^sub>G\<^sub>a\<^sub>l\<^sub>a\<^sub>x\<^sub>y_\<AA>_def, simp, rule const_StrictRefEq\<^sub>S\<^sub>e\<^sub>t_including, simp, simp, simp, rule OclIncluding_cong, simp, simp)
   apply(subst state_update_vs_allInstances_generic_tc, simp, simp, simp add: OclAsType\<^sub>G\<^sub>a\<^sub>l\<^sub>a\<^sub>x\<^sub>y_\<AA>_def, simp, rule const_StrictRefEq\<^sub>S\<^sub>e\<^sub>t_including, simp, simp, simp, rule OclIncluding_cong, simp, simp)
   apply(rule state_update_vs_allInstances_generic_empty)
-by((simp add: OclAsType\<^sub>G\<^sub>a\<^sub>l\<^sub>a\<^sub>x\<^sub>y_\<AA>_def)+) 
+by(simp_all add: OclAsType\<^sub>G\<^sub>a\<^sub>l\<^sub>a\<^sub>x\<^sub>y_\<AA>_def) 
 lemma \<sigma>\<^sub>1_OclAllInstances_at_post_exec_Galaxy : 
 shows "(st , \<sigma>\<^sub>1) \<Turnstile> (OclAllInstances_at_post (Galaxy)) \<doteq> Set{((\<lambda>_. \<lfloor>\<lfloor>(mkoid\<^sub>P\<^sub>e\<^sub>r\<^sub>s\<^sub>o\<^sub>n ((mk\<^sub>P\<^sub>e\<^sub>r\<^sub>s\<^sub>o\<^sub>n (oid1) (None) (None) (None) (None))) (((inst_assoc\<sigma>\<^sub>1) (oid\<^sub>P\<^sub>e\<^sub>r\<^sub>s\<^sub>o\<^sub>n_0_\<B>\<O>\<S>\<S>) (switch\<^sub>2_01) (oid1))) (\<lfloor>1000\<rfloor>))\<rfloor>\<rfloor>)::Person) .oclAsType(Galaxy) , ((\<lambda>_. \<lfloor>\<lfloor>(mkoid\<^sub>P\<^sub>e\<^sub>r\<^sub>s\<^sub>o\<^sub>n ((mk\<^sub>P\<^sub>e\<^sub>r\<^sub>s\<^sub>o\<^sub>n (oid2) (None) (None) (None) (None))) (((inst_assoc\<sigma>\<^sub>1) (oid\<^sub>P\<^sub>e\<^sub>r\<^sub>s\<^sub>o\<^sub>n_0_\<B>\<O>\<S>\<S>) (switch\<^sub>2_01) (oid2))) (\<lfloor>1200\<rfloor>))\<rfloor>\<rfloor>)::Person) .oclAsType(Galaxy) , ((\<lambda>_. \<lfloor>\<lfloor>(mkoid\<^sub>P\<^sub>e\<^sub>r\<^sub>s\<^sub>o\<^sub>n ((mk\<^sub>P\<^sub>e\<^sub>r\<^sub>s\<^sub>o\<^sub>n (oid4) (None) (None) (None) (None))) (((inst_assoc\<sigma>\<^sub>1) (oid\<^sub>P\<^sub>e\<^sub>r\<^sub>s\<^sub>o\<^sub>n_0_\<B>\<O>\<S>\<S>) (switch\<^sub>2_01) (oid4))) (\<lfloor>2600\<rfloor>))\<rfloor>\<rfloor>)::Person) .oclAsType(Galaxy) , X\<^sub>P\<^sub>e\<^sub>r\<^sub>s\<^sub>o\<^sub>n5\<sigma>\<^sub>1 .oclAsType(Galaxy) , ((\<lambda>_. \<lfloor>\<lfloor>(mkoid\<^sub>P\<^sub>e\<^sub>r\<^sub>s\<^sub>o\<^sub>n ((mk\<^sub>P\<^sub>e\<^sub>r\<^sub>s\<^sub>o\<^sub>n (oid6) (None) (None) (None) (None))) (((inst_assoc\<sigma>\<^sub>1) (oid\<^sub>P\<^sub>e\<^sub>r\<^sub>s\<^sub>o\<^sub>n_0_\<B>\<O>\<S>\<S>) (switch\<^sub>2_01) (oid6))) (\<lfloor>2300\<rfloor>))\<rfloor>\<rfloor>)::Person) .oclAsType(Galaxy) , X\<^sub>P\<^sub>e\<^sub>r\<^sub>s\<^sub>o\<^sub>n9\<sigma>\<^sub>1 .oclAsType(Galaxy)}"
   unfolding OclAllInstances_at_post_def
@@ -3171,7 +3186,7 @@ shows "(mk (\<sigma>\<^sub>1)) \<Turnstile> (OclAllInstances_generic (pre_post) 
   apply(subst state_update_vs_allInstances_generic_tc, simp, simp, simp add: OclAsType\<^sub>O\<^sub>c\<^sub>l\<^sub>A\<^sub>n\<^sub>y_\<AA>_def, simp, rule const_StrictRefEq\<^sub>S\<^sub>e\<^sub>t_including, simp, simp, simp, rule OclIncluding_cong, simp, simp)
   apply(subst state_update_vs_allInstances_generic_tc, simp, simp, simp add: OclAsType\<^sub>O\<^sub>c\<^sub>l\<^sub>A\<^sub>n\<^sub>y_\<AA>_def, simp, rule const_StrictRefEq\<^sub>S\<^sub>e\<^sub>t_including, simp, simp, simp, rule OclIncluding_cong, simp, simp)
   apply(rule state_update_vs_allInstances_generic_empty)
-by((simp add: OclAsType\<^sub>O\<^sub>c\<^sub>l\<^sub>A\<^sub>n\<^sub>y_\<AA>_def)+) 
+by(simp_all add: OclAsType\<^sub>O\<^sub>c\<^sub>l\<^sub>A\<^sub>n\<^sub>y_\<AA>_def) 
 lemma \<sigma>\<^sub>1_OclAllInstances_at_post_exec_OclAny : 
 shows "(st , \<sigma>\<^sub>1) \<Turnstile> (OclAllInstances_at_post (OclAny)) \<doteq> Set{((\<lambda>_. \<lfloor>\<lfloor>(mkoid\<^sub>P\<^sub>e\<^sub>r\<^sub>s\<^sub>o\<^sub>n ((mk\<^sub>P\<^sub>e\<^sub>r\<^sub>s\<^sub>o\<^sub>n (oid1) (None) (None) (None) (None))) (((inst_assoc\<sigma>\<^sub>1) (oid\<^sub>P\<^sub>e\<^sub>r\<^sub>s\<^sub>o\<^sub>n_0_\<B>\<O>\<S>\<S>) (switch\<^sub>2_01) (oid1))) (\<lfloor>1000\<rfloor>))\<rfloor>\<rfloor>)::Person) .oclAsType(OclAny) , ((\<lambda>_. \<lfloor>\<lfloor>(mkoid\<^sub>P\<^sub>e\<^sub>r\<^sub>s\<^sub>o\<^sub>n ((mk\<^sub>P\<^sub>e\<^sub>r\<^sub>s\<^sub>o\<^sub>n (oid2) (None) (None) (None) (None))) (((inst_assoc\<sigma>\<^sub>1) (oid\<^sub>P\<^sub>e\<^sub>r\<^sub>s\<^sub>o\<^sub>n_0_\<B>\<O>\<S>\<S>) (switch\<^sub>2_01) (oid2))) (\<lfloor>1200\<rfloor>))\<rfloor>\<rfloor>)::Person) .oclAsType(OclAny) , ((\<lambda>_. \<lfloor>\<lfloor>(mkoid\<^sub>P\<^sub>e\<^sub>r\<^sub>s\<^sub>o\<^sub>n ((mk\<^sub>P\<^sub>e\<^sub>r\<^sub>s\<^sub>o\<^sub>n (oid4) (None) (None) (None) (None))) (((inst_assoc\<sigma>\<^sub>1) (oid\<^sub>P\<^sub>e\<^sub>r\<^sub>s\<^sub>o\<^sub>n_0_\<B>\<O>\<S>\<S>) (switch\<^sub>2_01) (oid4))) (\<lfloor>2600\<rfloor>))\<rfloor>\<rfloor>)::Person) .oclAsType(OclAny) , X\<^sub>P\<^sub>e\<^sub>r\<^sub>s\<^sub>o\<^sub>n5\<sigma>\<^sub>1 .oclAsType(OclAny) , ((\<lambda>_. \<lfloor>\<lfloor>(mkoid\<^sub>P\<^sub>e\<^sub>r\<^sub>s\<^sub>o\<^sub>n ((mk\<^sub>P\<^sub>e\<^sub>r\<^sub>s\<^sub>o\<^sub>n (oid6) (None) (None) (None) (None))) (((inst_assoc\<sigma>\<^sub>1) (oid\<^sub>P\<^sub>e\<^sub>r\<^sub>s\<^sub>o\<^sub>n_0_\<B>\<O>\<S>\<S>) (switch\<^sub>2_01) (oid6))) (\<lfloor>2300\<rfloor>))\<rfloor>\<rfloor>)::Person) .oclAsType(OclAny) , X\<^sub>P\<^sub>e\<^sub>r\<^sub>s\<^sub>o\<^sub>n9\<sigma>\<^sub>1 .oclAsType(OclAny)}"
   unfolding OclAllInstances_at_post_def
@@ -3181,14 +3196,14 @@ shows "(\<sigma>\<^sub>1 , st) \<Turnstile> (OclAllInstances_at_pre (OclAny)) \<
   unfolding OclAllInstances_at_pre_def
 by(rule \<sigma>\<^sub>1_OclAllInstances_generic_exec_OclAny, simp) 
 
-(* 141 ************************************ 846 + 1 *)
+(* 141 ************************************ 845 + 1 *)
 definition "inst_assoc\<sigma>\<^sub>1' = (\<lambda>oid_class to_from oid. ((case (deref_assocs_list ((to_from::oid list list \<Rightarrow> oid list \<times> oid list)) ((oid::oid)) ((drop ((((map_of_list ([(oid\<^sub>P\<^sub>e\<^sub>r\<^sub>s\<^sub>o\<^sub>n_0_\<B>\<O>\<S>\<S> , (List.map ((\<lambda>(x , y). [x , y]) o switch\<^sub>2_01) ([[[oid7] , [oid7]] , [[oid6] , [oid7]] , [[oid2] , [oid2]] , [[oid1] , [oid2]]])))]))) ((oid_class::oid))))))) of Nil \<Rightarrow> None
     | l \<Rightarrow> (Some (l)))::oid list option))"
 
-(* 142 ************************************ 847 + 1 *)
+(* 142 ************************************ 846 + 1 *)
 definition "\<sigma>\<^sub>1' = (state.make ((Map.empty (oid1 \<mapsto> (in\<^sub>P\<^sub>e\<^sub>r\<^sub>s\<^sub>o\<^sub>n ((X\<^sub>P\<^sub>e\<^sub>r\<^sub>s\<^sub>o\<^sub>n1\<^sub>P\<^sub>e\<^sub>r\<^sub>s\<^sub>o\<^sub>n (inst_assoc\<sigma>\<^sub>1'))))) (oid2 \<mapsto> (in\<^sub>P\<^sub>e\<^sub>r\<^sub>s\<^sub>o\<^sub>n ((X\<^sub>P\<^sub>e\<^sub>r\<^sub>s\<^sub>o\<^sub>n2\<^sub>P\<^sub>e\<^sub>r\<^sub>s\<^sub>o\<^sub>n (inst_assoc\<sigma>\<^sub>1'))))) (oid3 \<mapsto> (in\<^sub>P\<^sub>e\<^sub>r\<^sub>s\<^sub>o\<^sub>n ((X\<^sub>P\<^sub>e\<^sub>r\<^sub>s\<^sub>o\<^sub>n3\<^sub>P\<^sub>e\<^sub>r\<^sub>s\<^sub>o\<^sub>n (inst_assoc\<sigma>\<^sub>1'))))) (oid4 \<mapsto> (in\<^sub>P\<^sub>e\<^sub>r\<^sub>s\<^sub>o\<^sub>n ((X\<^sub>P\<^sub>e\<^sub>r\<^sub>s\<^sub>o\<^sub>n4\<^sub>P\<^sub>e\<^sub>r\<^sub>s\<^sub>o\<^sub>n (inst_assoc\<sigma>\<^sub>1'))))) (oid6 \<mapsto> (in\<^sub>P\<^sub>e\<^sub>r\<^sub>s\<^sub>o\<^sub>n ((X\<^sub>P\<^sub>e\<^sub>r\<^sub>s\<^sub>o\<^sub>n6\<^sub>P\<^sub>e\<^sub>r\<^sub>s\<^sub>o\<^sub>n (inst_assoc\<sigma>\<^sub>1'))))) (oid7 \<mapsto> (in\<^sub>O\<^sub>c\<^sub>l\<^sub>A\<^sub>n\<^sub>y ((X\<^sub>P\<^sub>e\<^sub>r\<^sub>s\<^sub>o\<^sub>n7\<^sub>O\<^sub>c\<^sub>l\<^sub>A\<^sub>n\<^sub>y (inst_assoc\<sigma>\<^sub>1'))))) (oid8 \<mapsto> (in\<^sub>O\<^sub>c\<^sub>l\<^sub>A\<^sub>n\<^sub>y ((X\<^sub>P\<^sub>e\<^sub>r\<^sub>s\<^sub>o\<^sub>n8\<^sub>O\<^sub>c\<^sub>l\<^sub>A\<^sub>n\<^sub>y (inst_assoc\<sigma>\<^sub>1'))))) (oid9 \<mapsto> (in\<^sub>P\<^sub>e\<^sub>r\<^sub>s\<^sub>o\<^sub>n ((X\<^sub>P\<^sub>e\<^sub>r\<^sub>s\<^sub>o\<^sub>n9\<^sub>P\<^sub>e\<^sub>r\<^sub>s\<^sub>o\<^sub>n (inst_assoc\<sigma>\<^sub>1'))))))) (Map.empty))"
 
-(* 143 ************************************ 848 + 8 *)
+(* 143 ************************************ 847 + 8 *)
 definition "(X\<^sub>P\<^sub>e\<^sub>r\<^sub>s\<^sub>o\<^sub>n1\<sigma>\<^sub>1'::Person) = (\<lambda>_. \<lfloor>\<lfloor>(X\<^sub>P\<^sub>e\<^sub>r\<^sub>s\<^sub>o\<^sub>n1\<^sub>P\<^sub>e\<^sub>r\<^sub>s\<^sub>o\<^sub>n (inst_assoc\<sigma>\<^sub>1'))\<rfloor>\<rfloor>)"
 definition "(X\<^sub>P\<^sub>e\<^sub>r\<^sub>s\<^sub>o\<^sub>n2\<sigma>\<^sub>1'::Person) = (\<lambda>_. \<lfloor>\<lfloor>(X\<^sub>P\<^sub>e\<^sub>r\<^sub>s\<^sub>o\<^sub>n2\<^sub>P\<^sub>e\<^sub>r\<^sub>s\<^sub>o\<^sub>n (inst_assoc\<sigma>\<^sub>1'))\<rfloor>\<rfloor>)"
 definition "(X\<^sub>P\<^sub>e\<^sub>r\<^sub>s\<^sub>o\<^sub>n3\<sigma>\<^sub>1'::Person) = (\<lambda>_. \<lfloor>\<lfloor>(X\<^sub>P\<^sub>e\<^sub>r\<^sub>s\<^sub>o\<^sub>n3\<^sub>P\<^sub>e\<^sub>r\<^sub>s\<^sub>o\<^sub>n (inst_assoc\<sigma>\<^sub>1'))\<rfloor>\<rfloor>)"
@@ -3198,14 +3213,14 @@ definition "(X\<^sub>P\<^sub>e\<^sub>r\<^sub>s\<^sub>o\<^sub>n7\<sigma>\<^sub>1'
 definition "(X\<^sub>P\<^sub>e\<^sub>r\<^sub>s\<^sub>o\<^sub>n8\<sigma>\<^sub>1'::OclAny) = (\<lambda>_. \<lfloor>\<lfloor>(X\<^sub>P\<^sub>e\<^sub>r\<^sub>s\<^sub>o\<^sub>n8\<^sub>O\<^sub>c\<^sub>l\<^sub>A\<^sub>n\<^sub>y (inst_assoc\<sigma>\<^sub>1'))\<rfloor>\<rfloor>)"
 definition "(X\<^sub>P\<^sub>e\<^sub>r\<^sub>s\<^sub>o\<^sub>n9\<sigma>\<^sub>1'::Person) = (\<lambda>_. \<lfloor>\<lfloor>(X\<^sub>P\<^sub>e\<^sub>r\<^sub>s\<^sub>o\<^sub>n9\<^sub>P\<^sub>e\<^sub>r\<^sub>s\<^sub>o\<^sub>n (inst_assoc\<sigma>\<^sub>1'))\<rfloor>\<rfloor>)"
 
-(* 144 ************************************ 856 + 1 *)
+(* 144 ************************************ 855 + 1 *)
 lemma dom_\<sigma>\<^sub>1' : "(dom ((heap (\<sigma>\<^sub>1')))) = {oid1 , oid2 , oid3 , oid4 , oid6 , oid7 , oid8 , oid9}"
 by(auto simp: \<sigma>\<^sub>1'_def)
 
-(* 145 ************************************ 857 + 1 *)
-lemmas [simp,code_unfold] = dom_\<sigma>\<^sub>1'
+(* 145 ************************************ 856 + 1 *)
+lemmas[simp,code_unfold] = dom_\<sigma>\<^sub>1'
 
-(* 146 ************************************ 858 + 1 *)
+(* 146 ************************************ 857 + 1 *)
 lemma perm_\<sigma>\<^sub>1' : "\<sigma>\<^sub>1' = (state.make ((Map.empty (oid9 \<mapsto> (in\<^sub>P\<^sub>e\<^sub>r\<^sub>s\<^sub>o\<^sub>n ((X\<^sub>P\<^sub>e\<^sub>r\<^sub>s\<^sub>o\<^sub>n9\<^sub>P\<^sub>e\<^sub>r\<^sub>s\<^sub>o\<^sub>n (inst_assoc\<sigma>\<^sub>1'))))) (oid8 \<mapsto> (in\<^sub>O\<^sub>c\<^sub>l\<^sub>A\<^sub>n\<^sub>y ((X\<^sub>P\<^sub>e\<^sub>r\<^sub>s\<^sub>o\<^sub>n8\<^sub>O\<^sub>c\<^sub>l\<^sub>A\<^sub>n\<^sub>y (inst_assoc\<sigma>\<^sub>1'))))) (oid7 \<mapsto> (in\<^sub>O\<^sub>c\<^sub>l\<^sub>A\<^sub>n\<^sub>y ((X\<^sub>P\<^sub>e\<^sub>r\<^sub>s\<^sub>o\<^sub>n7\<^sub>O\<^sub>c\<^sub>l\<^sub>A\<^sub>n\<^sub>y (inst_assoc\<sigma>\<^sub>1'))))) (oid6 \<mapsto> (in\<^sub>P\<^sub>e\<^sub>r\<^sub>s\<^sub>o\<^sub>n ((X\<^sub>P\<^sub>e\<^sub>r\<^sub>s\<^sub>o\<^sub>n6\<^sub>P\<^sub>e\<^sub>r\<^sub>s\<^sub>o\<^sub>n (inst_assoc\<sigma>\<^sub>1'))))) (oid4 \<mapsto> (in\<^sub>P\<^sub>e\<^sub>r\<^sub>s\<^sub>o\<^sub>n ((X\<^sub>P\<^sub>e\<^sub>r\<^sub>s\<^sub>o\<^sub>n4\<^sub>P\<^sub>e\<^sub>r\<^sub>s\<^sub>o\<^sub>n (inst_assoc\<sigma>\<^sub>1'))))) (oid3 \<mapsto> (in\<^sub>P\<^sub>e\<^sub>r\<^sub>s\<^sub>o\<^sub>n ((X\<^sub>P\<^sub>e\<^sub>r\<^sub>s\<^sub>o\<^sub>n3\<^sub>P\<^sub>e\<^sub>r\<^sub>s\<^sub>o\<^sub>n (inst_assoc\<sigma>\<^sub>1'))))) (oid2 \<mapsto> (in\<^sub>P\<^sub>e\<^sub>r\<^sub>s\<^sub>o\<^sub>n ((X\<^sub>P\<^sub>e\<^sub>r\<^sub>s\<^sub>o\<^sub>n2\<^sub>P\<^sub>e\<^sub>r\<^sub>s\<^sub>o\<^sub>n (inst_assoc\<sigma>\<^sub>1'))))) (oid1 \<mapsto> (in\<^sub>P\<^sub>e\<^sub>r\<^sub>s\<^sub>o\<^sub>n ((X\<^sub>P\<^sub>e\<^sub>r\<^sub>s\<^sub>o\<^sub>n1\<^sub>P\<^sub>e\<^sub>r\<^sub>s\<^sub>o\<^sub>n (inst_assoc\<sigma>\<^sub>1'))))))) ((assocs (\<sigma>\<^sub>1'))))"
   apply(simp add: \<sigma>\<^sub>1'_def oid1_def oid2_def oid3_def oid4_def oid6_def oid7_def oid8_def oid9_def)
   apply(subst (1) fun_upd_twist, simp)
@@ -3238,7 +3253,7 @@ lemma perm_\<sigma>\<^sub>1' : "\<sigma>\<^sub>1' = (state.make ((Map.empty (oid
   apply(subst (1) fun_upd_twist, simp)
 by(simp)
 
-(* 147 ************************************ 859 + 12 *)
+(* 147 ************************************ 858 + 12 *)
 lemma \<sigma>\<^sub>1'_OclAllInstances_generic_exec_Person : 
 assumes [simp]: "(\<And>a. (pre_post ((mk (a)))) = a)"
 shows "(mk (\<sigma>\<^sub>1')) \<Turnstile> (OclAllInstances_generic (pre_post) (Person)) \<doteq> Set{X\<^sub>P\<^sub>e\<^sub>r\<^sub>s\<^sub>o\<^sub>n1\<sigma>\<^sub>1' , X\<^sub>P\<^sub>e\<^sub>r\<^sub>s\<^sub>o\<^sub>n2\<sigma>\<^sub>1' , X\<^sub>P\<^sub>e\<^sub>r\<^sub>s\<^sub>o\<^sub>n3\<sigma>\<^sub>1' , X\<^sub>P\<^sub>e\<^sub>r\<^sub>s\<^sub>o\<^sub>n4\<sigma>\<^sub>1' , X\<^sub>P\<^sub>e\<^sub>r\<^sub>s\<^sub>o\<^sub>n6\<sigma>\<^sub>1' , X\<^sub>P\<^sub>e\<^sub>r\<^sub>s\<^sub>o\<^sub>n7\<sigma>\<^sub>1' .oclAsType(Person) , X\<^sub>P\<^sub>e\<^sub>r\<^sub>s\<^sub>o\<^sub>n9\<sigma>\<^sub>1'}"
@@ -3253,7 +3268,7 @@ shows "(mk (\<sigma>\<^sub>1')) \<Turnstile> (OclAllInstances_generic (pre_post)
   apply(subst state_update_vs_allInstances_generic_ntc, simp, simp, simp add: OclAsType\<^sub>P\<^sub>e\<^sub>r\<^sub>s\<^sub>o\<^sub>n_\<AA>_def X\<^sub>P\<^sub>e\<^sub>r\<^sub>s\<^sub>o\<^sub>n8\<^sub>O\<^sub>c\<^sub>l\<^sub>A\<^sub>n\<^sub>y_def, simp, rule const_StrictRefEq\<^sub>S\<^sub>e\<^sub>t_including, simp, simp, simp)
   apply(subst state_update_vs_allInstances_generic_tc, simp, simp, simp add: OclAsType\<^sub>P\<^sub>e\<^sub>r\<^sub>s\<^sub>o\<^sub>n_\<AA>_def, simp, rule const_StrictRefEq\<^sub>S\<^sub>e\<^sub>t_including, simp, simp, simp, rule OclIncluding_cong, simp, simp)
   apply(rule state_update_vs_allInstances_generic_empty)
-by((simp add: OclAsType\<^sub>P\<^sub>e\<^sub>r\<^sub>s\<^sub>o\<^sub>n_\<AA>_def)+) 
+by(simp_all add: OclAsType\<^sub>P\<^sub>e\<^sub>r\<^sub>s\<^sub>o\<^sub>n_\<AA>_def) 
 lemma \<sigma>\<^sub>1'_OclAllInstances_at_post_exec_Person : 
 shows "(st , \<sigma>\<^sub>1') \<Turnstile> (OclAllInstances_at_post (Person)) \<doteq> Set{X\<^sub>P\<^sub>e\<^sub>r\<^sub>s\<^sub>o\<^sub>n1\<sigma>\<^sub>1' , X\<^sub>P\<^sub>e\<^sub>r\<^sub>s\<^sub>o\<^sub>n2\<sigma>\<^sub>1' , X\<^sub>P\<^sub>e\<^sub>r\<^sub>s\<^sub>o\<^sub>n3\<sigma>\<^sub>1' , X\<^sub>P\<^sub>e\<^sub>r\<^sub>s\<^sub>o\<^sub>n4\<sigma>\<^sub>1' , X\<^sub>P\<^sub>e\<^sub>r\<^sub>s\<^sub>o\<^sub>n6\<sigma>\<^sub>1' , X\<^sub>P\<^sub>e\<^sub>r\<^sub>s\<^sub>o\<^sub>n7\<sigma>\<^sub>1' .oclAsType(Person) , X\<^sub>P\<^sub>e\<^sub>r\<^sub>s\<^sub>o\<^sub>n9\<sigma>\<^sub>1'}"
   unfolding OclAllInstances_at_post_def
@@ -3276,7 +3291,7 @@ shows "(mk (\<sigma>\<^sub>1')) \<Turnstile> (OclAllInstances_generic (pre_post)
   apply(subst state_update_vs_allInstances_generic_ntc, simp, simp, simp add: OclAsType\<^sub>P\<^sub>l\<^sub>a\<^sub>n\<^sub>e\<^sub>t_\<AA>_def X\<^sub>P\<^sub>e\<^sub>r\<^sub>s\<^sub>o\<^sub>n8\<^sub>O\<^sub>c\<^sub>l\<^sub>A\<^sub>n\<^sub>y_def, simp, rule const_StrictRefEq\<^sub>S\<^sub>e\<^sub>t_including, simp, simp, simp)
   apply(subst state_update_vs_allInstances_generic_tc, simp, simp, simp add: OclAsType\<^sub>P\<^sub>l\<^sub>a\<^sub>n\<^sub>e\<^sub>t_\<AA>_def, simp, rule const_StrictRefEq\<^sub>S\<^sub>e\<^sub>t_including, simp, simp, simp, rule OclIncluding_cong, simp, simp)
   apply(rule state_update_vs_allInstances_generic_empty)
-by((simp add: OclAsType\<^sub>P\<^sub>l\<^sub>a\<^sub>n\<^sub>e\<^sub>t_\<AA>_def)+) 
+by(simp_all add: OclAsType\<^sub>P\<^sub>l\<^sub>a\<^sub>n\<^sub>e\<^sub>t_\<AA>_def) 
 lemma \<sigma>\<^sub>1'_OclAllInstances_at_post_exec_Planet : 
 shows "(st , \<sigma>\<^sub>1') \<Turnstile> (OclAllInstances_at_post (Planet)) \<doteq> Set{X\<^sub>P\<^sub>e\<^sub>r\<^sub>s\<^sub>o\<^sub>n1\<sigma>\<^sub>1' .oclAsType(Planet) , X\<^sub>P\<^sub>e\<^sub>r\<^sub>s\<^sub>o\<^sub>n2\<sigma>\<^sub>1' .oclAsType(Planet) , X\<^sub>P\<^sub>e\<^sub>r\<^sub>s\<^sub>o\<^sub>n3\<sigma>\<^sub>1' .oclAsType(Planet) , X\<^sub>P\<^sub>e\<^sub>r\<^sub>s\<^sub>o\<^sub>n4\<sigma>\<^sub>1' .oclAsType(Planet) , X\<^sub>P\<^sub>e\<^sub>r\<^sub>s\<^sub>o\<^sub>n6\<sigma>\<^sub>1' .oclAsType(Planet) , X\<^sub>P\<^sub>e\<^sub>r\<^sub>s\<^sub>o\<^sub>n9\<sigma>\<^sub>1' .oclAsType(Planet)}"
   unfolding OclAllInstances_at_post_def
@@ -3299,7 +3314,7 @@ shows "(mk (\<sigma>\<^sub>1')) \<Turnstile> (OclAllInstances_generic (pre_post)
   apply(subst state_update_vs_allInstances_generic_ntc, simp, simp, simp add: OclAsType\<^sub>G\<^sub>a\<^sub>l\<^sub>a\<^sub>x\<^sub>y_\<AA>_def X\<^sub>P\<^sub>e\<^sub>r\<^sub>s\<^sub>o\<^sub>n8\<^sub>O\<^sub>c\<^sub>l\<^sub>A\<^sub>n\<^sub>y_def, simp, rule const_StrictRefEq\<^sub>S\<^sub>e\<^sub>t_including, simp, simp, simp)
   apply(subst state_update_vs_allInstances_generic_tc, simp, simp, simp add: OclAsType\<^sub>G\<^sub>a\<^sub>l\<^sub>a\<^sub>x\<^sub>y_\<AA>_def, simp, rule const_StrictRefEq\<^sub>S\<^sub>e\<^sub>t_including, simp, simp, simp, rule OclIncluding_cong, simp, simp)
   apply(rule state_update_vs_allInstances_generic_empty)
-by((simp add: OclAsType\<^sub>G\<^sub>a\<^sub>l\<^sub>a\<^sub>x\<^sub>y_\<AA>_def)+) 
+by(simp_all add: OclAsType\<^sub>G\<^sub>a\<^sub>l\<^sub>a\<^sub>x\<^sub>y_\<AA>_def) 
 lemma \<sigma>\<^sub>1'_OclAllInstances_at_post_exec_Galaxy : 
 shows "(st , \<sigma>\<^sub>1') \<Turnstile> (OclAllInstances_at_post (Galaxy)) \<doteq> Set{X\<^sub>P\<^sub>e\<^sub>r\<^sub>s\<^sub>o\<^sub>n1\<sigma>\<^sub>1' .oclAsType(Galaxy) , X\<^sub>P\<^sub>e\<^sub>r\<^sub>s\<^sub>o\<^sub>n2\<sigma>\<^sub>1' .oclAsType(Galaxy) , X\<^sub>P\<^sub>e\<^sub>r\<^sub>s\<^sub>o\<^sub>n3\<sigma>\<^sub>1' .oclAsType(Galaxy) , X\<^sub>P\<^sub>e\<^sub>r\<^sub>s\<^sub>o\<^sub>n4\<sigma>\<^sub>1' .oclAsType(Galaxy) , X\<^sub>P\<^sub>e\<^sub>r\<^sub>s\<^sub>o\<^sub>n6\<sigma>\<^sub>1' .oclAsType(Galaxy) , X\<^sub>P\<^sub>e\<^sub>r\<^sub>s\<^sub>o\<^sub>n9\<sigma>\<^sub>1' .oclAsType(Galaxy)}"
   unfolding OclAllInstances_at_post_def
@@ -3322,7 +3337,7 @@ shows "(mk (\<sigma>\<^sub>1')) \<Turnstile> (OclAllInstances_generic (pre_post)
   apply(subst state_update_vs_allInstances_generic_tc, simp, simp, simp add: OclAsType\<^sub>O\<^sub>c\<^sub>l\<^sub>A\<^sub>n\<^sub>y_\<AA>_def, simp, rule const_StrictRefEq\<^sub>S\<^sub>e\<^sub>t_including, simp, simp, simp, rule OclIncluding_cong, simp, simp)
   apply(subst state_update_vs_allInstances_generic_tc, simp, simp, simp add: OclAsType\<^sub>O\<^sub>c\<^sub>l\<^sub>A\<^sub>n\<^sub>y_\<AA>_def, simp, rule const_StrictRefEq\<^sub>S\<^sub>e\<^sub>t_including, simp, simp, simp, rule OclIncluding_cong, simp, simp)
   apply(rule state_update_vs_allInstances_generic_empty)
-by((simp add: OclAsType\<^sub>O\<^sub>c\<^sub>l\<^sub>A\<^sub>n\<^sub>y_\<AA>_def)+) 
+by(simp_all add: OclAsType\<^sub>O\<^sub>c\<^sub>l\<^sub>A\<^sub>n\<^sub>y_\<AA>_def) 
 lemma \<sigma>\<^sub>1'_OclAllInstances_at_post_exec_OclAny : 
 shows "(st , \<sigma>\<^sub>1') \<Turnstile> (OclAllInstances_at_post (OclAny)) \<doteq> Set{X\<^sub>P\<^sub>e\<^sub>r\<^sub>s\<^sub>o\<^sub>n1\<sigma>\<^sub>1' .oclAsType(OclAny) , X\<^sub>P\<^sub>e\<^sub>r\<^sub>s\<^sub>o\<^sub>n2\<sigma>\<^sub>1' .oclAsType(OclAny) , X\<^sub>P\<^sub>e\<^sub>r\<^sub>s\<^sub>o\<^sub>n3\<sigma>\<^sub>1' .oclAsType(OclAny) , X\<^sub>P\<^sub>e\<^sub>r\<^sub>s\<^sub>o\<^sub>n4\<sigma>\<^sub>1' .oclAsType(OclAny) , X\<^sub>P\<^sub>e\<^sub>r\<^sub>s\<^sub>o\<^sub>n6\<sigma>\<^sub>1' .oclAsType(OclAny) , X\<^sub>P\<^sub>e\<^sub>r\<^sub>s\<^sub>o\<^sub>n7\<sigma>\<^sub>1' , X\<^sub>P\<^sub>e\<^sub>r\<^sub>s\<^sub>o\<^sub>n8\<sigma>\<^sub>1' , X\<^sub>P\<^sub>e\<^sub>r\<^sub>s\<^sub>o\<^sub>n9\<sigma>\<^sub>1' .oclAsType(OclAny)}"
   unfolding OclAllInstances_at_post_def
@@ -3332,93 +3347,11 @@ shows "(\<sigma>\<^sub>1' , st) \<Turnstile> (OclAllInstances_at_pre (OclAny)) \
   unfolding OclAllInstances_at_pre_def
 by(rule \<sigma>\<^sub>1'_OclAllInstances_generic_exec_OclAny, simp) 
 
-(* 148 ************************************ 871 + 1 *)
-definition "inst_assoc\<sigma>\<^sub>0 = (\<lambda>oid_class to_from oid. ((case (deref_assocs_list ((to_from::oid list list \<Rightarrow> oid list \<times> oid list)) ((oid::oid)) ((drop ((((map_of_list ([]))) ((oid_class::oid))))))) of Nil \<Rightarrow> None
-    | l \<Rightarrow> (Some (l)))::oid list option))"
-
-(* 149 ************************************ 872 + 1 *)
-definition "\<sigma>\<^sub>0 = (state.make ((Map.empty )) (Map.empty))"
-
-(* 150 ************************************ 873 + 0 *)
-
-(* 151 ************************************ 873 + 1 *)
-lemma dom_\<sigma>\<^sub>0 : "(dom ((heap (\<sigma>\<^sub>0)))) = {}"
-by(auto simp: \<sigma>\<^sub>0_def)
-
-(* 152 ************************************ 874 + 1 *)
-lemmas [simp,code_unfold] = dom_\<sigma>\<^sub>0
-
-(* 153 ************************************ 875 + 1 *)
-lemma perm_\<sigma>\<^sub>0 : "\<sigma>\<^sub>0 = (state.make ((Map.empty )) ((assocs (\<sigma>\<^sub>0))))"
-by(simp add: \<sigma>\<^sub>0_def)
-
-(* 154 ************************************ 876 + 12 *)
-lemma \<sigma>\<^sub>0_OclAllInstances_generic_exec_Person : 
-assumes [simp]: "(\<And>a. (pre_post ((mk (a)))) = a)"
-shows "(mk (\<sigma>\<^sub>0)) \<Turnstile> (OclAllInstances_generic (pre_post) (Person)) \<doteq> Set{}"
-  apply(subst perm_\<sigma>\<^sub>0)
-  apply(simp only: state.make_def)
-  apply(rule state_update_vs_allInstances_generic_empty)
-by(simp) 
-lemma \<sigma>\<^sub>0_OclAllInstances_at_post_exec_Person : 
-shows "(st , \<sigma>\<^sub>0) \<Turnstile> (OclAllInstances_at_post (Person)) \<doteq> Set{}"
-  unfolding OclAllInstances_at_post_def
-by(rule \<sigma>\<^sub>0_OclAllInstances_generic_exec_Person, simp) 
-lemma \<sigma>\<^sub>0_OclAllInstances_at_pre_exec_Person : 
-shows "(\<sigma>\<^sub>0 , st) \<Turnstile> (OclAllInstances_at_pre (Person)) \<doteq> Set{}"
-  unfolding OclAllInstances_at_pre_def
-by(rule \<sigma>\<^sub>0_OclAllInstances_generic_exec_Person, simp) 
-lemma \<sigma>\<^sub>0_OclAllInstances_generic_exec_Planet : 
-assumes [simp]: "(\<And>a. (pre_post ((mk (a)))) = a)"
-shows "(mk (\<sigma>\<^sub>0)) \<Turnstile> (OclAllInstances_generic (pre_post) (Planet)) \<doteq> Set{}"
-  apply(subst perm_\<sigma>\<^sub>0)
-  apply(simp only: state.make_def)
-  apply(rule state_update_vs_allInstances_generic_empty)
-by(simp) 
-lemma \<sigma>\<^sub>0_OclAllInstances_at_post_exec_Planet : 
-shows "(st , \<sigma>\<^sub>0) \<Turnstile> (OclAllInstances_at_post (Planet)) \<doteq> Set{}"
-  unfolding OclAllInstances_at_post_def
-by(rule \<sigma>\<^sub>0_OclAllInstances_generic_exec_Planet, simp) 
-lemma \<sigma>\<^sub>0_OclAllInstances_at_pre_exec_Planet : 
-shows "(\<sigma>\<^sub>0 , st) \<Turnstile> (OclAllInstances_at_pre (Planet)) \<doteq> Set{}"
-  unfolding OclAllInstances_at_pre_def
-by(rule \<sigma>\<^sub>0_OclAllInstances_generic_exec_Planet, simp) 
-lemma \<sigma>\<^sub>0_OclAllInstances_generic_exec_Galaxy : 
-assumes [simp]: "(\<And>a. (pre_post ((mk (a)))) = a)"
-shows "(mk (\<sigma>\<^sub>0)) \<Turnstile> (OclAllInstances_generic (pre_post) (Galaxy)) \<doteq> Set{}"
-  apply(subst perm_\<sigma>\<^sub>0)
-  apply(simp only: state.make_def)
-  apply(rule state_update_vs_allInstances_generic_empty)
-by(simp) 
-lemma \<sigma>\<^sub>0_OclAllInstances_at_post_exec_Galaxy : 
-shows "(st , \<sigma>\<^sub>0) \<Turnstile> (OclAllInstances_at_post (Galaxy)) \<doteq> Set{}"
-  unfolding OclAllInstances_at_post_def
-by(rule \<sigma>\<^sub>0_OclAllInstances_generic_exec_Galaxy, simp) 
-lemma \<sigma>\<^sub>0_OclAllInstances_at_pre_exec_Galaxy : 
-shows "(\<sigma>\<^sub>0 , st) \<Turnstile> (OclAllInstances_at_pre (Galaxy)) \<doteq> Set{}"
-  unfolding OclAllInstances_at_pre_def
-by(rule \<sigma>\<^sub>0_OclAllInstances_generic_exec_Galaxy, simp) 
-lemma \<sigma>\<^sub>0_OclAllInstances_generic_exec_OclAny : 
-assumes [simp]: "(\<And>a. (pre_post ((mk (a)))) = a)"
-shows "(mk (\<sigma>\<^sub>0)) \<Turnstile> (OclAllInstances_generic (pre_post) (OclAny)) \<doteq> Set{}"
-  apply(subst perm_\<sigma>\<^sub>0)
-  apply(simp only: state.make_def)
-  apply(rule state_update_vs_allInstances_generic_empty)
-by(simp) 
-lemma \<sigma>\<^sub>0_OclAllInstances_at_post_exec_OclAny : 
-shows "(st , \<sigma>\<^sub>0) \<Turnstile> (OclAllInstances_at_post (OclAny)) \<doteq> Set{}"
-  unfolding OclAllInstances_at_post_def
-by(rule \<sigma>\<^sub>0_OclAllInstances_generic_exec_OclAny, simp) 
-lemma \<sigma>\<^sub>0_OclAllInstances_at_pre_exec_OclAny : 
-shows "(\<sigma>\<^sub>0 , st) \<Turnstile> (OclAllInstances_at_pre (OclAny)) \<doteq> Set{}"
-  unfolding OclAllInstances_at_pre_def
-by(rule \<sigma>\<^sub>0_OclAllInstances_generic_exec_OclAny, simp) 
-
-(* 155 ************************************ 888 + 1 *)
+(* 148 ************************************ 870 + 1 *)
 lemma basic_\<sigma>\<^sub>1_\<sigma>\<^sub>1'_wff : "(WFF ((\<sigma>\<^sub>1 , \<sigma>\<^sub>1')))"
 by(simp add: WFF_def \<sigma>\<^sub>1_def \<sigma>\<^sub>1'_def oid_of_\<AA>_def oid1_def oid2_def oid3_def oid4_def oid5_def oid6_def oid7_def oid8_def oid9_def X\<^sub>P\<^sub>e\<^sub>r\<^sub>s\<^sub>o\<^sub>n1\<^sub>P\<^sub>e\<^sub>r\<^sub>s\<^sub>o\<^sub>n_def X\<^sub>P\<^sub>e\<^sub>r\<^sub>s\<^sub>o\<^sub>n2\<^sub>P\<^sub>e\<^sub>r\<^sub>s\<^sub>o\<^sub>n_def X\<^sub>P\<^sub>e\<^sub>r\<^sub>s\<^sub>o\<^sub>n3\<^sub>P\<^sub>e\<^sub>r\<^sub>s\<^sub>o\<^sub>n_def X\<^sub>P\<^sub>e\<^sub>r\<^sub>s\<^sub>o\<^sub>n4\<^sub>P\<^sub>e\<^sub>r\<^sub>s\<^sub>o\<^sub>n_def X\<^sub>P\<^sub>e\<^sub>r\<^sub>s\<^sub>o\<^sub>n5\<^sub>P\<^sub>e\<^sub>r\<^sub>s\<^sub>o\<^sub>n_def X\<^sub>P\<^sub>e\<^sub>r\<^sub>s\<^sub>o\<^sub>n6\<^sub>P\<^sub>e\<^sub>r\<^sub>s\<^sub>o\<^sub>n_def X\<^sub>P\<^sub>e\<^sub>r\<^sub>s\<^sub>o\<^sub>n7\<^sub>O\<^sub>c\<^sub>l\<^sub>A\<^sub>n\<^sub>y_def X\<^sub>P\<^sub>e\<^sub>r\<^sub>s\<^sub>o\<^sub>n8\<^sub>O\<^sub>c\<^sub>l\<^sub>A\<^sub>n\<^sub>y_def X\<^sub>P\<^sub>e\<^sub>r\<^sub>s\<^sub>o\<^sub>n9\<^sub>P\<^sub>e\<^sub>r\<^sub>s\<^sub>o\<^sub>n_def oid_of_typeoid\<^sub>O\<^sub>c\<^sub>l\<^sub>A\<^sub>n\<^sub>y_def oid_of_typeoid\<^sub>P\<^sub>e\<^sub>r\<^sub>s\<^sub>o\<^sub>n_def)
 
-(* 156 ************************************ 889 + 10 *)
+(* 149 ************************************ 871 + 10 *)
 lemma oid1\<sigma>\<^sub>1\<sigma>\<^sub>1'_\<sigma>\<^sub>1'_OclIsMaintained : "(\<sigma>\<^sub>1 , \<sigma>\<^sub>1') \<Turnstile> (OclIsMaintained (X\<^sub>P\<^sub>e\<^sub>r\<^sub>s\<^sub>o\<^sub>n1\<sigma>\<^sub>1'))"
 by(simp add: X\<^sub>P\<^sub>e\<^sub>r\<^sub>s\<^sub>o\<^sub>n1\<sigma>\<^sub>1'_def X\<^sub>P\<^sub>e\<^sub>r\<^sub>s\<^sub>o\<^sub>n1\<^sub>P\<^sub>e\<^sub>r\<^sub>s\<^sub>o\<^sub>n_def OclIsMaintained_def OclValid_def \<sigma>\<^sub>1_def \<sigma>\<^sub>1'_def oid_of_option_def oid1_def oid2_def oid3_def oid4_def oid5_def oid6_def oid7_def oid8_def oid9_def oid_of_typeoid\<^sub>O\<^sub>c\<^sub>l\<^sub>A\<^sub>n\<^sub>y_def oid_of_typeoid\<^sub>P\<^sub>e\<^sub>r\<^sub>s\<^sub>o\<^sub>n_def)
 lemma oid2\<sigma>\<^sub>1\<sigma>\<^sub>1'_\<sigma>\<^sub>1'_OclIsMaintained : "(\<sigma>\<^sub>1 , \<sigma>\<^sub>1') \<Turnstile> (OclIsMaintained (X\<^sub>P\<^sub>e\<^sub>r\<^sub>s\<^sub>o\<^sub>n2\<sigma>\<^sub>1'))"
@@ -3440,12 +3373,12 @@ by(simp add: X\<^sub>P\<^sub>e\<^sub>r\<^sub>s\<^sub>o\<^sub>n9\<sigma>\<^sub>1_
 lemma oid9\<sigma>\<^sub>1\<sigma>\<^sub>1'_\<sigma>\<^sub>1'_OclIsMaintained : "(\<sigma>\<^sub>1 , \<sigma>\<^sub>1') \<Turnstile> (OclIsMaintained (X\<^sub>P\<^sub>e\<^sub>r\<^sub>s\<^sub>o\<^sub>n9\<sigma>\<^sub>1'))"
 by(simp add: X\<^sub>P\<^sub>e\<^sub>r\<^sub>s\<^sub>o\<^sub>n9\<sigma>\<^sub>1'_def X\<^sub>P\<^sub>e\<^sub>r\<^sub>s\<^sub>o\<^sub>n9\<^sub>P\<^sub>e\<^sub>r\<^sub>s\<^sub>o\<^sub>n_def OclIsMaintained_def OclValid_def \<sigma>\<^sub>1_def \<sigma>\<^sub>1'_def oid_of_option_def oid1_def oid2_def oid3_def oid4_def oid5_def oid6_def oid7_def oid8_def oid9_def oid_of_typeoid\<^sub>O\<^sub>c\<^sub>l\<^sub>A\<^sub>n\<^sub>y_def oid_of_typeoid\<^sub>P\<^sub>e\<^sub>r\<^sub>s\<^sub>o\<^sub>n_def)
 
-(* 157 ************************************ 899 + 6 *)
+(* 150 ************************************ 881 + 6 *)
 generation_syntax [ shallow (generation_semantics [ design ]) ]
-setup{* (Generation_mode.update_compiler_config ((K (let open OCL in Ocl_compiler_config_ext (true, NONE, Oids ((Code_Numeral.Nat 0), (Code_Numeral.Nat 1), (Code_Numeral.Nat 10)), I ((Code_Numeral.Nat 0), (Code_Numeral.Nat 0)), Gen_design, SOME (OclClass ((String.explode "OclAny"), nil, uncurry cons (OclClass ((String.explode "Galaxy"), uncurry cons (I ((String.explode "sound"), OclTy_raw ((String.explode "unit"))), uncurry cons (I ((String.explode "moving"), OclTy_raw ((String.explode "bool"))), nil)), uncurry cons (OclClass ((String.explode "Planet"), uncurry cons (I ((String.explode "wormhole"), OclTy_raw ((String.explode "nat"))), uncurry cons (I ((String.explode "weight"), OclTy_raw ((String.explode "int"))), nil)), uncurry cons (OclClass ((String.explode "Person"), uncurry cons (I ((String.explode "boss"), OclTy_class (Ocl_ty_class_ext ((String.explode "oid"), (Code_Numeral.Nat 0), (Code_Numeral.Nat 2), Ocl_ty_class_node_ext ((Code_Numeral.Nat 0), OclMult (uncurry cons (I (Mult_star, NONE), nil)), NONE, (String.explode "Person"), ()), Ocl_ty_class_node_ext ((Code_Numeral.Nat 1), OclMult (uncurry cons (I (Mult_nat ((Code_Numeral.Nat 0)), SOME (Mult_nat ((Code_Numeral.Nat 1)))), nil)), SOME ((String.explode "boss")), (String.explode "Person"), ()), ()))), uncurry cons (I ((String.explode "salary"), OclTy_raw ((String.explode "int"))), nil)), nil), nil)), nil)), nil))), uncurry cons (OclAstDefPrePost (OclDefPP ((String.explode "\<sigma>\<^sub>1"), (String.explode "\<sigma>\<^sub>1'"))), uncurry cons (OclAstDefState (OclDefSt ((String.explode "\<sigma>\<^sub>0"), nil)), uncurry cons (OclAstDefState (OclDefSt ((String.explode "\<sigma>\<^sub>1'"), uncurry cons (OclDefCoreBinding ((String.explode "X\<^sub>P\<^sub>e\<^sub>r\<^sub>s\<^sub>o\<^sub>n1")), uncurry cons (OclDefCoreBinding ((String.explode "X\<^sub>P\<^sub>e\<^sub>r\<^sub>s\<^sub>o\<^sub>n2")), uncurry cons (OclDefCoreBinding ((String.explode "X\<^sub>P\<^sub>e\<^sub>r\<^sub>s\<^sub>o\<^sub>n3")), uncurry cons (OclDefCoreBinding ((String.explode "X\<^sub>P\<^sub>e\<^sub>r\<^sub>s\<^sub>o\<^sub>n4")), uncurry cons (OclDefCoreSkip, uncurry cons (OclDefCoreBinding ((String.explode "X\<^sub>P\<^sub>e\<^sub>r\<^sub>s\<^sub>o\<^sub>n6")), uncurry cons (OclDefCoreBinding ((String.explode "X\<^sub>P\<^sub>e\<^sub>r\<^sub>s\<^sub>o\<^sub>n7")), uncurry cons (OclDefCoreBinding ((String.explode "X\<^sub>P\<^sub>e\<^sub>r\<^sub>s\<^sub>o\<^sub>n8")), uncurry cons (OclDefCoreBinding ((String.explode "X\<^sub>P\<^sub>e\<^sub>r\<^sub>s\<^sub>o\<^sub>n9")), nil))))))))))), uncurry cons (OclAstDefState (OclDefSt ((String.explode "\<sigma>\<^sub>1"), uncurry cons (OclDefCoreAdd (Ocl_instance_single_ext ((String.explode ""), (String.explode "Person"), OclAttrNoCast (uncurry cons (I ((String.explode "salary"), Shall_base (ShallB_str ((String.explode "1000")))), uncurry cons (I ((String.explode "boss"), Shall_base (ShallB_self (Oid ((Code_Numeral.Nat 1))))), nil))), ())), uncurry cons (OclDefCoreAdd (Ocl_instance_single_ext ((String.explode ""), (String.explode "Person"), OclAttrNoCast (uncurry cons (I ((String.explode "salary"), Shall_base (ShallB_str ((String.explode "1200")))), nil)), ())), uncurry cons (OclDefCoreSkip, uncurry cons (OclDefCoreAdd (Ocl_instance_single_ext ((String.explode ""), (String.explode "Person"), OclAttrNoCast (uncurry cons (I ((String.explode "salary"), Shall_base (ShallB_str ((String.explode "2600")))), uncurry cons (I ((String.explode "boss"), Shall_base (ShallB_self (Oid ((Code_Numeral.Nat 4))))), nil))), ())), uncurry cons (OclDefCoreBinding ((String.explode "X\<^sub>P\<^sub>e\<^sub>r\<^sub>s\<^sub>o\<^sub>n5")), uncurry cons (OclDefCoreAdd (Ocl_instance_single_ext ((String.explode ""), (String.explode "Person"), OclAttrNoCast (uncurry cons (I ((String.explode "salary"), Shall_base (ShallB_str ((String.explode "2300")))), uncurry cons (I ((String.explode "boss"), Shall_base (ShallB_self (Oid ((Code_Numeral.Nat 3))))), nil))), ())), uncurry cons (OclDefCoreSkip, uncurry cons (OclDefCoreSkip, uncurry cons (OclDefCoreBinding ((String.explode "X\<^sub>P\<^sub>e\<^sub>r\<^sub>s\<^sub>o\<^sub>n9")), nil))))))))))), uncurry cons (OclAstInstance (OclInstance (uncurry cons (Ocl_instance_single_ext ((String.explode "X\<^sub>P\<^sub>e\<^sub>r\<^sub>s\<^sub>o\<^sub>n1"), (String.explode "Person"), OclAttrNoCast (uncurry cons (I ((String.explode "salary"), Shall_base (ShallB_str ((String.explode "1300")))), uncurry cons (I ((String.explode "boss"), Shall_base (ShallB_str ((String.explode "X\<^sub>P\<^sub>e\<^sub>r\<^sub>s\<^sub>o\<^sub>n2")))), nil))), ()), uncurry cons (Ocl_instance_single_ext ((String.explode "X\<^sub>P\<^sub>e\<^sub>r\<^sub>s\<^sub>o\<^sub>n2"), (String.explode "Person"), OclAttrNoCast (uncurry cons (I ((String.explode "salary"), Shall_base (ShallB_str ((String.explode "1800")))), uncurry cons (I ((String.explode "boss"), Shall_base (ShallB_str ((String.explode "X\<^sub>P\<^sub>e\<^sub>r\<^sub>s\<^sub>o\<^sub>n2")))), nil))), ()), uncurry cons (Ocl_instance_single_ext ((String.explode "X\<^sub>P\<^sub>e\<^sub>r\<^sub>s\<^sub>o\<^sub>n3"), (String.explode "Person"), OclAttrNoCast (nil), ()), uncurry cons (Ocl_instance_single_ext ((String.explode "X\<^sub>P\<^sub>e\<^sub>r\<^sub>s\<^sub>o\<^sub>n4"), (String.explode "Person"), OclAttrNoCast (uncurry cons (I ((String.explode "salary"), Shall_base (ShallB_str ((String.explode "2900")))), nil)), ()), uncurry cons (Ocl_instance_single_ext ((String.explode "X\<^sub>P\<^sub>e\<^sub>r\<^sub>s\<^sub>o\<^sub>n5"), (String.explode "Person"), OclAttrNoCast (uncurry cons (I ((String.explode "salary"), Shall_base (ShallB_str ((String.explode "3500")))), nil)), ()), uncurry cons (Ocl_instance_single_ext ((String.explode "X\<^sub>P\<^sub>e\<^sub>r\<^sub>s\<^sub>o\<^sub>n6"), (String.explode "Person"), OclAttrNoCast (uncurry cons (I ((String.explode "salary"), Shall_base (ShallB_str ((String.explode "2500")))), uncurry cons (I ((String.explode "boss"), Shall_base (ShallB_str ((String.explode "X\<^sub>P\<^sub>e\<^sub>r\<^sub>s\<^sub>o\<^sub>n7")))), nil))), ()), uncurry cons (Ocl_instance_single_ext ((String.explode "X\<^sub>P\<^sub>e\<^sub>r\<^sub>s\<^sub>o\<^sub>n7"), (String.explode "OclAny"), OclAttrCast ((String.explode "Person"), OclAttrNoCast (uncurry cons (I ((String.explode "salary"), Shall_base (ShallB_str ((String.explode "3200")))), uncurry cons (I ((String.explode "boss"), Shall_base (ShallB_str ((String.explode "X\<^sub>P\<^sub>e\<^sub>r\<^sub>s\<^sub>o\<^sub>n7")))), nil))), nil), ()), uncurry cons (Ocl_instance_single_ext ((String.explode "X\<^sub>P\<^sub>e\<^sub>r\<^sub>s\<^sub>o\<^sub>n8"), (String.explode "OclAny"), OclAttrNoCast (nil), ()), uncurry cons (Ocl_instance_single_ext ((String.explode "X\<^sub>P\<^sub>e\<^sub>r\<^sub>s\<^sub>o\<^sub>n9"), (String.explode "Person"), OclAttrNoCast (uncurry cons (I ((String.explode "salary"), Shall_base (ShallB_str ((String.explode "0")))), nil)), ()), nil))))))))))), uncurry cons (OclAstDefInt (OclDefI (uncurry cons ((String.explode "1000"), uncurry cons ((String.explode "1200"), uncurry cons ((String.explode "1300"), uncurry cons ((String.explode "1800"), uncurry cons ((String.explode "2600"), uncurry cons ((String.explode "2900"), uncurry cons ((String.explode "3200"), uncurry cons ((String.explode "3500"), nil)))))))))), uncurry cons (OclAstClassRaw (Ocl_class_raw_ext ((String.explode "Galaxy"), uncurry cons (I ((String.explode "sound"), OclTy_raw ((String.explode "unit"))), uncurry cons (I ((String.explode "moving"), OclTy_raw ((String.explode "bool"))), nil)), NONE, ())), uncurry cons (OclAstClassRaw (Ocl_class_raw_ext ((String.explode "Planet"), uncurry cons (I ((String.explode "wormhole"), OclTy_raw ((String.explode "nat"))), uncurry cons (I ((String.explode "weight"), OclTy_raw ((String.explode "int"))), nil)), SOME ((String.explode "Galaxy")), ())), uncurry cons (OclAstAssociation (Ocl_association_ext (OclAssTy_association, uncurry cons (I ((String.explode "Person"), I (OclMult (uncurry cons (I (Mult_star, NONE), nil)), NONE)), uncurry cons (I ((String.explode "Person"), I (OclMult (uncurry cons (I (Mult_nat ((Code_Numeral.Nat 0)), SOME (Mult_nat ((Code_Numeral.Nat 1)))), nil)), SOME ((String.explode "boss")))), nil)), ())), uncurry cons (OclAstClassRaw (Ocl_class_raw_ext ((String.explode "Person"), uncurry cons (I ((String.explode "salary"), OclTy_raw ((String.explode "int"))), nil), SOME ((String.explode "Planet")), ())), nil)))))))))), uncurry cons (I ((String.explode "X\<^sub>P\<^sub>e\<^sub>r\<^sub>s\<^sub>o\<^sub>n9"), I (Ocl_instance_single_ext ((String.explode "X\<^sub>P\<^sub>e\<^sub>r\<^sub>s\<^sub>o\<^sub>n9"), (String.explode "Person"), OclAttrNoCast (uncurry cons (I ((String.explode "salary"), Shall_base (ShallB_str ((String.explode "0")))), nil)), ()), Oid ((Code_Numeral.Nat 9)))), uncurry cons (I ((String.explode "X\<^sub>P\<^sub>e\<^sub>r\<^sub>s\<^sub>o\<^sub>n8"), I (Ocl_instance_single_ext ((String.explode "X\<^sub>P\<^sub>e\<^sub>r\<^sub>s\<^sub>o\<^sub>n8"), (String.explode "OclAny"), OclAttrNoCast (nil), ()), Oid ((Code_Numeral.Nat 8)))), uncurry cons (I ((String.explode "X\<^sub>P\<^sub>e\<^sub>r\<^sub>s\<^sub>o\<^sub>n7"), I (Ocl_instance_single_ext ((String.explode "X\<^sub>P\<^sub>e\<^sub>r\<^sub>s\<^sub>o\<^sub>n7"), (String.explode "OclAny"), OclAttrCast ((String.explode "Person"), OclAttrNoCast (uncurry cons (I ((String.explode "salary"), Shall_base (ShallB_str ((String.explode "3200")))), uncurry cons (I ((String.explode "boss"), Shall_base (ShallB_str ((String.explode "X\<^sub>P\<^sub>e\<^sub>r\<^sub>s\<^sub>o\<^sub>n7")))), nil))), nil), ()), Oid ((Code_Numeral.Nat 7)))), uncurry cons (I ((String.explode "X\<^sub>P\<^sub>e\<^sub>r\<^sub>s\<^sub>o\<^sub>n6"), I (Ocl_instance_single_ext ((String.explode "X\<^sub>P\<^sub>e\<^sub>r\<^sub>s\<^sub>o\<^sub>n6"), (String.explode "Person"), OclAttrNoCast (uncurry cons (I ((String.explode "salary"), Shall_base (ShallB_str ((String.explode "2500")))), uncurry cons (I ((String.explode "boss"), Shall_base (ShallB_str ((String.explode "X\<^sub>P\<^sub>e\<^sub>r\<^sub>s\<^sub>o\<^sub>n7")))), nil))), ()), Oid ((Code_Numeral.Nat 6)))), uncurry cons (I ((String.explode "X\<^sub>P\<^sub>e\<^sub>r\<^sub>s\<^sub>o\<^sub>n5"), I (Ocl_instance_single_ext ((String.explode "X\<^sub>P\<^sub>e\<^sub>r\<^sub>s\<^sub>o\<^sub>n5"), (String.explode "Person"), OclAttrNoCast (uncurry cons (I ((String.explode "salary"), Shall_base (ShallB_str ((String.explode "3500")))), nil)), ()), Oid ((Code_Numeral.Nat 5)))), uncurry cons (I ((String.explode "X\<^sub>P\<^sub>e\<^sub>r\<^sub>s\<^sub>o\<^sub>n4"), I (Ocl_instance_single_ext ((String.explode "X\<^sub>P\<^sub>e\<^sub>r\<^sub>s\<^sub>o\<^sub>n4"), (String.explode "Person"), OclAttrNoCast (uncurry cons (I ((String.explode "salary"), Shall_base (ShallB_str ((String.explode "2900")))), nil)), ()), Oid ((Code_Numeral.Nat 4)))), uncurry cons (I ((String.explode "X\<^sub>P\<^sub>e\<^sub>r\<^sub>s\<^sub>o\<^sub>n3"), I (Ocl_instance_single_ext ((String.explode "X\<^sub>P\<^sub>e\<^sub>r\<^sub>s\<^sub>o\<^sub>n3"), (String.explode "Person"), OclAttrNoCast (nil), ()), Oid ((Code_Numeral.Nat 3)))), uncurry cons (I ((String.explode "X\<^sub>P\<^sub>e\<^sub>r\<^sub>s\<^sub>o\<^sub>n2"), I (Ocl_instance_single_ext ((String.explode "X\<^sub>P\<^sub>e\<^sub>r\<^sub>s\<^sub>o\<^sub>n2"), (String.explode "Person"), OclAttrNoCast (uncurry cons (I ((String.explode "salary"), Shall_base (ShallB_str ((String.explode "1800")))), uncurry cons (I ((String.explode "boss"), Shall_base (ShallB_str ((String.explode "X\<^sub>P\<^sub>e\<^sub>r\<^sub>s\<^sub>o\<^sub>n2")))), nil))), ()), Oid ((Code_Numeral.Nat 2)))), uncurry cons (I ((String.explode "X\<^sub>P\<^sub>e\<^sub>r\<^sub>s\<^sub>o\<^sub>n1"), I (Ocl_instance_single_ext ((String.explode "X\<^sub>P\<^sub>e\<^sub>r\<^sub>s\<^sub>o\<^sub>n1"), (String.explode "Person"), OclAttrNoCast (uncurry cons (I ((String.explode "salary"), Shall_base (ShallB_str ((String.explode "1300")))), uncurry cons (I ((String.explode "boss"), Shall_base (ShallB_str ((String.explode "X\<^sub>P\<^sub>e\<^sub>r\<^sub>s\<^sub>o\<^sub>n2")))), nil))), ()), Oid ((Code_Numeral.Nat 1)))), nil))))))))), uncurry cons (I ((String.explode "\<sigma>\<^sub>0"), nil), uncurry cons (I ((String.explode "\<sigma>\<^sub>1'"), uncurry cons (I (Oids ((Code_Numeral.Nat 0), (Code_Numeral.Nat 1), (Code_Numeral.Nat 1)), OclDefCoreBinding (I ((String.explode "X\<^sub>P\<^sub>e\<^sub>r\<^sub>s\<^sub>o\<^sub>n1"), Ocl_instance_single_ext ((String.explode "X\<^sub>P\<^sub>e\<^sub>r\<^sub>s\<^sub>o\<^sub>n1"), (String.explode "Person"), OclAttrNoCast (uncurry cons (I ((String.explode "salary"), Shall_base (ShallB_str ((String.explode "1300")))), uncurry cons (I ((String.explode "boss"), Shall_base (ShallB_str ((String.explode "X\<^sub>P\<^sub>e\<^sub>r\<^sub>s\<^sub>o\<^sub>n2")))), nil))), ())))), uncurry cons (I (Oids ((Code_Numeral.Nat 0), (Code_Numeral.Nat 1), (Code_Numeral.Nat 2)), OclDefCoreBinding (I ((String.explode "X\<^sub>P\<^sub>e\<^sub>r\<^sub>s\<^sub>o\<^sub>n2"), Ocl_instance_single_ext ((String.explode "X\<^sub>P\<^sub>e\<^sub>r\<^sub>s\<^sub>o\<^sub>n2"), (String.explode "Person"), OclAttrNoCast (uncurry cons (I ((String.explode "salary"), Shall_base (ShallB_str ((String.explode "1800")))), uncurry cons (I ((String.explode "boss"), Shall_base (ShallB_str ((String.explode "X\<^sub>P\<^sub>e\<^sub>r\<^sub>s\<^sub>o\<^sub>n2")))), nil))), ())))), uncurry cons (I (Oids ((Code_Numeral.Nat 0), (Code_Numeral.Nat 1), (Code_Numeral.Nat 3)), OclDefCoreBinding (I ((String.explode "X\<^sub>P\<^sub>e\<^sub>r\<^sub>s\<^sub>o\<^sub>n3"), Ocl_instance_single_ext ((String.explode "X\<^sub>P\<^sub>e\<^sub>r\<^sub>s\<^sub>o\<^sub>n3"), (String.explode "Person"), OclAttrNoCast (nil), ())))), uncurry cons (I (Oids ((Code_Numeral.Nat 0), (Code_Numeral.Nat 1), (Code_Numeral.Nat 4)), OclDefCoreBinding (I ((String.explode "X\<^sub>P\<^sub>e\<^sub>r\<^sub>s\<^sub>o\<^sub>n4"), Ocl_instance_single_ext ((String.explode "X\<^sub>P\<^sub>e\<^sub>r\<^sub>s\<^sub>o\<^sub>n4"), (String.explode "Person"), OclAttrNoCast (uncurry cons (I ((String.explode "salary"), Shall_base (ShallB_str ((String.explode "2900")))), nil)), ())))), uncurry cons (I (Oids ((Code_Numeral.Nat 0), (Code_Numeral.Nat 1), (Code_Numeral.Nat 6)), OclDefCoreBinding (I ((String.explode "X\<^sub>P\<^sub>e\<^sub>r\<^sub>s\<^sub>o\<^sub>n6"), Ocl_instance_single_ext ((String.explode "X\<^sub>P\<^sub>e\<^sub>r\<^sub>s\<^sub>o\<^sub>n6"), (String.explode "Person"), OclAttrNoCast (uncurry cons (I ((String.explode "salary"), Shall_base (ShallB_str ((String.explode "2500")))), uncurry cons (I ((String.explode "boss"), Shall_base (ShallB_str ((String.explode "X\<^sub>P\<^sub>e\<^sub>r\<^sub>s\<^sub>o\<^sub>n7")))), nil))), ())))), uncurry cons (I (Oids ((Code_Numeral.Nat 0), (Code_Numeral.Nat 1), (Code_Numeral.Nat 7)), OclDefCoreBinding (I ((String.explode "X\<^sub>P\<^sub>e\<^sub>r\<^sub>s\<^sub>o\<^sub>n7"), Ocl_instance_single_ext ((String.explode "X\<^sub>P\<^sub>e\<^sub>r\<^sub>s\<^sub>o\<^sub>n7"), (String.explode "OclAny"), OclAttrCast ((String.explode "Person"), OclAttrNoCast (uncurry cons (I ((String.explode "salary"), Shall_base (ShallB_str ((String.explode "3200")))), uncurry cons (I ((String.explode "boss"), Shall_base (ShallB_str ((String.explode "X\<^sub>P\<^sub>e\<^sub>r\<^sub>s\<^sub>o\<^sub>n7")))), nil))), nil), ())))), uncurry cons (I (Oids ((Code_Numeral.Nat 0), (Code_Numeral.Nat 1), (Code_Numeral.Nat 8)), OclDefCoreBinding (I ((String.explode "X\<^sub>P\<^sub>e\<^sub>r\<^sub>s\<^sub>o\<^sub>n8"), Ocl_instance_single_ext ((String.explode "X\<^sub>P\<^sub>e\<^sub>r\<^sub>s\<^sub>o\<^sub>n8"), (String.explode "OclAny"), OclAttrNoCast (nil), ())))), uncurry cons (I (Oids ((Code_Numeral.Nat 0), (Code_Numeral.Nat 1), (Code_Numeral.Nat 9)), OclDefCoreBinding (I ((String.explode "X\<^sub>P\<^sub>e\<^sub>r\<^sub>s\<^sub>o\<^sub>n9"), Ocl_instance_single_ext ((String.explode "X\<^sub>P\<^sub>e\<^sub>r\<^sub>s\<^sub>o\<^sub>n9"), (String.explode "Person"), OclAttrNoCast (uncurry cons (I ((String.explode "salary"), Shall_base (ShallB_str ((String.explode "0")))), nil)), ())))), nil))))))))), uncurry cons (I ((String.explode "\<sigma>\<^sub>1"), uncurry cons (I (Oids ((Code_Numeral.Nat 0), (Code_Numeral.Nat 1), (Code_Numeral.Nat 1)), OclDefCoreAdd (Ocl_instance_single_ext ((String.explode ""), (String.explode "Person"), OclAttrNoCast (uncurry cons (I ((String.explode "salary"), Shall_base (ShallB_str ((String.explode "1000")))), uncurry cons (I ((String.explode "boss"), Shall_base (ShallB_self (Oid ((Code_Numeral.Nat 1))))), nil))), ()))), uncurry cons (I (Oids ((Code_Numeral.Nat 0), (Code_Numeral.Nat 1), (Code_Numeral.Nat 2)), OclDefCoreAdd (Ocl_instance_single_ext ((String.explode ""), (String.explode "Person"), OclAttrNoCast (uncurry cons (I ((String.explode "salary"), Shall_base (ShallB_str ((String.explode "1200")))), nil)), ()))), uncurry cons (I (Oids ((Code_Numeral.Nat 0), (Code_Numeral.Nat 1), (Code_Numeral.Nat 4)), OclDefCoreAdd (Ocl_instance_single_ext ((String.explode ""), (String.explode "Person"), OclAttrNoCast (uncurry cons (I ((String.explode "salary"), Shall_base (ShallB_str ((String.explode "2600")))), uncurry cons (I ((String.explode "boss"), Shall_base (ShallB_self (Oid ((Code_Numeral.Nat 4))))), nil))), ()))), uncurry cons (I (Oids ((Code_Numeral.Nat 0), (Code_Numeral.Nat 1), (Code_Numeral.Nat 5)), OclDefCoreBinding (I ((String.explode "X\<^sub>P\<^sub>e\<^sub>r\<^sub>s\<^sub>o\<^sub>n5"), Ocl_instance_single_ext ((String.explode "X\<^sub>P\<^sub>e\<^sub>r\<^sub>s\<^sub>o\<^sub>n5"), (String.explode "Person"), OclAttrNoCast (uncurry cons (I ((String.explode "salary"), Shall_base (ShallB_str ((String.explode "3500")))), nil)), ())))), uncurry cons (I (Oids ((Code_Numeral.Nat 0), (Code_Numeral.Nat 1), (Code_Numeral.Nat 6)), OclDefCoreAdd (Ocl_instance_single_ext ((String.explode ""), (String.explode "Person"), OclAttrNoCast (uncurry cons (I ((String.explode "salary"), Shall_base (ShallB_str ((String.explode "2300")))), uncurry cons (I ((String.explode "boss"), Shall_base (ShallB_self (Oid ((Code_Numeral.Nat 3))))), nil))), ()))), uncurry cons (I (Oids ((Code_Numeral.Nat 0), (Code_Numeral.Nat 1), (Code_Numeral.Nat 9)), OclDefCoreBinding (I ((String.explode "X\<^sub>P\<^sub>e\<^sub>r\<^sub>s\<^sub>o\<^sub>n9"), Ocl_instance_single_ext ((String.explode "X\<^sub>P\<^sub>e\<^sub>r\<^sub>s\<^sub>o\<^sub>n9"), (String.explode "Person"), OclAttrNoCast (uncurry cons (I ((String.explode "salary"), Shall_base (ShallB_str ((String.explode "0")))), nil)), ())))), nil))))))), nil))), true, false, I (uncurry cons ((String.explode "dot\<C>\<O>\<N>\<T>\<E>\<N>\<T>\<S>at_pre"), uncurry cons ((String.explode "dot\<M>\<O>\<V>\<I>\<N>\<G>at_pre"), uncurry cons ((String.explode "dot\<S>\<O>\<U>\<N>\<D>at_pre"), uncurry cons ((String.explode "dot\<W>\<E>\<I>\<G>\<H>\<T>at_pre"), uncurry cons ((String.explode "dot\<W>\<O>\<R>\<M>\<H>\<O>\<L>\<E>at_pre"), uncurry cons ((String.explode "dot\<S>\<A>\<L>\<A>\<R>\<Y>at_pre"), uncurry cons ((String.explode "dot_0_\<B>\<O>\<S>\<S>at_pre"), nil))))))), uncurry cons ((String.explode "dot\<C>\<O>\<N>\<T>\<E>\<N>\<T>\<S>"), uncurry cons ((String.explode "dot\<M>\<O>\<V>\<I>\<N>\<G>"), uncurry cons ((String.explode "dot\<S>\<O>\<U>\<N>\<D>"), uncurry cons ((String.explode "dot\<W>\<E>\<I>\<G>\<H>\<T>"), uncurry cons ((String.explode "dot\<W>\<O>\<R>\<M>\<H>\<O>\<L>\<E>"), uncurry cons ((String.explode "dot\<S>\<A>\<L>\<A>\<R>\<Y>"), uncurry cons ((String.explode "dot_0_\<B>\<O>\<S>\<S>"), nil)))))))), ()) end)))) *}
-consts dot\<C>\<O>\<N>\<T>\<E>\<N>\<T>\<S> :: "Person \<Rightarrow> Set_int" ("(_) .contents'(')")
-consts dot\<C>\<O>\<N>\<T>\<E>\<N>\<T>\<S>at_pre :: "Person \<Rightarrow> Set_int" ("(_) .contents@pre'(')")
-Context[shallow] Person :: contents () : Set(int)
+setup{* (Generation_mode.update_compiler_config ((K (let open OCL in Ocl_compiler_config_ext (true, NONE, Oids ((Code_Numeral.Nat 0), (Code_Numeral.Nat 1), (Code_Numeral.Nat 10)), I ((Code_Numeral.Nat 0), (Code_Numeral.Nat 0)), Gen_design, SOME (OclClass ((String.explode "OclAny"), nil, uncurry cons (OclClass ((String.explode "Galaxy"), uncurry cons (I ((String.explode "sound"), OclTy_base_void), uncurry cons (I ((String.explode "moving"), OclTy_base_boolean), nil)), uncurry cons (OclClass ((String.explode "Planet"), uncurry cons (I ((String.explode "wormhole"), OclTy_base_unlimitednatural), uncurry cons (I ((String.explode "weight"), OclTy_base_integer), nil)), uncurry cons (OclClass ((String.explode "Person"), uncurry cons (I ((String.explode "boss"), OclTy_class (Ocl_ty_class_ext ((String.explode "oid"), (Code_Numeral.Nat 0), (Code_Numeral.Nat 2), Ocl_ty_class_node_ext ((Code_Numeral.Nat 0), OclMult (uncurry cons (I (Mult_star, NONE), nil)), NONE, (String.explode "Person"), ()), Ocl_ty_class_node_ext ((Code_Numeral.Nat 1), OclMult (uncurry cons (I (Mult_nat ((Code_Numeral.Nat 0)), SOME (Mult_nat ((Code_Numeral.Nat 1)))), nil)), SOME ((String.explode "boss")), (String.explode "Person"), ()), ()))), uncurry cons (I ((String.explode "salary"), OclTy_base_integer), nil)), nil), nil)), nil)), nil))), uncurry cons (OclAstDefPrePost (OclDefPP ((String.explode "\<sigma>\<^sub>1"), (String.explode "\<sigma>\<^sub>1'"))), uncurry cons (OclAstDefState (OclDefSt ((String.explode "\<sigma>\<^sub>1'"), uncurry cons (OclDefCoreBinding ((String.explode "X\<^sub>P\<^sub>e\<^sub>r\<^sub>s\<^sub>o\<^sub>n1")), uncurry cons (OclDefCoreBinding ((String.explode "X\<^sub>P\<^sub>e\<^sub>r\<^sub>s\<^sub>o\<^sub>n2")), uncurry cons (OclDefCoreBinding ((String.explode "X\<^sub>P\<^sub>e\<^sub>r\<^sub>s\<^sub>o\<^sub>n3")), uncurry cons (OclDefCoreBinding ((String.explode "X\<^sub>P\<^sub>e\<^sub>r\<^sub>s\<^sub>o\<^sub>n4")), uncurry cons (OclDefCoreSkip, uncurry cons (OclDefCoreBinding ((String.explode "X\<^sub>P\<^sub>e\<^sub>r\<^sub>s\<^sub>o\<^sub>n6")), uncurry cons (OclDefCoreBinding ((String.explode "X\<^sub>P\<^sub>e\<^sub>r\<^sub>s\<^sub>o\<^sub>n7")), uncurry cons (OclDefCoreBinding ((String.explode "X\<^sub>P\<^sub>e\<^sub>r\<^sub>s\<^sub>o\<^sub>n8")), uncurry cons (OclDefCoreBinding ((String.explode "X\<^sub>P\<^sub>e\<^sub>r\<^sub>s\<^sub>o\<^sub>n9")), nil))))))))))), uncurry cons (OclAstDefState (OclDefSt ((String.explode "\<sigma>\<^sub>1"), uncurry cons (OclDefCoreAdd (Ocl_instance_single_ext ((String.explode ""), (String.explode "Person"), OclAttrNoCast (uncurry cons (I ((String.explode "salary"), Shall_base (ShallB_term (OclDefInteger ((String.explode "1000"))))), uncurry cons (I ((String.explode "boss"), Shall_base (ShallB_self (Oid ((Code_Numeral.Nat 1))))), nil))), ())), uncurry cons (OclDefCoreAdd (Ocl_instance_single_ext ((String.explode ""), (String.explode "Person"), OclAttrNoCast (uncurry cons (I ((String.explode "salary"), Shall_base (ShallB_term (OclDefInteger ((String.explode "1200"))))), nil)), ())), uncurry cons (OclDefCoreSkip, uncurry cons (OclDefCoreAdd (Ocl_instance_single_ext ((String.explode ""), (String.explode "Person"), OclAttrNoCast (uncurry cons (I ((String.explode "salary"), Shall_base (ShallB_term (OclDefInteger ((String.explode "2600"))))), uncurry cons (I ((String.explode "boss"), Shall_base (ShallB_self (Oid ((Code_Numeral.Nat 4))))), nil))), ())), uncurry cons (OclDefCoreBinding ((String.explode "X\<^sub>P\<^sub>e\<^sub>r\<^sub>s\<^sub>o\<^sub>n5")), uncurry cons (OclDefCoreAdd (Ocl_instance_single_ext ((String.explode ""), (String.explode "Person"), OclAttrNoCast (uncurry cons (I ((String.explode "salary"), Shall_base (ShallB_term (OclDefInteger ((String.explode "2300"))))), uncurry cons (I ((String.explode "boss"), Shall_base (ShallB_self (Oid ((Code_Numeral.Nat 3))))), nil))), ())), uncurry cons (OclDefCoreSkip, uncurry cons (OclDefCoreSkip, uncurry cons (OclDefCoreBinding ((String.explode "X\<^sub>P\<^sub>e\<^sub>r\<^sub>s\<^sub>o\<^sub>n9")), nil))))))))))), uncurry cons (OclAstInstance (OclInstance (uncurry cons (Ocl_instance_single_ext ((String.explode "X\<^sub>P\<^sub>e\<^sub>r\<^sub>s\<^sub>o\<^sub>n1"), (String.explode "Person"), OclAttrNoCast (uncurry cons (I ((String.explode "salary"), Shall_base (ShallB_term (OclDefInteger ((String.explode "1300"))))), uncurry cons (I ((String.explode "boss"), Shall_base (ShallB_str ((String.explode "X\<^sub>P\<^sub>e\<^sub>r\<^sub>s\<^sub>o\<^sub>n2")))), nil))), ()), uncurry cons (Ocl_instance_single_ext ((String.explode "X\<^sub>P\<^sub>e\<^sub>r\<^sub>s\<^sub>o\<^sub>n2"), (String.explode "Person"), OclAttrNoCast (uncurry cons (I ((String.explode "salary"), Shall_base (ShallB_term (OclDefInteger ((String.explode "1800"))))), uncurry cons (I ((String.explode "boss"), Shall_base (ShallB_str ((String.explode "X\<^sub>P\<^sub>e\<^sub>r\<^sub>s\<^sub>o\<^sub>n2")))), nil))), ()), uncurry cons (Ocl_instance_single_ext ((String.explode "X\<^sub>P\<^sub>e\<^sub>r\<^sub>s\<^sub>o\<^sub>n3"), (String.explode "Person"), OclAttrNoCast (nil), ()), uncurry cons (Ocl_instance_single_ext ((String.explode "X\<^sub>P\<^sub>e\<^sub>r\<^sub>s\<^sub>o\<^sub>n4"), (String.explode "Person"), OclAttrNoCast (uncurry cons (I ((String.explode "salary"), Shall_base (ShallB_term (OclDefInteger ((String.explode "2900"))))), nil)), ()), uncurry cons (Ocl_instance_single_ext ((String.explode "X\<^sub>P\<^sub>e\<^sub>r\<^sub>s\<^sub>o\<^sub>n5"), (String.explode "Person"), OclAttrNoCast (uncurry cons (I ((String.explode "salary"), Shall_base (ShallB_term (OclDefInteger ((String.explode "3500"))))), nil)), ()), uncurry cons (Ocl_instance_single_ext ((String.explode "X\<^sub>P\<^sub>e\<^sub>r\<^sub>s\<^sub>o\<^sub>n6"), (String.explode "Person"), OclAttrNoCast (uncurry cons (I ((String.explode "salary"), Shall_base (ShallB_term (OclDefInteger ((String.explode "2500"))))), uncurry cons (I ((String.explode "boss"), Shall_base (ShallB_str ((String.explode "X\<^sub>P\<^sub>e\<^sub>r\<^sub>s\<^sub>o\<^sub>n7")))), nil))), ()), uncurry cons (Ocl_instance_single_ext ((String.explode "X\<^sub>P\<^sub>e\<^sub>r\<^sub>s\<^sub>o\<^sub>n7"), (String.explode "OclAny"), OclAttrCast ((String.explode "Person"), OclAttrNoCast (uncurry cons (I ((String.explode "salary"), Shall_base (ShallB_term (OclDefInteger ((String.explode "3200"))))), uncurry cons (I ((String.explode "boss"), Shall_base (ShallB_str ((String.explode "X\<^sub>P\<^sub>e\<^sub>r\<^sub>s\<^sub>o\<^sub>n7")))), nil))), nil), ()), uncurry cons (Ocl_instance_single_ext ((String.explode "X\<^sub>P\<^sub>e\<^sub>r\<^sub>s\<^sub>o\<^sub>n8"), (String.explode "OclAny"), OclAttrNoCast (nil), ()), uncurry cons (Ocl_instance_single_ext ((String.explode "X\<^sub>P\<^sub>e\<^sub>r\<^sub>s\<^sub>o\<^sub>n9"), (String.explode "Person"), OclAttrNoCast (uncurry cons (I ((String.explode "salary"), Shall_base (ShallB_term (OclDefInteger ((String.explode "0"))))), nil)), ()), nil))))))))))), uncurry cons (OclAstClassRaw (Ocl_class_raw_ext ((String.explode "Galaxy"), uncurry cons (I ((String.explode "sound"), OclTy_base_void), uncurry cons (I ((String.explode "moving"), OclTy_base_boolean), nil)), nil, nil, NONE, ())), uncurry cons (OclAstClassRaw (Ocl_class_raw_ext ((String.explode "Planet"), uncurry cons (I ((String.explode "wormhole"), OclTy_base_unlimitednatural), uncurry cons (I ((String.explode "weight"), OclTy_base_integer), nil)), nil, nil, SOME ((String.explode "Galaxy")), ())), uncurry cons (OclAstAssociation (Ocl_association_ext (OclAssTy_association, uncurry cons (I ((String.explode "Person"), I (OclMult (uncurry cons (I (Mult_star, NONE), nil)), NONE)), uncurry cons (I ((String.explode "Person"), I (OclMult (uncurry cons (I (Mult_nat ((Code_Numeral.Nat 0)), SOME (Mult_nat ((Code_Numeral.Nat 1)))), nil)), SOME ((String.explode "boss")))), nil)), ())), uncurry cons (OclAstClassRaw (Ocl_class_raw_ext ((String.explode "Person"), uncurry cons (I ((String.explode "salary"), OclTy_base_integer), nil), nil, nil, SOME ((String.explode "Planet")), ())), nil)))))))), uncurry cons (I ((String.explode "X\<^sub>P\<^sub>e\<^sub>r\<^sub>s\<^sub>o\<^sub>n9"), I (Ocl_instance_single_ext ((String.explode "X\<^sub>P\<^sub>e\<^sub>r\<^sub>s\<^sub>o\<^sub>n9"), (String.explode "Person"), OclAttrNoCast (uncurry cons (I ((String.explode "salary"), Shall_base (ShallB_term (OclDefInteger ((String.explode "0"))))), nil)), ()), Oid ((Code_Numeral.Nat 9)))), uncurry cons (I ((String.explode "X\<^sub>P\<^sub>e\<^sub>r\<^sub>s\<^sub>o\<^sub>n8"), I (Ocl_instance_single_ext ((String.explode "X\<^sub>P\<^sub>e\<^sub>r\<^sub>s\<^sub>o\<^sub>n8"), (String.explode "OclAny"), OclAttrNoCast (nil), ()), Oid ((Code_Numeral.Nat 8)))), uncurry cons (I ((String.explode "X\<^sub>P\<^sub>e\<^sub>r\<^sub>s\<^sub>o\<^sub>n7"), I (Ocl_instance_single_ext ((String.explode "X\<^sub>P\<^sub>e\<^sub>r\<^sub>s\<^sub>o\<^sub>n7"), (String.explode "OclAny"), OclAttrCast ((String.explode "Person"), OclAttrNoCast (uncurry cons (I ((String.explode "salary"), Shall_base (ShallB_term (OclDefInteger ((String.explode "3200"))))), uncurry cons (I ((String.explode "boss"), Shall_base (ShallB_str ((String.explode "X\<^sub>P\<^sub>e\<^sub>r\<^sub>s\<^sub>o\<^sub>n7")))), nil))), nil), ()), Oid ((Code_Numeral.Nat 7)))), uncurry cons (I ((String.explode "X\<^sub>P\<^sub>e\<^sub>r\<^sub>s\<^sub>o\<^sub>n6"), I (Ocl_instance_single_ext ((String.explode "X\<^sub>P\<^sub>e\<^sub>r\<^sub>s\<^sub>o\<^sub>n6"), (String.explode "Person"), OclAttrNoCast (uncurry cons (I ((String.explode "salary"), Shall_base (ShallB_term (OclDefInteger ((String.explode "2500"))))), uncurry cons (I ((String.explode "boss"), Shall_base (ShallB_str ((String.explode "X\<^sub>P\<^sub>e\<^sub>r\<^sub>s\<^sub>o\<^sub>n7")))), nil))), ()), Oid ((Code_Numeral.Nat 6)))), uncurry cons (I ((String.explode "X\<^sub>P\<^sub>e\<^sub>r\<^sub>s\<^sub>o\<^sub>n5"), I (Ocl_instance_single_ext ((String.explode "X\<^sub>P\<^sub>e\<^sub>r\<^sub>s\<^sub>o\<^sub>n5"), (String.explode "Person"), OclAttrNoCast (uncurry cons (I ((String.explode "salary"), Shall_base (ShallB_term (OclDefInteger ((String.explode "3500"))))), nil)), ()), Oid ((Code_Numeral.Nat 5)))), uncurry cons (I ((String.explode "X\<^sub>P\<^sub>e\<^sub>r\<^sub>s\<^sub>o\<^sub>n4"), I (Ocl_instance_single_ext ((String.explode "X\<^sub>P\<^sub>e\<^sub>r\<^sub>s\<^sub>o\<^sub>n4"), (String.explode "Person"), OclAttrNoCast (uncurry cons (I ((String.explode "salary"), Shall_base (ShallB_term (OclDefInteger ((String.explode "2900"))))), nil)), ()), Oid ((Code_Numeral.Nat 4)))), uncurry cons (I ((String.explode "X\<^sub>P\<^sub>e\<^sub>r\<^sub>s\<^sub>o\<^sub>n3"), I (Ocl_instance_single_ext ((String.explode "X\<^sub>P\<^sub>e\<^sub>r\<^sub>s\<^sub>o\<^sub>n3"), (String.explode "Person"), OclAttrNoCast (nil), ()), Oid ((Code_Numeral.Nat 3)))), uncurry cons (I ((String.explode "X\<^sub>P\<^sub>e\<^sub>r\<^sub>s\<^sub>o\<^sub>n2"), I (Ocl_instance_single_ext ((String.explode "X\<^sub>P\<^sub>e\<^sub>r\<^sub>s\<^sub>o\<^sub>n2"), (String.explode "Person"), OclAttrNoCast (uncurry cons (I ((String.explode "salary"), Shall_base (ShallB_term (OclDefInteger ((String.explode "1800"))))), uncurry cons (I ((String.explode "boss"), Shall_base (ShallB_str ((String.explode "X\<^sub>P\<^sub>e\<^sub>r\<^sub>s\<^sub>o\<^sub>n2")))), nil))), ()), Oid ((Code_Numeral.Nat 2)))), uncurry cons (I ((String.explode "X\<^sub>P\<^sub>e\<^sub>r\<^sub>s\<^sub>o\<^sub>n1"), I (Ocl_instance_single_ext ((String.explode "X\<^sub>P\<^sub>e\<^sub>r\<^sub>s\<^sub>o\<^sub>n1"), (String.explode "Person"), OclAttrNoCast (uncurry cons (I ((String.explode "salary"), Shall_base (ShallB_term (OclDefInteger ((String.explode "1300"))))), uncurry cons (I ((String.explode "boss"), Shall_base (ShallB_str ((String.explode "X\<^sub>P\<^sub>e\<^sub>r\<^sub>s\<^sub>o\<^sub>n2")))), nil))), ()), Oid ((Code_Numeral.Nat 1)))), nil))))))))), uncurry cons (I ((String.explode "\<sigma>\<^sub>1'"), uncurry cons (I (Oids ((Code_Numeral.Nat 0), (Code_Numeral.Nat 1), (Code_Numeral.Nat 1)), OclDefCoreBinding (I ((String.explode "X\<^sub>P\<^sub>e\<^sub>r\<^sub>s\<^sub>o\<^sub>n1"), Ocl_instance_single_ext ((String.explode "X\<^sub>P\<^sub>e\<^sub>r\<^sub>s\<^sub>o\<^sub>n1"), (String.explode "Person"), OclAttrNoCast (uncurry cons (I ((String.explode "salary"), Shall_base (ShallB_term (OclDefInteger ((String.explode "1300"))))), uncurry cons (I ((String.explode "boss"), Shall_base (ShallB_str ((String.explode "X\<^sub>P\<^sub>e\<^sub>r\<^sub>s\<^sub>o\<^sub>n2")))), nil))), ())))), uncurry cons (I (Oids ((Code_Numeral.Nat 0), (Code_Numeral.Nat 1), (Code_Numeral.Nat 2)), OclDefCoreBinding (I ((String.explode "X\<^sub>P\<^sub>e\<^sub>r\<^sub>s\<^sub>o\<^sub>n2"), Ocl_instance_single_ext ((String.explode "X\<^sub>P\<^sub>e\<^sub>r\<^sub>s\<^sub>o\<^sub>n2"), (String.explode "Person"), OclAttrNoCast (uncurry cons (I ((String.explode "salary"), Shall_base (ShallB_term (OclDefInteger ((String.explode "1800"))))), uncurry cons (I ((String.explode "boss"), Shall_base (ShallB_str ((String.explode "X\<^sub>P\<^sub>e\<^sub>r\<^sub>s\<^sub>o\<^sub>n2")))), nil))), ())))), uncurry cons (I (Oids ((Code_Numeral.Nat 0), (Code_Numeral.Nat 1), (Code_Numeral.Nat 3)), OclDefCoreBinding (I ((String.explode "X\<^sub>P\<^sub>e\<^sub>r\<^sub>s\<^sub>o\<^sub>n3"), Ocl_instance_single_ext ((String.explode "X\<^sub>P\<^sub>e\<^sub>r\<^sub>s\<^sub>o\<^sub>n3"), (String.explode "Person"), OclAttrNoCast (nil), ())))), uncurry cons (I (Oids ((Code_Numeral.Nat 0), (Code_Numeral.Nat 1), (Code_Numeral.Nat 4)), OclDefCoreBinding (I ((String.explode "X\<^sub>P\<^sub>e\<^sub>r\<^sub>s\<^sub>o\<^sub>n4"), Ocl_instance_single_ext ((String.explode "X\<^sub>P\<^sub>e\<^sub>r\<^sub>s\<^sub>o\<^sub>n4"), (String.explode "Person"), OclAttrNoCast (uncurry cons (I ((String.explode "salary"), Shall_base (ShallB_term (OclDefInteger ((String.explode "2900"))))), nil)), ())))), uncurry cons (I (Oids ((Code_Numeral.Nat 0), (Code_Numeral.Nat 1), (Code_Numeral.Nat 6)), OclDefCoreBinding (I ((String.explode "X\<^sub>P\<^sub>e\<^sub>r\<^sub>s\<^sub>o\<^sub>n6"), Ocl_instance_single_ext ((String.explode "X\<^sub>P\<^sub>e\<^sub>r\<^sub>s\<^sub>o\<^sub>n6"), (String.explode "Person"), OclAttrNoCast (uncurry cons (I ((String.explode "salary"), Shall_base (ShallB_term (OclDefInteger ((String.explode "2500"))))), uncurry cons (I ((String.explode "boss"), Shall_base (ShallB_str ((String.explode "X\<^sub>P\<^sub>e\<^sub>r\<^sub>s\<^sub>o\<^sub>n7")))), nil))), ())))), uncurry cons (I (Oids ((Code_Numeral.Nat 0), (Code_Numeral.Nat 1), (Code_Numeral.Nat 7)), OclDefCoreBinding (I ((String.explode "X\<^sub>P\<^sub>e\<^sub>r\<^sub>s\<^sub>o\<^sub>n7"), Ocl_instance_single_ext ((String.explode "X\<^sub>P\<^sub>e\<^sub>r\<^sub>s\<^sub>o\<^sub>n7"), (String.explode "OclAny"), OclAttrCast ((String.explode "Person"), OclAttrNoCast (uncurry cons (I ((String.explode "salary"), Shall_base (ShallB_term (OclDefInteger ((String.explode "3200"))))), uncurry cons (I ((String.explode "boss"), Shall_base (ShallB_str ((String.explode "X\<^sub>P\<^sub>e\<^sub>r\<^sub>s\<^sub>o\<^sub>n7")))), nil))), nil), ())))), uncurry cons (I (Oids ((Code_Numeral.Nat 0), (Code_Numeral.Nat 1), (Code_Numeral.Nat 8)), OclDefCoreBinding (I ((String.explode "X\<^sub>P\<^sub>e\<^sub>r\<^sub>s\<^sub>o\<^sub>n8"), Ocl_instance_single_ext ((String.explode "X\<^sub>P\<^sub>e\<^sub>r\<^sub>s\<^sub>o\<^sub>n8"), (String.explode "OclAny"), OclAttrNoCast (nil), ())))), uncurry cons (I (Oids ((Code_Numeral.Nat 0), (Code_Numeral.Nat 1), (Code_Numeral.Nat 9)), OclDefCoreBinding (I ((String.explode "X\<^sub>P\<^sub>e\<^sub>r\<^sub>s\<^sub>o\<^sub>n9"), Ocl_instance_single_ext ((String.explode "X\<^sub>P\<^sub>e\<^sub>r\<^sub>s\<^sub>o\<^sub>n9"), (String.explode "Person"), OclAttrNoCast (uncurry cons (I ((String.explode "salary"), Shall_base (ShallB_term (OclDefInteger ((String.explode "0"))))), nil)), ())))), nil))))))))), uncurry cons (I ((String.explode "\<sigma>\<^sub>1"), uncurry cons (I (Oids ((Code_Numeral.Nat 0), (Code_Numeral.Nat 1), (Code_Numeral.Nat 1)), OclDefCoreAdd (Ocl_instance_single_ext ((String.explode ""), (String.explode "Person"), OclAttrNoCast (uncurry cons (I ((String.explode "salary"), Shall_base (ShallB_term (OclDefInteger ((String.explode "1000"))))), uncurry cons (I ((String.explode "boss"), Shall_base (ShallB_self (Oid ((Code_Numeral.Nat 1))))), nil))), ()))), uncurry cons (I (Oids ((Code_Numeral.Nat 0), (Code_Numeral.Nat 1), (Code_Numeral.Nat 2)), OclDefCoreAdd (Ocl_instance_single_ext ((String.explode ""), (String.explode "Person"), OclAttrNoCast (uncurry cons (I ((String.explode "salary"), Shall_base (ShallB_term (OclDefInteger ((String.explode "1200"))))), nil)), ()))), uncurry cons (I (Oids ((Code_Numeral.Nat 0), (Code_Numeral.Nat 1), (Code_Numeral.Nat 4)), OclDefCoreAdd (Ocl_instance_single_ext ((String.explode ""), (String.explode "Person"), OclAttrNoCast (uncurry cons (I ((String.explode "salary"), Shall_base (ShallB_term (OclDefInteger ((String.explode "2600"))))), uncurry cons (I ((String.explode "boss"), Shall_base (ShallB_self (Oid ((Code_Numeral.Nat 4))))), nil))), ()))), uncurry cons (I (Oids ((Code_Numeral.Nat 0), (Code_Numeral.Nat 1), (Code_Numeral.Nat 5)), OclDefCoreBinding (I ((String.explode "X\<^sub>P\<^sub>e\<^sub>r\<^sub>s\<^sub>o\<^sub>n5"), Ocl_instance_single_ext ((String.explode "X\<^sub>P\<^sub>e\<^sub>r\<^sub>s\<^sub>o\<^sub>n5"), (String.explode "Person"), OclAttrNoCast (uncurry cons (I ((String.explode "salary"), Shall_base (ShallB_term (OclDefInteger ((String.explode "3500"))))), nil)), ())))), uncurry cons (I (Oids ((Code_Numeral.Nat 0), (Code_Numeral.Nat 1), (Code_Numeral.Nat 6)), OclDefCoreAdd (Ocl_instance_single_ext ((String.explode ""), (String.explode "Person"), OclAttrNoCast (uncurry cons (I ((String.explode "salary"), Shall_base (ShallB_term (OclDefInteger ((String.explode "2300"))))), uncurry cons (I ((String.explode "boss"), Shall_base (ShallB_self (Oid ((Code_Numeral.Nat 3))))), nil))), ()))), uncurry cons (I (Oids ((Code_Numeral.Nat 0), (Code_Numeral.Nat 1), (Code_Numeral.Nat 9)), OclDefCoreBinding (I ((String.explode "X\<^sub>P\<^sub>e\<^sub>r\<^sub>s\<^sub>o\<^sub>n9"), Ocl_instance_single_ext ((String.explode "X\<^sub>P\<^sub>e\<^sub>r\<^sub>s\<^sub>o\<^sub>n9"), (String.explode "Person"), OclAttrNoCast (uncurry cons (I ((String.explode "salary"), Shall_base (ShallB_term (OclDefInteger ((String.explode "0"))))), nil)), ())))), nil))))))), nil)), true, false, I (uncurry cons ((String.explode "dot\<C>\<O>\<N>\<T>\<E>\<N>\<T>\<S>at_pre"), uncurry cons ((String.explode "dot\<M>\<O>\<V>\<I>\<N>\<G>at_pre"), uncurry cons ((String.explode "dot\<S>\<O>\<U>\<N>\<D>at_pre"), uncurry cons ((String.explode "dot\<W>\<E>\<I>\<G>\<H>\<T>at_pre"), uncurry cons ((String.explode "dot\<W>\<O>\<R>\<M>\<H>\<O>\<L>\<E>at_pre"), uncurry cons ((String.explode "dot\<S>\<A>\<L>\<A>\<R>\<Y>at_pre"), uncurry cons ((String.explode "dot_0_\<B>\<O>\<S>\<S>at_pre"), nil))))))), uncurry cons ((String.explode "dot\<C>\<O>\<N>\<T>\<E>\<N>\<T>\<S>"), uncurry cons ((String.explode "dot\<M>\<O>\<V>\<I>\<N>\<G>"), uncurry cons ((String.explode "dot\<S>\<O>\<U>\<N>\<D>"), uncurry cons ((String.explode "dot\<W>\<E>\<I>\<G>\<H>\<T>"), uncurry cons ((String.explode "dot\<W>\<O>\<R>\<M>\<H>\<O>\<L>\<E>"), uncurry cons ((String.explode "dot\<S>\<A>\<L>\<A>\<R>\<Y>"), uncurry cons ((String.explode "dot_0_\<B>\<O>\<S>\<S>"), nil)))))))), ()) end)))) *}
+consts dot\<C>\<O>\<N>\<T>\<E>\<N>\<T>\<S> :: "Person \<Rightarrow> Set_Integer" ("(_) .contents'(')")
+consts dot\<C>\<O>\<N>\<T>\<E>\<N>\<T>\<S>at_pre :: "Person \<Rightarrow> Set_Integer" ("(_) .contents@pre'(')")
+Context[shallow] Person :: contents () : Set(Integer)
   Post : `result \<triangleq> if (self .boss \<doteq> null)
                    then (Set{}->including(self .salary))
                    else (self .boss .contents()->including(self .salary))
@@ -3454,16 +3387,14 @@ Context[shallow] Person :: contents () : Set(int)
   Pre : `false`
 thm dot\<C>\<O>\<N>\<T>\<E>\<N>\<T>\<S>_def
 
-(* 158 ************************************ 905 + 2 *)
+(* 151 ************************************ 887 + 2 *)
 Context[shallow] Person
   Inv a : `self .boss <> null implies (self .salary  \<triangleq>  ((self .boss) .salary))`
-thm Person_aat_pre_def
-                            Person_a_def
+thm Person_aat_pre_def Person_a_def
 
-(* 159 ************************************ 907 + 2 *)
+(* 152 ************************************ 889 + 2 *)
 Context[shallow] Planet
   Inv A : `true and (self .weight \<le>\<^sub>i\<^sub>n\<^sub>t \<zero>)`
-thm Planet_Aat_pre_def
-                            Planet_A_def
+thm Planet_Aat_pre_def Planet_A_def
 
 end
